feat: Addressed some Mark notes

examples/boogieOutput/boogieOutput.bpl
@@ -1,83 +1,118 @@
-// Dafny 2.3.0.10506
-// Command Line Options: -print:examples/sorting/boogieOutput.bpl examples/sorting/boogieOutput.dfy
+// dafny 4.11.0.0
+// Command Line Options: -print:examples/boogieOutput/boogieOutput.bpl examples/boogieOutput/boogieOutput.dfy
 
-const $$Language$Dafny: bool;
-
+const $$Language$Dafny: bool
+uses {
 axiom $$Language$Dafny;
+}
 
 type Ty;
 
 type Bv0 = int;
 
-const unique TBool: Ty;
+const unique TBool: Ty
+uses {
+axiom Tag(TBool) == TagBool;
+}
 
-const unique TChar: Ty;
+const unique TChar: Ty
+uses {
+axiom Tag(TChar) == TagChar;
+}
 
-const unique TInt: Ty;
+const unique TInt: Ty
+uses {
+axiom Tag(TInt) == TagInt;
+}
 
-const unique TReal: Ty;
+const unique TField: Ty
+uses {
+axiom Tag(TField) == TagField;
+}
 
-const unique TORDINAL: Ty;
+const unique TReal: Ty
+uses {
+axiom Tag(TReal) == TagReal;
+}
 
-function TBitvector(int) : Ty;
+const unique TORDINAL: Ty
+uses {
+axiom Tag(TORDINAL) == TagORDINAL;
+}
 
-function TSet(Ty) : Ty;
-
-function TISet(Ty) : Ty;
-
-function TMultiSet(Ty) : Ty;
-
-function TSeq(Ty) : Ty;
-
-function TMap(Ty, Ty) : Ty;
-
-function TIMap(Ty, Ty) : Ty;
-
-function Inv0_TBitvector(Ty) : int;
+revealed function TBitvector(int) : Ty;
 
 axiom (forall w: int :: { TBitvector(w) } Inv0_TBitvector(TBitvector(w)) == w);
 
-function Inv0_TSet(Ty) : Ty;
+revealed function TSet(Ty) : Ty;
 
 axiom (forall t: Ty :: { TSet(t) } Inv0_TSet(TSet(t)) == t);
 
-function Inv0_TISet(Ty) : Ty;
+axiom (forall t: Ty :: { TSet(t) } Tag(TSet(t)) == TagSet);
+
+revealed function TISet(Ty) : Ty;
 
 axiom (forall t: Ty :: { TISet(t) } Inv0_TISet(TISet(t)) == t);
 
-function Inv0_TSeq(Ty) : Ty;
+axiom (forall t: Ty :: { TISet(t) } Tag(TISet(t)) == TagISet);
 
-axiom (forall t: Ty :: { TSeq(t) } Inv0_TSeq(TSeq(t)) == t);
-
-function Inv0_TMultiSet(Ty) : Ty;
+revealed function TMultiSet(Ty) : Ty;
 
 axiom (forall t: Ty :: { TMultiSet(t) } Inv0_TMultiSet(TMultiSet(t)) == t);
 
-function Inv0_TMap(Ty) : Ty;
+axiom (forall t: Ty :: { TMultiSet(t) } Tag(TMultiSet(t)) == TagMultiSet);
 
-function Inv1_TMap(Ty) : Ty;
+revealed function TSeq(Ty) : Ty;
+
+axiom (forall t: Ty :: { TSeq(t) } Inv0_TSeq(TSeq(t)) == t);
+
+axiom (forall t: Ty :: { TSeq(t) } Tag(TSeq(t)) == TagSeq);
+
+revealed function TMap(Ty, Ty) : Ty;
 
 axiom (forall t: Ty, u: Ty :: { TMap(t, u) } Inv0_TMap(TMap(t, u)) == t);
 
 axiom (forall t: Ty, u: Ty :: { TMap(t, u) } Inv1_TMap(TMap(t, u)) == u);
 
-function Inv0_TIMap(Ty) : Ty;
+axiom (forall t: Ty, u: Ty :: { TMap(t, u) } Tag(TMap(t, u)) == TagMap);
 
-function Inv1_TIMap(Ty) : Ty;
+revealed function TIMap(Ty, Ty) : Ty;
 
 axiom (forall t: Ty, u: Ty :: { TIMap(t, u) } Inv0_TIMap(TIMap(t, u)) == t);
 
 axiom (forall t: Ty, u: Ty :: { TIMap(t, u) } Inv1_TIMap(TIMap(t, u)) == u);
 
+axiom (forall t: Ty, u: Ty :: { TIMap(t, u) } Tag(TIMap(t, u)) == TagIMap);
+
+revealed function Inv0_TBitvector(Ty) : int;
+
+revealed function Inv0_TSet(Ty) : Ty;
+
+revealed function Inv0_TISet(Ty) : Ty;
+
+revealed function Inv0_TSeq(Ty) : Ty;
+
+revealed function Inv0_TMultiSet(Ty) : Ty;
+
+revealed function Inv0_TMap(Ty) : Ty;
+
+revealed function Inv1_TMap(Ty) : Ty;
+
+revealed function Inv0_TIMap(Ty) : Ty;
+
+revealed function Inv1_TIMap(Ty) : Ty;
+
 type TyTag;
 
-function Tag(Ty) : TyTag;
+revealed function Tag(Ty) : TyTag;
 
 const unique TagBool: TyTag;
 
 const unique TagChar: TyTag;
 
 const unique TagInt: TyTag;
+
+const unique TagField: TyTag;
 
 const unique TagReal: TyTag;
 
@@ -97,69 +132,57 @@ const unique TagIMap: TyTag;
 
 const unique TagClass: TyTag;
 
-axiom Tag(TBool) == TagBool;
+type TyTagFamily;
 
-axiom Tag(TChar) == TagChar;
+revealed function TagFamily(Ty) : TyTagFamily;
 
-axiom Tag(TInt) == TagInt;
-
-axiom Tag(TReal) == TagReal;
-
-axiom Tag(TORDINAL) == TagORDINAL;
-
-axiom (forall t: Ty :: { TSet(t) } Tag(TSet(t)) == TagSet);
-
-axiom (forall t: Ty :: { TISet(t) } Tag(TISet(t)) == TagISet);
-
-axiom (forall t: Ty :: { TMultiSet(t) } Tag(TMultiSet(t)) == TagMultiSet);
-
-axiom (forall t: Ty :: { TSeq(t) } Tag(TSeq(t)) == TagSeq);
-
-axiom (forall t: Ty, u: Ty :: { TMap(t, u) } Tag(TMap(t, u)) == TagMap);
-
-axiom (forall t: Ty, u: Ty :: { TIMap(t, u) } Tag(TIMap(t, u)) == TagIMap);
-
-function {:identity} LitInt(x: int) : int;
-
-axiom (forall x: int :: {:identity} { LitInt(x): int } LitInt(x): int == x);
-
-axiom (forall x: int :: { $Box(LitInt(x)) } $Box(LitInt(x)) == Lit($Box(x)));
-
-function {:identity} LitReal(x: real) : real;
-
-axiom (forall x: real :: {:identity} { LitReal(x): real } LitReal(x): real == x);
-
-axiom (forall x: real :: { $Box(LitReal(x)) } $Box(LitReal(x)) == Lit($Box(x)));
-
-function {:identity} Lit<T>(x: T) : T;
-
+revealed function {:identity} Lit<T>(x: T) : T
+uses {
 axiom (forall<T> x: T :: {:identity} { Lit(x): T } Lit(x): T == x);
+}
 
 axiom (forall<T> x: T :: { $Box(Lit(x)) } $Box(Lit(x)) == Lit($Box(x)));
 
+revealed function {:identity} LitInt(x: int) : int
+uses {
+axiom (forall x: int :: {:identity} { LitInt(x): int } LitInt(x): int == x);
+}
+
+axiom (forall x: int :: { $Box(LitInt(x)) } $Box(LitInt(x)) == Lit($Box(x)));
+
+revealed function {:identity} LitReal(x: real) : real
+uses {
+axiom (forall x: real :: {:identity} { LitReal(x): real } LitReal(x): real == x);
+}
+
+axiom (forall x: real :: { $Box(LitReal(x)) } $Box(LitReal(x)) == Lit($Box(x)));
+
+revealed function {:inline} char#IsChar(n: int) : bool
+{
+  (0 <= n && n < 55296) || (57344 <= n && n < 1114112)
+}
+
 type char;
 
-function char#FromInt(int) : char;
-
-function char#ToInt(char) : int;
-
-axiom (forall ch: char :: 
-  { char#ToInt(ch) } 
-  char#FromInt(char#ToInt(ch)) == ch
-     && 0 <= char#ToInt(ch)
-     && char#ToInt(ch) < 65536);
+revealed function char#FromInt(int) : char;
 
 axiom (forall n: int :: 
   { char#FromInt(n) } 
-  0 <= n && n < 65536 ==> char#ToInt(char#FromInt(n)) == n);
+  char#IsChar(n) ==> char#ToInt(char#FromInt(n)) == n);
 
-function char#Plus(char, char) : char;
+revealed function char#ToInt(char) : int;
 
-function char#Minus(char, char) : char;
+axiom (forall ch: char :: 
+  { char#ToInt(ch) } 
+  char#FromInt(char#ToInt(ch)) == ch && char#IsChar(char#ToInt(ch)));
+
+revealed function char#Plus(char, char) : char;
 
 axiom (forall a: char, b: char :: 
   { char#Plus(a, b) } 
   char#Plus(a, b) == char#FromInt(char#ToInt(a) + char#ToInt(b)));
+
+revealed function char#Minus(char, char) : char;
 
 axiom (forall a: char, b: char :: 
   { char#Minus(a, b) } 
@@ -169,19 +192,39 @@ type ref;
 
 const null: ref;
 
-const unique NoTraitAtAll: ClassName;
+const locals: ref;
 
-function TraitParent(ClassName) : ClassName;
+type FieldFamily;
+
+const unique object_field: FieldFamily;
+
+revealed function field_depth(f: Field) : int;
+
+revealed function field_family(f: Field) : FieldFamily;
+
+revealed function local_field(ff: FieldFamily, depth: int) : Field
+uses {
+axiom (forall ff: FieldFamily, depth: int :: 
+  {:trigger local_field(ff, depth)} 
+  field_depth(local_field(ff, depth)) == depth
+     && field_family(local_field(ff, depth)) == ff);
+}
 
 type Box;
 
 const $ArbitraryBoxValue: Box;
 
-function $Box<T>(T) : Box;
+revealed function $Box<T>(T) : Box;
 
-function $Unbox<T>(Box) : T;
+revealed function $Unbox<T>(Box) : T;
 
-axiom (forall<T> x: T :: { $Box(x) } $Unbox($Box(x)) == x);
+axiom (forall<T> x: T :: {:weight 3} { $Box(x) } $Unbox($Box(x)) == x);
+
+axiom (forall<T> x: Box :: { $Unbox(x): T } $Box($Unbox(x): T) == x);
+
+revealed function $IsBox(Box, Ty) : bool;
+
+revealed function $IsAllocBox(Box, Ty, Heap) : bool;
 
 axiom (forall bx: Box :: 
   { $IsBox(bx, TInt) } 
@@ -202,37 +245,40 @@ axiom (forall bx: Box ::
   $IsBox(bx, TChar)
      ==> $Box($Unbox(bx): char) == bx && $Is($Unbox(bx): char, TChar));
 
+axiom (forall bx: Box :: 
+  { $IsBox(bx, TBitvector(0)) } 
+  $IsBox(bx, TBitvector(0))
+     ==> $Box($Unbox(bx): Bv0) == bx && $Is($Unbox(bx): Bv0, TBitvector(0)));
+
 axiom (forall bx: Box, t: Ty :: 
   { $IsBox(bx, TSet(t)) } 
   $IsBox(bx, TSet(t))
-     ==> $Box($Unbox(bx): Set Box) == bx && $Is($Unbox(bx): Set Box, TSet(t)));
+     ==> $Box($Unbox(bx): Set) == bx && $Is($Unbox(bx): Set, TSet(t)));
 
 axiom (forall bx: Box, t: Ty :: 
   { $IsBox(bx, TISet(t)) } 
   $IsBox(bx, TISet(t))
-     ==> $Box($Unbox(bx): ISet Box) == bx && $Is($Unbox(bx): ISet Box, TISet(t)));
+     ==> $Box($Unbox(bx): ISet) == bx && $Is($Unbox(bx): ISet, TISet(t)));
 
 axiom (forall bx: Box, t: Ty :: 
   { $IsBox(bx, TMultiSet(t)) } 
   $IsBox(bx, TMultiSet(t))
-     ==> $Box($Unbox(bx): MultiSet Box) == bx
-       && $Is($Unbox(bx): MultiSet Box, TMultiSet(t)));
+     ==> $Box($Unbox(bx): MultiSet) == bx && $Is($Unbox(bx): MultiSet, TMultiSet(t)));
 
 axiom (forall bx: Box, t: Ty :: 
   { $IsBox(bx, TSeq(t)) } 
   $IsBox(bx, TSeq(t))
-     ==> $Box($Unbox(bx): Seq Box) == bx && $Is($Unbox(bx): Seq Box, TSeq(t)));
+     ==> $Box($Unbox(bx): Seq) == bx && $Is($Unbox(bx): Seq, TSeq(t)));
 
 axiom (forall bx: Box, s: Ty, t: Ty :: 
   { $IsBox(bx, TMap(s, t)) } 
   $IsBox(bx, TMap(s, t))
-     ==> $Box($Unbox(bx): Map Box Box) == bx && $Is($Unbox(bx): Map Box Box, TMap(s, t)));
+     ==> $Box($Unbox(bx): Map) == bx && $Is($Unbox(bx): Map, TMap(s, t)));
 
 axiom (forall bx: Box, s: Ty, t: Ty :: 
   { $IsBox(bx, TIMap(s, t)) } 
   $IsBox(bx, TIMap(s, t))
-     ==> $Box($Unbox(bx): IMap Box Box) == bx
-       && $Is($Unbox(bx): IMap Box Box, TIMap(s, t)));
+     ==> $Box($Unbox(bx): IMap) == bx && $Is($Unbox(bx): IMap, TIMap(s, t)));
 
 axiom (forall<T> v: T, t: Ty :: 
   { $IsBox($Box(v), t) } 
@@ -242,13 +288,7 @@ axiom (forall<T> v: T, t: Ty, h: Heap ::
   { $IsAllocBox($Box(v), t, h) } 
   $IsAllocBox($Box(v), t, h) <==> $IsAlloc(v, t, h));
 
-function $Is<T>(T, Ty) : bool;
-
-function $IsAlloc<T>(T, Ty, Heap) : bool;
-
-function $IsBox<T>(T, Ty) : bool;
-
-function $IsAllocBox<T>(T, Ty, Heap) : bool;
+revealed function $Is<T>(T, Ty) : bool;
 
 axiom (forall v: int :: { $Is(v, TInt) } $Is(v, TInt));
 
@@ -258,7 +298,71 @@ axiom (forall v: bool :: { $Is(v, TBool) } $Is(v, TBool));
 
 axiom (forall v: char :: { $Is(v, TChar) } $Is(v, TChar));
 
+axiom (forall v: Field :: { $Is(v, TField) } $Is(v, TField));
+
 axiom (forall v: ORDINAL :: { $Is(v, TORDINAL) } $Is(v, TORDINAL));
+
+axiom (forall v: Bv0 :: { $Is(v, TBitvector(0)) } $Is(v, TBitvector(0)));
+
+axiom (forall v: Set, t0: Ty :: 
+  { $Is(v, TSet(t0)) } 
+  $Is(v, TSet(t0))
+     <==> (forall bx: Box :: 
+      { Set#IsMember(v, bx) } 
+      Set#IsMember(v, bx) ==> $IsBox(bx, t0)));
+
+axiom (forall v: ISet, t0: Ty :: 
+  { $Is(v, TISet(t0)) } 
+  $Is(v, TISet(t0)) <==> (forall bx: Box :: { v[bx] } v[bx] ==> $IsBox(bx, t0)));
+
+axiom (forall v: MultiSet, t0: Ty :: 
+  { $Is(v, TMultiSet(t0)) } 
+  $Is(v, TMultiSet(t0))
+     <==> (forall bx: Box :: 
+      { MultiSet#Multiplicity(v, bx) } 
+      0 < MultiSet#Multiplicity(v, bx) ==> $IsBox(bx, t0)));
+
+axiom (forall v: MultiSet, t0: Ty :: 
+  { $Is(v, TMultiSet(t0)) } 
+  $Is(v, TMultiSet(t0)) ==> $IsGoodMultiSet(v));
+
+axiom (forall v: Seq, t0: Ty :: 
+  { $Is(v, TSeq(t0)) } 
+  $Is(v, TSeq(t0))
+     <==> (forall i: int :: 
+      { Seq#Index(v, i) } 
+      0 <= i && i < Seq#Length(v) ==> $IsBox(Seq#Index(v, i), t0)));
+
+axiom (forall v: Map, t0: Ty, t1: Ty :: 
+  { $Is(v, TMap(t0, t1)) } 
+  $Is(v, TMap(t0, t1))
+     <==> (forall bx: Box :: 
+      { Map#Elements(v)[bx] } { Set#IsMember(Map#Domain(v), bx) } 
+      Set#IsMember(Map#Domain(v), bx)
+         ==> $IsBox(Map#Elements(v)[bx], t1) && $IsBox(bx, t0)));
+
+axiom (forall v: Map, t0: Ty, t1: Ty :: 
+  { $Is(v, TMap(t0, t1)) } 
+  $Is(v, TMap(t0, t1))
+     ==> $Is(Map#Domain(v), TSet(t0))
+       && $Is(Map#Values(v), TSet(t1))
+       && $Is(Map#Items(v), TSet(Tclass._System.Tuple2(t0, t1))));
+
+axiom (forall v: IMap, t0: Ty, t1: Ty :: 
+  { $Is(v, TIMap(t0, t1)) } 
+  $Is(v, TIMap(t0, t1))
+     <==> (forall bx: Box :: 
+      { IMap#Elements(v)[bx] } { IMap#Domain(v)[bx] } 
+      IMap#Domain(v)[bx] ==> $IsBox(IMap#Elements(v)[bx], t1) && $IsBox(bx, t0)));
+
+axiom (forall v: IMap, t0: Ty, t1: Ty :: 
+  { $Is(v, TIMap(t0, t1)) } 
+  $Is(v, TIMap(t0, t1))
+     ==> $Is(IMap#Domain(v), TISet(t0))
+       && $Is(IMap#Values(v), TISet(t1))
+       && $Is(IMap#Items(v), TISet(Tclass._System.Tuple2(t0, t1))));
+
+revealed function $IsAlloc<T>(T, Ty, Heap) : bool;
 
 axiom (forall h: Heap, v: int :: { $IsAlloc(v, TInt, h) } $IsAlloc(v, TInt, h));
 
@@ -272,81 +376,62 @@ axiom (forall h: Heap, v: ORDINAL ::
   { $IsAlloc(v, TORDINAL, h) } 
   $IsAlloc(v, TORDINAL, h));
 
-axiom (forall v: Set Box, t0: Ty :: 
-  { $Is(v, TSet(t0)) } 
-  $Is(v, TSet(t0)) <==> (forall bx: Box :: { v[bx] } v[bx] ==> $IsBox(bx, t0)));
+axiom (forall v: Bv0, h: Heap :: 
+  { $IsAlloc(v, TBitvector(0), h) } 
+  $IsAlloc(v, TBitvector(0), h));
 
-axiom (forall v: ISet Box, t0: Ty :: 
-  { $Is(v, TISet(t0)) } 
-  $Is(v, TISet(t0)) <==> (forall bx: Box :: { v[bx] } v[bx] ==> $IsBox(bx, t0)));
-
-axiom (forall v: MultiSet Box, t0: Ty :: 
-  { $Is(v, TMultiSet(t0)) } 
-  $Is(v, TMultiSet(t0))
-     <==> (forall bx: Box :: { v[bx] } 0 < v[bx] ==> $IsBox(bx, t0)));
-
-axiom (forall v: MultiSet Box, t0: Ty :: 
-  { $Is(v, TMultiSet(t0)) } 
-  $Is(v, TMultiSet(t0)) ==> $IsGoodMultiSet(v));
-
-axiom (forall v: Seq Box, t0: Ty :: 
-  { $Is(v, TSeq(t0)) } 
-  $Is(v, TSeq(t0))
-     <==> (forall i: int :: 
-      { Seq#Index(v, i) } 
-      0 <= i && i < Seq#Length(v) ==> $IsBox(Seq#Index(v, i), t0)));
-
-axiom (forall v: Set Box, t0: Ty, h: Heap :: 
+axiom (forall v: Set, t0: Ty, h: Heap :: 
   { $IsAlloc(v, TSet(t0), h) } 
   $IsAlloc(v, TSet(t0), h)
-     <==> (forall bx: Box :: { v[bx] } v[bx] ==> $IsAllocBox(bx, t0, h)));
+     <==> (forall bx: Box :: 
+      { Set#IsMember(v, bx) } 
+      Set#IsMember(v, bx) ==> $IsAllocBox(bx, t0, h)));
 
-axiom (forall v: ISet Box, t0: Ty, h: Heap :: 
+axiom (forall v: ISet, t0: Ty, h: Heap :: 
   { $IsAlloc(v, TISet(t0), h) } 
   $IsAlloc(v, TISet(t0), h)
      <==> (forall bx: Box :: { v[bx] } v[bx] ==> $IsAllocBox(bx, t0, h)));
 
-axiom (forall v: MultiSet Box, t0: Ty, h: Heap :: 
+axiom (forall v: MultiSet, t0: Ty, h: Heap :: 
   { $IsAlloc(v, TMultiSet(t0), h) } 
   $IsAlloc(v, TMultiSet(t0), h)
-     <==> (forall bx: Box :: { v[bx] } 0 < v[bx] ==> $IsAllocBox(bx, t0, h)));
+     <==> (forall bx: Box :: 
+      { MultiSet#Multiplicity(v, bx) } 
+      0 < MultiSet#Multiplicity(v, bx) ==> $IsAllocBox(bx, t0, h)));
 
-axiom (forall v: Seq Box, t0: Ty, h: Heap :: 
+axiom (forall v: Seq, t0: Ty, h: Heap :: 
   { $IsAlloc(v, TSeq(t0), h) } 
   $IsAlloc(v, TSeq(t0), h)
      <==> (forall i: int :: 
       { Seq#Index(v, i) } 
       0 <= i && i < Seq#Length(v) ==> $IsAllocBox(Seq#Index(v, i), t0, h)));
 
-axiom (forall v: Map Box Box, t0: Ty, t1: Ty :: 
-  { $Is(v, TMap(t0, t1)) } 
-  $Is(v, TMap(t0, t1))
-     <==> (forall bx: Box :: 
-      { Map#Elements(v)[bx] } { Map#Domain(v)[bx] } 
-      Map#Domain(v)[bx] ==> $IsBox(Map#Elements(v)[bx], t1) && $IsBox(bx, t0)));
-
-axiom (forall v: Map Box Box, t0: Ty, t1: Ty, h: Heap :: 
+axiom (forall v: Map, t0: Ty, t1: Ty, h: Heap :: 
   { $IsAlloc(v, TMap(t0, t1), h) } 
   $IsAlloc(v, TMap(t0, t1), h)
      <==> (forall bx: Box :: 
-      { Map#Elements(v)[bx] } { Map#Domain(v)[bx] } 
-      Map#Domain(v)[bx]
+      { Map#Elements(v)[bx] } { Set#IsMember(Map#Domain(v), bx) } 
+      Set#IsMember(Map#Domain(v), bx)
          ==> $IsAllocBox(Map#Elements(v)[bx], t1, h) && $IsAllocBox(bx, t0, h)));
 
-axiom (forall v: IMap Box Box, t0: Ty, t1: Ty :: 
-  { $Is(v, TIMap(t0, t1)) } 
-  $Is(v, TIMap(t0, t1))
-     <==> (forall bx: Box :: 
-      { IMap#Elements(v)[bx] } { IMap#Domain(v)[bx] } 
-      IMap#Domain(v)[bx] ==> $IsBox(IMap#Elements(v)[bx], t1) && $IsBox(bx, t0)));
-
-axiom (forall v: IMap Box Box, t0: Ty, t1: Ty, h: Heap :: 
+axiom (forall v: IMap, t0: Ty, t1: Ty, h: Heap :: 
   { $IsAlloc(v, TIMap(t0, t1), h) } 
   $IsAlloc(v, TIMap(t0, t1), h)
      <==> (forall bx: Box :: 
       { IMap#Elements(v)[bx] } { IMap#Domain(v)[bx] } 
       IMap#Domain(v)[bx]
          ==> $IsAllocBox(IMap#Elements(v)[bx], t1, h) && $IsAllocBox(bx, t0, h)));
+
+revealed function $AlwaysAllocated(Ty) : bool;
+
+axiom (forall ty: Ty :: 
+  { $AlwaysAllocated(ty) } 
+  $AlwaysAllocated(ty)
+     ==> (forall h: Heap, v: Box :: 
+      { $IsAllocBox(v, ty, h) } 
+      $IsBox(v, ty) ==> $IsAllocBox(v, ty, h)));
+
+revealed function $OlderTag(Heap) : bool;
 
 type ClassName;
 
@@ -360,15 +445,22 @@ const unique class._System.seq: ClassName;
 
 const unique class._System.multiset: ClassName;
 
-function Tclass._System.object?() : Ty;
+revealed function Tclass._System.object?() : Ty
+uses {
+// Tclass._System.object? Tag
+axiom Tag(Tclass._System.object?()) == Tagclass._System.object?
+   && TagFamily(Tclass._System.object?()) == tytagFamily$object;
+}
 
-function dtype(ref) : Ty;
+revealed function Tclass._System.Tuple2(Ty, Ty) : Ty;
 
-function TypeTuple(a: ClassName, b: ClassName) : ClassName;
+revealed function dtype(ref) : Ty;
 
-function TypeTupleCar(ClassName) : ClassName;
+revealed function TypeTuple(a: ClassName, b: ClassName) : ClassName;
 
-function TypeTupleCdr(ClassName) : ClassName;
+revealed function TypeTupleCar(ClassName) : ClassName;
+
+revealed function TypeTupleCdr(ClassName) : ClassName;
 
 axiom (forall a: ClassName, b: ClassName :: 
   { TypeTuple(a, b) } 
@@ -376,47 +468,49 @@ axiom (forall a: ClassName, b: ClassName ::
 
 type HandleType;
 
-function SetRef_to_SetBox(s: [ref]bool) : Set Box;
+revealed function SetRef_to_SetBox(s: [ref]bool) : Set;
 
 axiom (forall s: [ref]bool, bx: Box :: 
-  { SetRef_to_SetBox(s)[bx] } 
-  SetRef_to_SetBox(s)[bx] == s[$Unbox(bx): ref]);
+  { Set#IsMember(SetRef_to_SetBox(s), bx) } 
+  Set#IsMember(SetRef_to_SetBox(s), bx) == s[$Unbox(bx): ref]);
 
 axiom (forall s: [ref]bool :: 
   { SetRef_to_SetBox(s) } 
   $Is(SetRef_to_SetBox(s), TSet(Tclass._System.object?())));
 
+revealed function Apply1(Ty, Ty, Heap, HandleType, Box) : Box;
+
 type DatatypeType;
 
 type DtCtorId;
 
-function DatatypeCtorId(DatatypeType) : DtCtorId;
+revealed function DatatypeCtorId(DatatypeType) : DtCtorId;
 
-function DtRank(DatatypeType) : int;
+revealed function DtRank(DatatypeType) : int;
 
-function BoxRank(Box) : int;
+revealed function BoxRank(Box) : int;
 
 axiom (forall d: DatatypeType :: { BoxRank($Box(d)) } BoxRank($Box(d)) == DtRank(d));
 
 type ORDINAL = Box;
 
-function ORD#IsNat(ORDINAL) : bool;
+revealed function ORD#IsNat(ORDINAL) : bool;
 
-function ORD#Offset(ORDINAL) : int;
+revealed function ORD#Offset(ORDINAL) : int;
 
 axiom (forall o: ORDINAL :: { ORD#Offset(o) } 0 <= ORD#Offset(o));
 
-function {:inline} ORD#IsLimit(o: ORDINAL) : bool
+revealed function {:inline} ORD#IsLimit(o: ORDINAL) : bool
 {
   ORD#Offset(o) == 0
 }
 
-function {:inline} ORD#IsSucc(o: ORDINAL) : bool
+revealed function {:inline} ORD#IsSucc(o: ORDINAL) : bool
 {
   0 < ORD#Offset(o)
 }
 
-function ORD#FromNat(int) : ORDINAL;
+revealed function ORD#FromNat(int) : ORDINAL;
 
 axiom (forall n: int :: 
   { ORD#FromNat(n) } 
@@ -426,16 +520,15 @@ axiom (forall o: ORDINAL ::
   { ORD#Offset(o) } { ORD#IsNat(o) } 
   ORD#IsNat(o) ==> o == ORD#FromNat(ORD#Offset(o)));
 
-function ORD#Less(ORDINAL, ORDINAL) : bool;
+revealed function ORD#Less(ORDINAL, ORDINAL) : bool;
 
 axiom (forall o: ORDINAL, p: ORDINAL :: 
   { ORD#Less(o, p) } 
   (ORD#Less(o, p) ==> o != p)
      && (ORD#IsNat(o) && !ORD#IsNat(p) ==> ORD#Less(o, p))
      && (ORD#IsNat(o) && ORD#IsNat(p)
-       ==> ORD#Less(o, p) == (ORD#Offset(o) < ORD#Offset(p))));
-
-axiom (forall o: ORDINAL, p: ORDINAL :: { ORD#Less(o, p) } ORD#Less(o, p) ==> o != p);
+       ==> ORD#Less(o, p) == (ORD#Offset(o) < ORD#Offset(p)))
+     && (ORD#Less(o, p) && ORD#IsNat(p) ==> ORD#IsNat(o)));
 
 axiom (forall o: ORDINAL, p: ORDINAL :: 
   { ORD#Less(o, p), ORD#Less(p, o) } 
@@ -445,13 +538,13 @@ axiom (forall o: ORDINAL, p: ORDINAL, r: ORDINAL ::
   { ORD#Less(o, p), ORD#Less(p, r) } { ORD#Less(o, p), ORD#Less(o, r) } 
   ORD#Less(o, p) && ORD#Less(p, r) ==> ORD#Less(o, r));
 
-function ORD#LessThanLimit(ORDINAL, ORDINAL) : bool;
+revealed function ORD#LessThanLimit(ORDINAL, ORDINAL) : bool;
 
 axiom (forall o: ORDINAL, p: ORDINAL :: 
   { ORD#LessThanLimit(o, p) } 
   ORD#LessThanLimit(o, p) == ORD#Less(o, p));
 
-function ORD#Plus(ORDINAL, ORDINAL) : ORDINAL;
+revealed function ORD#Plus(ORDINAL, ORDINAL) : ORDINAL;
 
 axiom (forall o: ORDINAL, p: ORDINAL :: 
   { ORD#Plus(o, p) } 
@@ -470,7 +563,7 @@ axiom (forall o: ORDINAL, p: ORDINAL ::
   (o == ORD#FromNat(0) ==> ORD#Plus(o, p) == p)
      && (p == ORD#FromNat(0) ==> ORD#Plus(o, p) == o));
 
-function ORD#Minus(ORDINAL, ORDINAL) : ORDINAL;
+revealed function ORD#Minus(ORDINAL, ORDINAL) : ORDINAL;
 
 axiom (forall o: ORDINAL, p: ORDINAL :: 
   { ORD#Minus(o, p) } 
@@ -516,19 +609,15 @@ axiom (forall o: ORDINAL, m: int, n: int ::
          ==> ORD#Plus(ORD#Minus(o, ORD#FromNat(m)), ORD#FromNat(n))
            == ORD#Plus(o, ORD#FromNat(n - m))));
 
-const $ModuleContextHeight: int;
-
-const $FunctionContextHeight: int;
-
 type LayerType;
 
 const $LZ: LayerType;
 
-function $LS(LayerType) : LayerType;
+revealed function $LS(LayerType) : LayerType;
 
-function AsFuelBottom(LayerType) : LayerType;
+revealed function AsFuelBottom(LayerType) : LayerType;
 
-function AtLayer<A>([LayerType]A, LayerType) : A;
+revealed function AtLayer<A>([LayerType]A, LayerType) : A;
 
 axiom (forall<A> f: [LayerType]A, ly: LayerType :: 
   { AtLayer(f, ly) } 
@@ -538,47 +627,64 @@ axiom (forall<A> f: [LayerType]A, ly: LayerType ::
   { AtLayer(f, $LS(ly)) } 
   AtLayer(f, $LS(ly)) == AtLayer(f, ly));
 
-type Field _;
+type Field;
 
-function FDim<T>(Field T) : int;
+revealed function FDim(Field) : int
+uses {
+axiom FDim(alloc) == 0;
+}
 
-function IndexField(int) : Field Box;
+revealed function IndexField(int) : Field;
 
 axiom (forall i: int :: { IndexField(i) } FDim(IndexField(i)) == 1);
 
-function IndexField_Inverse<T>(Field T) : int;
+revealed function IndexField_Inverse(Field) : int;
 
 axiom (forall i: int :: { IndexField(i) } IndexField_Inverse(IndexField(i)) == i);
 
-function MultiIndexField(Field Box, int) : Field Box;
+revealed function MultiIndexField(Field, int) : Field;
 
-axiom (forall f: Field Box, i: int :: 
+axiom (forall f: Field, i: int :: 
   { MultiIndexField(f, i) } 
   FDim(MultiIndexField(f, i)) == FDim(f) + 1);
 
-function MultiIndexField_Inverse0<T>(Field T) : Field T;
+revealed function MultiIndexField_Inverse0(Field) : Field;
 
-function MultiIndexField_Inverse1<T>(Field T) : int;
+revealed function MultiIndexField_Inverse1(Field) : int;
 
-axiom (forall f: Field Box, i: int :: 
+axiom (forall f: Field, i: int :: 
   { MultiIndexField(f, i) } 
   MultiIndexField_Inverse0(MultiIndexField(f, i)) == f
      && MultiIndexField_Inverse1(MultiIndexField(f, i)) == i);
 
-function DeclType<T>(Field T) : ClassName;
+revealed function DeclType(Field) : ClassName;
 
 type NameFamily;
 
-function DeclName<T>(Field T) : NameFamily;
+revealed function DeclName(Field) : NameFamily
+uses {
+axiom DeclName(alloc) == allocName;
+}
 
-function FieldOfDecl<alpha>(ClassName, NameFamily) : Field alpha;
+revealed function FieldOfDecl(ClassName, NameFamily) : Field;
 
-axiom (forall<T> cl: ClassName, nm: NameFamily :: 
-  { FieldOfDecl(cl, nm): Field T } 
-  DeclType(FieldOfDecl(cl, nm): Field T) == cl
-     && DeclName(FieldOfDecl(cl, nm): Field T) == nm);
+axiom (forall cl: ClassName, nm: NameFamily :: 
+  { FieldOfDecl(cl, nm): Field } 
+  DeclType(FieldOfDecl(cl, nm): Field) == cl
+     && DeclName(FieldOfDecl(cl, nm): Field) == nm);
 
-function $IsGhostField<T>(Field T) : bool;
+revealed function $IsGhostField(Field) : bool
+uses {
+axiom $IsGhostField(alloc);
+}
+
+axiom (forall h: Heap, k: Heap :: 
+  { $HeapSuccGhost(h, k) } 
+  $HeapSuccGhost(h, k)
+     ==> $HeapSucc(h, k)
+       && (forall o: ref, f: Field :: 
+        { read(k, o, f) } 
+        !$IsGhostField(f) ==> read(h, o, f) == read(k, o, f)));
 
 axiom (forall<T> h: Heap, k: Heap, v: T, t: Ty :: 
   { $HeapSucc(h, k), $IsAlloc(v, t, h) } 
@@ -588,237 +694,224 @@ axiom (forall h: Heap, k: Heap, bx: Box, t: Ty ::
   { $HeapSucc(h, k), $IsAllocBox(bx, t, h) } 
   $HeapSucc(h, k) ==> $IsAllocBox(bx, t, h) ==> $IsAllocBox(bx, t, k));
 
-const unique alloc: Field bool;
+const unique alloc: Field;
 
 const unique allocName: NameFamily;
 
-axiom FDim(alloc) == 0 && DeclName(alloc) == allocName && !$IsGhostField(alloc);
+revealed function _System.array.Length(a: ref) : int;
 
-function _System.array.Length(a: ref) : int;
+axiom (forall o: ref :: { _System.array.Length(o) } 0 <= _System.array.Length(o));
 
-axiom (forall o: ref :: 0 <= _System.array.Length(o));
-
-function Int(x: real) : int;
-
+revealed function Int(x: real) : int
+uses {
 axiom (forall x: real :: { Int(x): int } Int(x): int == int(x));
+}
 
-function Real(x: int) : real;
-
+revealed function Real(x: int) : real
+uses {
 axiom (forall x: int :: { Real(x): real } Real(x): real == real(x));
+}
 
 axiom (forall i: int :: { Int(Real(i)) } Int(Real(i)) == i);
 
-function {:inline} _System.real.Floor(x: real) : int
+revealed function {:inline} _System.real.Floor(x: real) : int
 {
   Int(x)
 }
 
-type Heap = <alpha>[ref,Field alpha]alpha;
+type Heap = [ref][Field]Box;
 
-function {:inline} read<alpha>(H: Heap, r: ref, f: Field alpha) : alpha
+revealed function {:inline} read(H: Heap, r: ref, f: Field) : Box
 {
-  H[r, f]
+  H[r][f]
 }
 
-function {:inline} update<alpha>(H: Heap, r: ref, f: Field alpha, v: alpha) : Heap
+revealed function {:inline} update(H: Heap, r: ref, f: Field, v: Box) : Heap
 {
-  H[r, f := v]
+  H[r := H[r][f := v]]
 }
 
-function $IsGoodHeap(Heap) : bool;
+revealed function $IsGoodHeap(Heap) : bool;
 
-function $IsHeapAnchor(Heap) : bool;
+revealed function $IsHeapAnchor(Heap) : bool;
 
 var $Heap: Heap where $IsGoodHeap($Heap) && $IsHeapAnchor($Heap);
 
-const $OneHeap: Heap;
-
+const $OneHeap: Heap
+uses {
 axiom $IsGoodHeap($OneHeap);
+}
 
-function $HeapSucc(Heap, Heap) : bool;
+revealed function $HeapSucc(Heap, Heap) : bool;
 
-axiom (forall<alpha> h: Heap, r: ref, f: Field alpha, x: alpha :: 
+axiom (forall h: Heap, r: ref, f: Field, x: Box :: 
   { update(h, r, f, x) } 
   $IsGoodHeap(update(h, r, f, x)) ==> $HeapSucc(h, update(h, r, f, x)));
 
 axiom (forall a: Heap, b: Heap, c: Heap :: 
   { $HeapSucc(a, b), $HeapSucc(b, c) } 
-  $HeapSucc(a, b) && $HeapSucc(b, c) ==> $HeapSucc(a, c));
+  a != c ==> $HeapSucc(a, b) && $HeapSucc(b, c) ==> $HeapSucc(a, c));
 
 axiom (forall h: Heap, k: Heap :: 
   { $HeapSucc(h, k) } 
   $HeapSucc(h, k)
-     ==> (forall o: ref :: { read(k, o, alloc) } read(h, o, alloc) ==> read(k, o, alloc)));
+     ==> (forall o: ref :: 
+      { read(k, o, alloc) } 
+      $Unbox(read(h, o, alloc)) ==> $Unbox(read(k, o, alloc))));
 
-function $HeapSuccGhost(Heap, Heap) : bool;
+revealed function $HeapSuccGhost(Heap, Heap) : bool;
 
-axiom (forall h: Heap, k: Heap :: 
-  { $HeapSuccGhost(h, k) } 
-  $HeapSuccGhost(h, k)
-     ==> $HeapSucc(h, k)
-       && (forall<alpha> o: ref, f: Field alpha :: 
-        { read(k, o, f) } 
-        !$IsGhostField(f) ==> read(h, o, f) == read(k, o, f)));
-
-type TickType;
-
-var $Tick: TickType;
-
-procedure $YieldHavoc(this: ref, rds: Set Box, nw: Set Box);
+procedure $YieldHavoc(this: ref, rds: Set, nw: Set);
   modifies $Heap;
-  ensures (forall<alpha> $o: ref, $f: Field alpha :: 
+  ensures (forall $o: ref, $f: Field :: 
     { read($Heap, $o, $f) } 
-    $o != null && read(old($Heap), $o, alloc)
+    $o != null && $Unbox(read(old($Heap), $o, alloc))
        ==> 
-      $o == this || rds[$Box($o)] || nw[$Box($o)]
+      $o == this || Set#IsMember(rds, $Box($o)) || Set#IsMember(nw, $Box($o))
        ==> read($Heap, $o, $f) == read(old($Heap), $o, $f));
   ensures $HeapSucc(old($Heap), $Heap);
 
 
 
-procedure $IterHavoc0(this: ref, rds: Set Box, modi: Set Box);
+procedure $IterHavoc0(this: ref, rds: Set, modi: Set);
   modifies $Heap;
-  ensures (forall<alpha> $o: ref, $f: Field alpha :: 
+  ensures (forall $o: ref, $f: Field :: 
     { read($Heap, $o, $f) } 
-    $o != null && read(old($Heap), $o, alloc)
+    $o != null && $Unbox(read(old($Heap), $o, alloc))
        ==> 
-      rds[$Box($o)] && !modi[$Box($o)] && $o != this
+      Set#IsMember(rds, $Box($o)) && !Set#IsMember(modi, $Box($o)) && $o != this
        ==> read($Heap, $o, $f) == read(old($Heap), $o, $f));
   ensures $HeapSucc(old($Heap), $Heap);
 
 
 
-procedure $IterHavoc1(this: ref, modi: Set Box, nw: Set Box);
+procedure $IterHavoc1(this: ref, modi: Set, nw: Set);
   modifies $Heap;
-  ensures (forall<alpha> $o: ref, $f: Field alpha :: 
+  ensures (forall $o: ref, $f: Field :: 
     { read($Heap, $o, $f) } 
-    $o != null && read(old($Heap), $o, alloc)
+    $o != null && $Unbox(read(old($Heap), $o, alloc))
        ==> read($Heap, $o, $f) == read(old($Heap), $o, $f)
          || $o == this
-         || modi[$Box($o)]
-         || nw[$Box($o)]);
+         || Set#IsMember(modi, $Box($o))
+         || Set#IsMember(nw, $Box($o)));
   ensures $HeapSucc(old($Heap), $Heap);
 
 
 
-procedure $IterCollectNewObjects(prevHeap: Heap, newHeap: Heap, this: ref, NW: Field (Set Box))
-   returns (s: Set Box);
+procedure $IterCollectNewObjects(prevHeap: Heap, newHeap: Heap, this: ref, NW: Field) returns (s: Set);
   ensures (forall bx: Box :: 
-    { s[bx] } 
-    s[bx]
-       <==> read(newHeap, this, NW)[bx]
+    { Set#IsMember(s, bx) } 
+    Set#IsMember(s, bx)
+       <==> Set#IsMember($Unbox(read(newHeap, this, NW)): Set, bx)
          || (
           $Unbox(bx) != null
-           && !read(prevHeap, $Unbox(bx): ref, alloc)
-           && read(newHeap, $Unbox(bx): ref, alloc)));
+           && !$Unbox(read(prevHeap, $Unbox(bx): ref, alloc))
+           && $Unbox(read(newHeap, $Unbox(bx): ref, alloc))));
 
 
 
-type Set T = [T]bool;
+type Set;
 
-function Set#Card<T>(Set T) : int;
+revealed function Set#Card(s: Set) : int;
 
-axiom (forall<T> s: Set T :: { Set#Card(s) } 0 <= Set#Card(s));
+axiom (forall s: Set :: { Set#Card(s) } 0 <= Set#Card(s));
 
-function Set#Empty<T>() : Set T;
+revealed function Set#Empty() : Set;
 
-axiom (forall<T> o: T :: { Set#Empty()[o] } !Set#Empty()[o]);
+revealed function Set#IsMember(s: Set, o: Box) : bool;
 
-axiom (forall<T> s: Set T :: 
+axiom (forall o: Box :: 
+  { Set#IsMember(Set#Empty(), o) } 
+  !Set#IsMember(Set#Empty(), o));
+
+axiom (forall s: Set :: 
   { Set#Card(s) } 
   (Set#Card(s) == 0 <==> s == Set#Empty())
-     && (Set#Card(s) != 0 ==> (exists x: T :: s[x])));
+     && (Set#Card(s) != 0
+       ==> (exists x: Box :: { Set#IsMember(s, x) } Set#IsMember(s, x))));
 
-function Set#Singleton<T>(T) : Set T;
+revealed function Set#UnionOne(s: Set, o: Box) : Set;
 
-axiom (forall<T> r: T :: { Set#Singleton(r) } Set#Singleton(r)[r]);
+axiom (forall a: Set, x: Box, o: Box :: 
+  { Set#IsMember(Set#UnionOne(a, x), o) } 
+  Set#IsMember(Set#UnionOne(a, x), o) <==> o == x || Set#IsMember(a, o));
 
-axiom (forall<T> r: T, o: T :: 
-  { Set#Singleton(r)[o] } 
-  Set#Singleton(r)[o] <==> r == o);
+axiom (forall a: Set, x: Box :: 
+  { Set#UnionOne(a, x) } 
+  Set#IsMember(Set#UnionOne(a, x), x));
 
-axiom (forall<T> r: T :: 
-  { Set#Card(Set#Singleton(r)) } 
-  Set#Card(Set#Singleton(r)) == 1);
+axiom (forall a: Set, x: Box, y: Box :: 
+  { Set#UnionOne(a, x), Set#IsMember(a, y) } 
+  Set#IsMember(a, y) ==> Set#IsMember(Set#UnionOne(a, x), y));
 
-function Set#UnionOne<T>(Set T, T) : Set T;
-
-axiom (forall<T> a: Set T, x: T, o: T :: 
-  { Set#UnionOne(a, x)[o] } 
-  Set#UnionOne(a, x)[o] <==> o == x || a[o]);
-
-axiom (forall<T> a: Set T, x: T :: { Set#UnionOne(a, x) } Set#UnionOne(a, x)[x]);
-
-axiom (forall<T> a: Set T, x: T, y: T :: 
-  { Set#UnionOne(a, x), a[y] } 
-  a[y] ==> Set#UnionOne(a, x)[y]);
-
-axiom (forall<T> a: Set T, x: T :: 
+axiom (forall a: Set, x: Box :: 
   { Set#Card(Set#UnionOne(a, x)) } 
-  a[x] ==> Set#Card(Set#UnionOne(a, x)) == Set#Card(a));
+  Set#IsMember(a, x) ==> Set#Card(Set#UnionOne(a, x)) == Set#Card(a));
 
-axiom (forall<T> a: Set T, x: T :: 
+axiom (forall a: Set, x: Box :: 
   { Set#Card(Set#UnionOne(a, x)) } 
-  !a[x] ==> Set#Card(Set#UnionOne(a, x)) == Set#Card(a) + 1);
+  !Set#IsMember(a, x) ==> Set#Card(Set#UnionOne(a, x)) == Set#Card(a) + 1);
 
-function Set#Union<T>(Set T, Set T) : Set T;
+revealed function Set#Union(a: Set, b: Set) : Set;
 
-axiom (forall<T> a: Set T, b: Set T, o: T :: 
-  { Set#Union(a, b)[o] } 
-  Set#Union(a, b)[o] <==> a[o] || b[o]);
+axiom (forall a: Set, b: Set, o: Box :: 
+  { Set#IsMember(Set#Union(a, b), o) } 
+  Set#IsMember(Set#Union(a, b), o) <==> Set#IsMember(a, o) || Set#IsMember(b, o));
 
-axiom (forall<T> a: Set T, b: Set T, y: T :: 
-  { Set#Union(a, b), a[y] } 
-  a[y] ==> Set#Union(a, b)[y]);
+axiom (forall a: Set, b: Set, y: Box :: 
+  { Set#Union(a, b), Set#IsMember(a, y) } 
+  Set#IsMember(a, y) ==> Set#IsMember(Set#Union(a, b), y));
 
-axiom (forall<T> a: Set T, b: Set T, y: T :: 
-  { Set#Union(a, b), b[y] } 
-  b[y] ==> Set#Union(a, b)[y]);
+axiom (forall a: Set, b: Set, y: Box :: 
+  { Set#Union(a, b), Set#IsMember(b, y) } 
+  Set#IsMember(b, y) ==> Set#IsMember(Set#Union(a, b), y));
 
-axiom (forall<T> a: Set T, b: Set T :: 
+axiom (forall a: Set, b: Set :: 
   { Set#Union(a, b) } 
   Set#Disjoint(a, b)
      ==> Set#Difference(Set#Union(a, b), a) == b
        && Set#Difference(Set#Union(a, b), b) == a);
 
-function Set#Intersection<T>(Set T, Set T) : Set T;
+revealed function Set#Intersection(a: Set, b: Set) : Set;
 
-axiom (forall<T> a: Set T, b: Set T, o: T :: 
-  { Set#Intersection(a, b)[o] } 
-  Set#Intersection(a, b)[o] <==> a[o] && b[o]);
+axiom (forall a: Set, b: Set, o: Box :: 
+  { Set#IsMember(Set#Intersection(a, b), o) } 
+  Set#IsMember(Set#Intersection(a, b), o)
+     <==> Set#IsMember(a, o) && Set#IsMember(b, o));
 
-axiom (forall<T> a: Set T, b: Set T :: 
+axiom (forall a: Set, b: Set :: 
   { Set#Union(Set#Union(a, b), b) } 
   Set#Union(Set#Union(a, b), b) == Set#Union(a, b));
 
-axiom (forall<T> a: Set T, b: Set T :: 
+axiom (forall a: Set, b: Set :: 
   { Set#Union(a, Set#Union(a, b)) } 
   Set#Union(a, Set#Union(a, b)) == Set#Union(a, b));
 
-axiom (forall<T> a: Set T, b: Set T :: 
+axiom (forall a: Set, b: Set :: 
   { Set#Intersection(Set#Intersection(a, b), b) } 
   Set#Intersection(Set#Intersection(a, b), b) == Set#Intersection(a, b));
 
-axiom (forall<T> a: Set T, b: Set T :: 
+axiom (forall a: Set, b: Set :: 
   { Set#Intersection(a, Set#Intersection(a, b)) } 
   Set#Intersection(a, Set#Intersection(a, b)) == Set#Intersection(a, b));
 
-axiom (forall<T> a: Set T, b: Set T :: 
+axiom (forall a: Set, b: Set :: 
   { Set#Card(Set#Union(a, b)) } { Set#Card(Set#Intersection(a, b)) } 
   Set#Card(Set#Union(a, b)) + Set#Card(Set#Intersection(a, b))
      == Set#Card(a) + Set#Card(b));
 
-function Set#Difference<T>(Set T, Set T) : Set T;
+revealed function Set#Difference(a: Set, b: Set) : Set;
 
-axiom (forall<T> a: Set T, b: Set T, o: T :: 
-  { Set#Difference(a, b)[o] } 
-  Set#Difference(a, b)[o] <==> a[o] && !b[o]);
+axiom (forall a: Set, b: Set, o: Box :: 
+  { Set#IsMember(Set#Difference(a, b), o) } 
+  Set#IsMember(Set#Difference(a, b), o)
+     <==> Set#IsMember(a, o) && !Set#IsMember(b, o));
 
-axiom (forall<T> a: Set T, b: Set T, y: T :: 
-  { Set#Difference(a, b), b[y] } 
-  b[y] ==> !Set#Difference(a, b)[y]);
+axiom (forall a: Set, b: Set, y: Box :: 
+  { Set#Difference(a, b), Set#IsMember(b, y) } 
+  Set#IsMember(b, y) ==> !Set#IsMember(Set#Difference(a, b), y));
 
-axiom (forall<T> a: Set T, b: Set T :: 
+axiom (forall a: Set, b: Set :: 
   { Set#Card(Set#Difference(a, b)) } 
   Set#Card(Set#Difference(a, b))
          + Set#Card(Set#Difference(b, a))
@@ -826,119 +919,138 @@ axiom (forall<T> a: Set T, b: Set T ::
        == Set#Card(Set#Union(a, b))
      && Set#Card(Set#Difference(a, b)) == Set#Card(a) - Set#Card(Set#Intersection(a, b)));
 
-function Set#Subset<T>(Set T, Set T) : bool;
+revealed function Set#Subset(a: Set, b: Set) : bool;
 
-axiom (forall<T> a: Set T, b: Set T :: 
+axiom (forall a: Set, b: Set :: 
   { Set#Subset(a, b) } 
-  Set#Subset(a, b) <==> (forall o: T :: { a[o] } { b[o] } a[o] ==> b[o]));
+  Set#Subset(a, b)
+     <==> (forall o: Box :: 
+      { Set#IsMember(a, o) } { Set#IsMember(b, o) } 
+      Set#IsMember(a, o) ==> Set#IsMember(b, o)));
 
-function Set#Equal<T>(Set T, Set T) : bool;
+revealed function Set#Equal(a: Set, b: Set) : bool;
 
-axiom (forall<T> a: Set T, b: Set T :: 
+axiom (forall a: Set, b: Set :: 
   { Set#Equal(a, b) } 
-  Set#Equal(a, b) <==> (forall o: T :: { a[o] } { b[o] } a[o] <==> b[o]));
+  Set#Equal(a, b)
+     <==> (forall o: Box :: 
+      { Set#IsMember(a, o) } { Set#IsMember(b, o) } 
+      Set#IsMember(a, o) <==> Set#IsMember(b, o)));
 
-axiom (forall<T> a: Set T, b: Set T :: { Set#Equal(a, b) } Set#Equal(a, b) ==> a == b);
+axiom (forall a: Set, b: Set :: { Set#Equal(a, b) } Set#Equal(a, b) ==> a == b);
 
-function Set#Disjoint<T>(Set T, Set T) : bool;
+revealed function Set#Disjoint(a: Set, b: Set) : bool;
 
-axiom (forall<T> a: Set T, b: Set T :: 
+axiom (forall a: Set, b: Set :: 
   { Set#Disjoint(a, b) } 
-  Set#Disjoint(a, b) <==> (forall o: T :: { a[o] } { b[o] } !a[o] || !b[o]));
+  Set#Disjoint(a, b)
+     <==> (forall o: Box :: 
+      { Set#IsMember(a, o) } { Set#IsMember(b, o) } 
+      !Set#IsMember(a, o) || !Set#IsMember(b, o)));
 
-type ISet T = [T]bool;
+revealed function Set#FromBoogieMap([Box]bool) : Set;
 
-function ISet#Empty<T>() : Set T;
+axiom (forall m: [Box]bool, bx: Box :: 
+  { Set#IsMember(Set#FromBoogieMap(m), bx) } 
+  Set#IsMember(Set#FromBoogieMap(m), bx) == m[bx]);
 
-axiom (forall<T> o: T :: { ISet#Empty()[o] } !ISet#Empty()[o]);
+type ISet = [Box]bool;
 
-function ISet#UnionOne<T>(ISet T, T) : ISet T;
+revealed function ISet#Empty() : ISet;
 
-axiom (forall<T> a: ISet T, x: T, o: T :: 
+axiom (forall o: Box :: { ISet#Empty()[o] } !ISet#Empty()[o]);
+
+revealed function ISet#FromSet(Set) : ISet;
+
+axiom (forall s: Set, bx: Box :: 
+  { ISet#FromSet(s)[bx] } 
+  ISet#FromSet(s)[bx] == Set#IsMember(s, bx));
+
+revealed function ISet#UnionOne(ISet, Box) : ISet;
+
+axiom (forall a: ISet, x: Box, o: Box :: 
   { ISet#UnionOne(a, x)[o] } 
   ISet#UnionOne(a, x)[o] <==> o == x || a[o]);
 
-axiom (forall<T> a: ISet T, x: T :: { ISet#UnionOne(a, x) } ISet#UnionOne(a, x)[x]);
+axiom (forall a: ISet, x: Box :: { ISet#UnionOne(a, x) } ISet#UnionOne(a, x)[x]);
 
-axiom (forall<T> a: ISet T, x: T, y: T :: 
+axiom (forall a: ISet, x: Box, y: Box :: 
   { ISet#UnionOne(a, x), a[y] } 
   a[y] ==> ISet#UnionOne(a, x)[y]);
 
-function ISet#Union<T>(ISet T, ISet T) : ISet T;
+revealed function ISet#Union(ISet, ISet) : ISet;
 
-axiom (forall<T> a: ISet T, b: ISet T, o: T :: 
+axiom (forall a: ISet, b: ISet, o: Box :: 
   { ISet#Union(a, b)[o] } 
   ISet#Union(a, b)[o] <==> a[o] || b[o]);
 
-axiom (forall<T> a: ISet T, b: ISet T, y: T :: 
+axiom (forall a: ISet, b: ISet, y: Box :: 
   { ISet#Union(a, b), a[y] } 
   a[y] ==> ISet#Union(a, b)[y]);
 
-axiom (forall<T> a: Set T, b: Set T, y: T :: 
+axiom (forall a: ISet, b: ISet, y: Box :: 
   { ISet#Union(a, b), b[y] } 
   b[y] ==> ISet#Union(a, b)[y]);
 
-axiom (forall<T> a: ISet T, b: ISet T :: 
+axiom (forall a: ISet, b: ISet :: 
   { ISet#Union(a, b) } 
   ISet#Disjoint(a, b)
      ==> ISet#Difference(ISet#Union(a, b), a) == b
        && ISet#Difference(ISet#Union(a, b), b) == a);
 
-function ISet#Intersection<T>(ISet T, ISet T) : ISet T;
+revealed function ISet#Intersection(ISet, ISet) : ISet;
 
-axiom (forall<T> a: ISet T, b: ISet T, o: T :: 
+axiom (forall a: ISet, b: ISet, o: Box :: 
   { ISet#Intersection(a, b)[o] } 
   ISet#Intersection(a, b)[o] <==> a[o] && b[o]);
 
-axiom (forall<T> a: ISet T, b: ISet T :: 
+axiom (forall a: ISet, b: ISet :: 
   { ISet#Union(ISet#Union(a, b), b) } 
   ISet#Union(ISet#Union(a, b), b) == ISet#Union(a, b));
 
-axiom (forall<T> a: Set T, b: Set T :: 
+axiom (forall a: ISet, b: ISet :: 
   { ISet#Union(a, ISet#Union(a, b)) } 
   ISet#Union(a, ISet#Union(a, b)) == ISet#Union(a, b));
 
-axiom (forall<T> a: ISet T, b: ISet T :: 
+axiom (forall a: ISet, b: ISet :: 
   { ISet#Intersection(ISet#Intersection(a, b), b) } 
   ISet#Intersection(ISet#Intersection(a, b), b) == ISet#Intersection(a, b));
 
-axiom (forall<T> a: ISet T, b: ISet T :: 
+axiom (forall a: ISet, b: ISet :: 
   { ISet#Intersection(a, ISet#Intersection(a, b)) } 
   ISet#Intersection(a, ISet#Intersection(a, b)) == ISet#Intersection(a, b));
 
-function ISet#Difference<T>(ISet T, ISet T) : ISet T;
+revealed function ISet#Difference(ISet, ISet) : ISet;
 
-axiom (forall<T> a: ISet T, b: ISet T, o: T :: 
+axiom (forall a: ISet, b: ISet, o: Box :: 
   { ISet#Difference(a, b)[o] } 
   ISet#Difference(a, b)[o] <==> a[o] && !b[o]);
 
-axiom (forall<T> a: ISet T, b: ISet T, y: T :: 
+axiom (forall a: ISet, b: ISet, y: Box :: 
   { ISet#Difference(a, b), b[y] } 
   b[y] ==> !ISet#Difference(a, b)[y]);
 
-function ISet#Subset<T>(ISet T, ISet T) : bool;
+revealed function ISet#Subset(ISet, ISet) : bool;
 
-axiom (forall<T> a: ISet T, b: ISet T :: 
+axiom (forall a: ISet, b: ISet :: 
   { ISet#Subset(a, b) } 
-  ISet#Subset(a, b) <==> (forall o: T :: { a[o] } { b[o] } a[o] ==> b[o]));
+  ISet#Subset(a, b) <==> (forall o: Box :: { a[o] } { b[o] } a[o] ==> b[o]));
 
-function ISet#Equal<T>(ISet T, ISet T) : bool;
+revealed function ISet#Equal(ISet, ISet) : bool;
 
-axiom (forall<T> a: ISet T, b: ISet T :: 
+axiom (forall a: ISet, b: ISet :: 
   { ISet#Equal(a, b) } 
-  ISet#Equal(a, b) <==> (forall o: T :: { a[o] } { b[o] } a[o] <==> b[o]));
+  ISet#Equal(a, b) <==> (forall o: Box :: { a[o] } { b[o] } a[o] <==> b[o]));
 
-axiom (forall<T> a: ISet T, b: ISet T :: 
-  { ISet#Equal(a, b) } 
-  ISet#Equal(a, b) ==> a == b);
+axiom (forall a: ISet, b: ISet :: { ISet#Equal(a, b) } ISet#Equal(a, b) ==> a == b);
 
-function ISet#Disjoint<T>(ISet T, ISet T) : bool;
+revealed function ISet#Disjoint(ISet, ISet) : bool;
 
-axiom (forall<T> a: ISet T, b: ISet T :: 
+axiom (forall a: ISet, b: ISet :: 
   { ISet#Disjoint(a, b) } 
-  ISet#Disjoint(a, b) <==> (forall o: T :: { a[o] } { b[o] } !a[o] || !b[o]));
+  ISet#Disjoint(a, b) <==> (forall o: Box :: { a[o] } { b[o] } !a[o] || !b[o]));
 
-function Math#min(a: int, b: int) : int;
+revealed function Math#min(a: int, b: int) : int;
 
 axiom (forall a: int, b: int :: { Math#min(a, b) } a <= b <==> Math#min(a, b) == a);
 
@@ -948,108 +1060,138 @@ axiom (forall a: int, b: int ::
   { Math#min(a, b) } 
   Math#min(a, b) == a || Math#min(a, b) == b);
 
-function Math#clip(a: int) : int;
+revealed function Math#clip(a: int) : int;
 
 axiom (forall a: int :: { Math#clip(a) } 0 <= a ==> Math#clip(a) == a);
 
 axiom (forall a: int :: { Math#clip(a) } a < 0 ==> Math#clip(a) == 0);
 
-type MultiSet T = [T]int;
+type MultiSet;
 
-function $IsGoodMultiSet<T>(ms: MultiSet T) : bool;
+revealed function MultiSet#Multiplicity(m: MultiSet, o: Box) : int;
 
-axiom (forall<T> ms: MultiSet T :: 
+revealed function MultiSet#UpdateMultiplicity(m: MultiSet, o: Box, n: int) : MultiSet;
+
+axiom (forall m: MultiSet, o: Box, n: int, p: Box :: 
+  { MultiSet#Multiplicity(MultiSet#UpdateMultiplicity(m, o, n), p) } 
+  0 <= n
+     ==> (o == p ==> MultiSet#Multiplicity(MultiSet#UpdateMultiplicity(m, o, n), p) == n)
+       && (o != p
+         ==> MultiSet#Multiplicity(MultiSet#UpdateMultiplicity(m, o, n), p)
+           == MultiSet#Multiplicity(m, p)));
+
+revealed function $IsGoodMultiSet(ms: MultiSet) : bool;
+
+axiom (forall ms: MultiSet :: 
   { $IsGoodMultiSet(ms) } 
   $IsGoodMultiSet(ms)
-     <==> (forall bx: T :: { ms[bx] } 0 <= ms[bx] && ms[bx] <= MultiSet#Card(ms)));
+     <==> (forall bx: Box :: 
+      { MultiSet#Multiplicity(ms, bx) } 
+      0 <= MultiSet#Multiplicity(ms, bx)
+         && MultiSet#Multiplicity(ms, bx) <= MultiSet#Card(ms)));
 
-function MultiSet#Card<T>(MultiSet T) : int;
+revealed function MultiSet#Card(m: MultiSet) : int;
 
-axiom (forall<T> s: MultiSet T :: { MultiSet#Card(s) } 0 <= MultiSet#Card(s));
+axiom (forall s: MultiSet :: { MultiSet#Card(s) } 0 <= MultiSet#Card(s));
 
-axiom (forall<T> s: MultiSet T, x: T, n: int :: 
-  { MultiSet#Card(s[x := n]) } 
-  0 <= n ==> MultiSet#Card(s[x := n]) == MultiSet#Card(s) - s[x] + n);
+axiom (forall s: MultiSet, x: Box, n: int :: 
+  { MultiSet#Card(MultiSet#UpdateMultiplicity(s, x, n)) } 
+  0 <= n
+     ==> MultiSet#Card(MultiSet#UpdateMultiplicity(s, x, n))
+       == MultiSet#Card(s) - MultiSet#Multiplicity(s, x) + n);
 
-function MultiSet#Empty<T>() : MultiSet T;
+revealed function MultiSet#Empty() : MultiSet;
 
-axiom (forall<T> o: T :: { MultiSet#Empty()[o] } MultiSet#Empty()[o] == 0);
+axiom (forall o: Box :: 
+  { MultiSet#Multiplicity(MultiSet#Empty(), o) } 
+  MultiSet#Multiplicity(MultiSet#Empty(), o) == 0);
 
-axiom (forall<T> s: MultiSet T :: 
+axiom (forall s: MultiSet :: 
   { MultiSet#Card(s) } 
   (MultiSet#Card(s) == 0 <==> s == MultiSet#Empty())
-     && (MultiSet#Card(s) != 0 ==> (exists x: T :: 0 < s[x])));
+     && (MultiSet#Card(s) != 0
+       ==> (exists x: Box :: 
+        { MultiSet#Multiplicity(s, x) } 
+        0 < MultiSet#Multiplicity(s, x))));
 
-function MultiSet#Singleton<T>(T) : MultiSet T;
+revealed function MultiSet#Singleton(o: Box) : MultiSet;
 
-axiom (forall<T> r: T, o: T :: 
-  { MultiSet#Singleton(r)[o] } 
-  (MultiSet#Singleton(r)[o] == 1 <==> r == o)
-     && (MultiSet#Singleton(r)[o] == 0 <==> r != o));
+axiom (forall r: Box, o: Box :: 
+  { MultiSet#Multiplicity(MultiSet#Singleton(r), o) } 
+  (MultiSet#Multiplicity(MultiSet#Singleton(r), o) == 1 <==> r == o)
+     && (MultiSet#Multiplicity(MultiSet#Singleton(r), o) == 0 <==> r != o));
 
-axiom (forall<T> r: T :: 
+axiom (forall r: Box :: 
   { MultiSet#Singleton(r) } 
   MultiSet#Singleton(r) == MultiSet#UnionOne(MultiSet#Empty(), r));
 
-function MultiSet#UnionOne<T>(MultiSet T, T) : MultiSet T;
+revealed function MultiSet#UnionOne(m: MultiSet, o: Box) : MultiSet;
 
-axiom (forall<T> a: MultiSet T, x: T, o: T :: 
-  { MultiSet#UnionOne(a, x)[o] } 
-  0 < MultiSet#UnionOne(a, x)[o] <==> o == x || 0 < a[o]);
+axiom (forall a: MultiSet, x: Box, o: Box :: 
+  { MultiSet#Multiplicity(MultiSet#UnionOne(a, x), o) } 
+  0 < MultiSet#Multiplicity(MultiSet#UnionOne(a, x), o)
+     <==> o == x || 0 < MultiSet#Multiplicity(a, o));
 
-axiom (forall<T> a: MultiSet T, x: T :: 
+axiom (forall a: MultiSet, x: Box :: 
   { MultiSet#UnionOne(a, x) } 
-  MultiSet#UnionOne(a, x)[x] == a[x] + 1);
+  MultiSet#Multiplicity(MultiSet#UnionOne(a, x), x)
+     == MultiSet#Multiplicity(a, x) + 1);
 
-axiom (forall<T> a: MultiSet T, x: T, y: T :: 
-  { MultiSet#UnionOne(a, x), a[y] } 
-  0 < a[y] ==> 0 < MultiSet#UnionOne(a, x)[y]);
+axiom (forall a: MultiSet, x: Box, y: Box :: 
+  { MultiSet#UnionOne(a, x), MultiSet#Multiplicity(a, y) } 
+  0 < MultiSet#Multiplicity(a, y)
+     ==> 0 < MultiSet#Multiplicity(MultiSet#UnionOne(a, x), y));
 
-axiom (forall<T> a: MultiSet T, x: T, y: T :: 
-  { MultiSet#UnionOne(a, x), a[y] } 
-  x != y ==> a[y] == MultiSet#UnionOne(a, x)[y]);
+axiom (forall a: MultiSet, x: Box, y: Box :: 
+  { MultiSet#UnionOne(a, x), MultiSet#Multiplicity(a, y) } 
+  x != y
+     ==> MultiSet#Multiplicity(a, y) == MultiSet#Multiplicity(MultiSet#UnionOne(a, x), y));
 
-axiom (forall<T> a: MultiSet T, x: T :: 
+axiom (forall a: MultiSet, x: Box :: 
   { MultiSet#Card(MultiSet#UnionOne(a, x)) } 
   MultiSet#Card(MultiSet#UnionOne(a, x)) == MultiSet#Card(a) + 1);
 
-function MultiSet#Union<T>(MultiSet T, MultiSet T) : MultiSet T;
+revealed function MultiSet#Union(a: MultiSet, b: MultiSet) : MultiSet;
 
-axiom (forall<T> a: MultiSet T, b: MultiSet T, o: T :: 
-  { MultiSet#Union(a, b)[o] } 
-  MultiSet#Union(a, b)[o] == a[o] + b[o]);
+axiom (forall a: MultiSet, b: MultiSet, o: Box :: 
+  { MultiSet#Multiplicity(MultiSet#Union(a, b), o) } 
+  MultiSet#Multiplicity(MultiSet#Union(a, b), o)
+     == MultiSet#Multiplicity(a, o) + MultiSet#Multiplicity(b, o));
 
-axiom (forall<T> a: MultiSet T, b: MultiSet T :: 
+axiom (forall a: MultiSet, b: MultiSet :: 
   { MultiSet#Card(MultiSet#Union(a, b)) } 
   MultiSet#Card(MultiSet#Union(a, b)) == MultiSet#Card(a) + MultiSet#Card(b));
 
-function MultiSet#Intersection<T>(MultiSet T, MultiSet T) : MultiSet T;
+revealed function MultiSet#Intersection(a: MultiSet, b: MultiSet) : MultiSet;
 
-axiom (forall<T> a: MultiSet T, b: MultiSet T, o: T :: 
-  { MultiSet#Intersection(a, b)[o] } 
-  MultiSet#Intersection(a, b)[o] == Math#min(a[o], b[o]));
+axiom (forall a: MultiSet, b: MultiSet, o: Box :: 
+  { MultiSet#Multiplicity(MultiSet#Intersection(a, b), o) } 
+  MultiSet#Multiplicity(MultiSet#Intersection(a, b), o)
+     == Math#min(MultiSet#Multiplicity(a, o), MultiSet#Multiplicity(b, o)));
 
-axiom (forall<T> a: MultiSet T, b: MultiSet T :: 
+axiom (forall a: MultiSet, b: MultiSet :: 
   { MultiSet#Intersection(MultiSet#Intersection(a, b), b) } 
   MultiSet#Intersection(MultiSet#Intersection(a, b), b)
      == MultiSet#Intersection(a, b));
 
-axiom (forall<T> a: MultiSet T, b: MultiSet T :: 
+axiom (forall a: MultiSet, b: MultiSet :: 
   { MultiSet#Intersection(a, MultiSet#Intersection(a, b)) } 
   MultiSet#Intersection(a, MultiSet#Intersection(a, b))
      == MultiSet#Intersection(a, b));
 
-function MultiSet#Difference<T>(MultiSet T, MultiSet T) : MultiSet T;
+revealed function MultiSet#Difference(a: MultiSet, b: MultiSet) : MultiSet;
 
-axiom (forall<T> a: MultiSet T, b: MultiSet T, o: T :: 
-  { MultiSet#Difference(a, b)[o] } 
-  MultiSet#Difference(a, b)[o] == Math#clip(a[o] - b[o]));
+axiom (forall a: MultiSet, b: MultiSet, o: Box :: 
+  { MultiSet#Multiplicity(MultiSet#Difference(a, b), o) } 
+  MultiSet#Multiplicity(MultiSet#Difference(a, b), o)
+     == Math#clip(MultiSet#Multiplicity(a, o) - MultiSet#Multiplicity(b, o)));
 
-axiom (forall<T> a: MultiSet T, b: MultiSet T, y: T :: 
-  { MultiSet#Difference(a, b), b[y], a[y] } 
-  a[y] <= b[y] ==> MultiSet#Difference(a, b)[y] == 0);
+axiom (forall a: MultiSet, b: MultiSet, y: Box :: 
+  { MultiSet#Difference(a, b), MultiSet#Multiplicity(b, y), MultiSet#Multiplicity(a, y) } 
+  MultiSet#Multiplicity(a, y) <= MultiSet#Multiplicity(b, y)
+     ==> MultiSet#Multiplicity(MultiSet#Difference(a, b), y) == 0);
 
-axiom (forall<T> a: MultiSet T, b: MultiSet T :: 
+axiom (forall a: MultiSet, b: MultiSet :: 
   { MultiSet#Card(MultiSet#Difference(a, b)) } 
   MultiSet#Card(MultiSet#Difference(a, b))
          + MultiSet#Card(MultiSet#Difference(b, a))
@@ -1058,195 +1200,181 @@ axiom (forall<T> a: MultiSet T, b: MultiSet T ::
      && MultiSet#Card(MultiSet#Difference(a, b))
        == MultiSet#Card(a) - MultiSet#Card(MultiSet#Intersection(a, b)));
 
-function MultiSet#Subset<T>(MultiSet T, MultiSet T) : bool;
+revealed function MultiSet#Subset(a: MultiSet, b: MultiSet) : bool;
 
-axiom (forall<T> a: MultiSet T, b: MultiSet T :: 
+axiom (forall a: MultiSet, b: MultiSet :: 
   { MultiSet#Subset(a, b) } 
-  MultiSet#Subset(a, b) <==> (forall o: T :: { a[o] } { b[o] } a[o] <= b[o]));
+  MultiSet#Subset(a, b)
+     <==> (forall o: Box :: 
+      { MultiSet#Multiplicity(a, o) } { MultiSet#Multiplicity(b, o) } 
+      MultiSet#Multiplicity(a, o) <= MultiSet#Multiplicity(b, o)));
 
-function MultiSet#Equal<T>(MultiSet T, MultiSet T) : bool;
+revealed function MultiSet#Equal(a: MultiSet, b: MultiSet) : bool;
 
-axiom (forall<T> a: MultiSet T, b: MultiSet T :: 
+axiom (forall a: MultiSet, b: MultiSet :: 
   { MultiSet#Equal(a, b) } 
-  MultiSet#Equal(a, b) <==> (forall o: T :: { a[o] } { b[o] } a[o] == b[o]));
+  MultiSet#Equal(a, b)
+     <==> (forall o: Box :: 
+      { MultiSet#Multiplicity(a, o) } { MultiSet#Multiplicity(b, o) } 
+      MultiSet#Multiplicity(a, o) == MultiSet#Multiplicity(b, o)));
 
-axiom (forall<T> a: MultiSet T, b: MultiSet T :: 
+axiom (forall a: MultiSet, b: MultiSet :: 
   { MultiSet#Equal(a, b) } 
   MultiSet#Equal(a, b) ==> a == b);
 
-function MultiSet#Disjoint<T>(MultiSet T, MultiSet T) : bool;
+revealed function MultiSet#Disjoint(a: MultiSet, b: MultiSet) : bool;
 
-axiom (forall<T> a: MultiSet T, b: MultiSet T :: 
+axiom (forall a: MultiSet, b: MultiSet :: 
   { MultiSet#Disjoint(a, b) } 
   MultiSet#Disjoint(a, b)
-     <==> (forall o: T :: { a[o] } { b[o] } a[o] == 0 || b[o] == 0));
+     <==> (forall o: Box :: 
+      { MultiSet#Multiplicity(a, o) } { MultiSet#Multiplicity(b, o) } 
+      MultiSet#Multiplicity(a, o) == 0 || MultiSet#Multiplicity(b, o) == 0));
 
-function MultiSet#FromSet<T>(Set T) : MultiSet T;
+revealed function MultiSet#FromSet(s: Set) : MultiSet;
 
-axiom (forall<T> s: Set T, a: T :: 
-  { MultiSet#FromSet(s)[a] } 
-  (MultiSet#FromSet(s)[a] == 0 <==> !s[a])
-     && (MultiSet#FromSet(s)[a] == 1 <==> s[a]));
+axiom (forall s: Set, a: Box :: 
+  { MultiSet#Multiplicity(MultiSet#FromSet(s), a) } 
+  (MultiSet#Multiplicity(MultiSet#FromSet(s), a) == 0 <==> !Set#IsMember(s, a))
+     && (MultiSet#Multiplicity(MultiSet#FromSet(s), a) == 1 <==> Set#IsMember(s, a)));
 
-axiom (forall<T> s: Set T :: 
+axiom (forall s: Set :: 
   { MultiSet#Card(MultiSet#FromSet(s)) } 
   MultiSet#Card(MultiSet#FromSet(s)) == Set#Card(s));
 
-function MultiSet#FromSeq<T>(Seq T) : MultiSet T;
+revealed function MultiSet#FromSeq(s: Seq) : MultiSet
+uses {
+axiom MultiSet#FromSeq(Seq#Empty()) == MultiSet#Empty();
+}
 
-axiom (forall<T> s: Seq T :: 
-  { MultiSet#FromSeq(s) } 
-  $IsGoodMultiSet(MultiSet#FromSeq(s)));
+axiom (forall s: Seq :: { MultiSet#FromSeq(s) } $IsGoodMultiSet(MultiSet#FromSeq(s)));
 
-axiom (forall<T> s: Seq T :: 
+axiom (forall s: Seq :: 
   { MultiSet#Card(MultiSet#FromSeq(s)) } 
   MultiSet#Card(MultiSet#FromSeq(s)) == Seq#Length(s));
 
-axiom (forall<T> s: Seq T, v: T :: 
+axiom (forall s: Seq, v: Box :: 
   { MultiSet#FromSeq(Seq#Build(s, v)) } 
   MultiSet#FromSeq(Seq#Build(s, v)) == MultiSet#UnionOne(MultiSet#FromSeq(s), v));
 
-axiom (forall<T>  :: 
-  MultiSet#FromSeq(Seq#Empty(): Seq T) == MultiSet#Empty(): MultiSet T);
-
-axiom (forall<T> a: Seq T, b: Seq T :: 
+axiom (forall a: Seq, b: Seq :: 
   { MultiSet#FromSeq(Seq#Append(a, b)) } 
   MultiSet#FromSeq(Seq#Append(a, b))
      == MultiSet#Union(MultiSet#FromSeq(a), MultiSet#FromSeq(b)));
 
-axiom (forall<T> s: Seq T, i: int, v: T, x: T :: 
-  { MultiSet#FromSeq(Seq#Update(s, i, v))[x] } 
+axiom (forall s: Seq, i: int, v: Box, x: Box :: 
+  { MultiSet#Multiplicity(MultiSet#FromSeq(Seq#Update(s, i, v)), x) } 
   0 <= i && i < Seq#Length(s)
-     ==> MultiSet#FromSeq(Seq#Update(s, i, v))[x]
-       == MultiSet#Union(MultiSet#Difference(MultiSet#FromSeq(s), MultiSet#Singleton(Seq#Index(s, i))), 
-        MultiSet#Singleton(v))[x]);
+     ==> MultiSet#Multiplicity(MultiSet#FromSeq(Seq#Update(s, i, v)), x)
+       == MultiSet#Multiplicity(MultiSet#Union(MultiSet#Difference(MultiSet#FromSeq(s), MultiSet#Singleton(Seq#Index(s, i))), 
+          MultiSet#Singleton(v)), 
+        x));
 
-axiom (forall<T> s: Seq T, x: T :: 
-  { MultiSet#FromSeq(s)[x] } 
+axiom (forall s: Seq, x: Box :: 
+  { MultiSet#Multiplicity(MultiSet#FromSeq(s), x) } 
   (exists i: int :: 
       { Seq#Index(s, i) } 
       0 <= i && i < Seq#Length(s) && x == Seq#Index(s, i))
-     <==> 0 < MultiSet#FromSeq(s)[x]);
+     <==> 0 < MultiSet#Multiplicity(MultiSet#FromSeq(s), x));
 
-type Seq _;
+type Seq;
 
-function Seq#Length<T>(Seq T) : int;
+revealed function Seq#Length(s: Seq) : int;
 
-axiom (forall<T> s: Seq T :: { Seq#Length(s) } 0 <= Seq#Length(s));
+axiom (forall s: Seq :: { Seq#Length(s) } 0 <= Seq#Length(s));
 
-function Seq#Empty<T>() : Seq T;
+revealed function Seq#Empty() : Seq
+uses {
+axiom Seq#Length(Seq#Empty()) == 0;
+}
 
-axiom (forall<T>  :: { Seq#Empty(): Seq T } Seq#Length(Seq#Empty(): Seq T) == 0);
+axiom (forall s: Seq :: { Seq#Length(s) } Seq#Length(s) == 0 ==> s == Seq#Empty());
 
-axiom (forall<T> s: Seq T :: 
-  { Seq#Length(s) } 
-  Seq#Length(s) == 0 ==> s == Seq#Empty());
+revealed function Seq#Build(s: Seq, val: Box) : Seq;
 
-axiom (forall<T> t: Ty :: { $Is(Seq#Empty(): Seq T, t) } $Is(Seq#Empty(): Seq T, t));
+revealed function Seq#Build_inv0(s: Seq) : Seq;
 
-function Seq#Singleton<T>(T) : Seq T;
+revealed function Seq#Build_inv1(s: Seq) : Box;
 
-axiom (forall<T> t: T :: 
-  { Seq#Length(Seq#Singleton(t)) } 
-  Seq#Length(Seq#Singleton(t)) == 1);
-
-function Seq#Build<T>(s: Seq T, val: T) : Seq T;
-
-function Seq#Build_inv0<T>(s: Seq T) : Seq T;
-
-function Seq#Build_inv1<T>(s: Seq T) : T;
-
-axiom (forall<T> s: Seq T, val: T :: 
+axiom (forall s: Seq, val: Box :: 
   { Seq#Build(s, val) } 
   Seq#Build_inv0(Seq#Build(s, val)) == s
      && Seq#Build_inv1(Seq#Build(s, val)) == val);
 
-axiom (forall<T> s: Seq T, v: T :: 
+axiom (forall s: Seq, v: Box :: 
   { Seq#Build(s, v) } 
   Seq#Length(Seq#Build(s, v)) == 1 + Seq#Length(s));
 
-axiom (forall<T> s: Seq T, i: int, v: T :: 
+axiom (forall s: Seq, i: int, v: Box :: 
   { Seq#Index(Seq#Build(s, v), i) } 
   (i == Seq#Length(s) ==> Seq#Index(Seq#Build(s, v), i) == v)
      && (i != Seq#Length(s) ==> Seq#Index(Seq#Build(s, v), i) == Seq#Index(s, i)));
 
-axiom (forall s: Seq Box, bx: Box, t: Ty :: 
-  { $Is(Seq#Build(s, bx), TSeq(t)) } 
-  $Is(s, TSeq(t)) && $IsBox(bx, t) ==> $Is(Seq#Build(s, bx), TSeq(t)));
-
-function Seq#Append<T>(Seq T, Seq T) : Seq T;
-
-axiom (forall<T> s0: Seq T, s1: Seq T :: 
+axiom (forall s0: Seq, s1: Seq :: 
   { Seq#Length(Seq#Append(s0, s1)) } 
   Seq#Length(Seq#Append(s0, s1)) == Seq#Length(s0) + Seq#Length(s1));
 
-axiom (forall s0: Seq Box, s1: Seq Box, t: Ty :: 
-  { $Is(Seq#Append(s0, s1), t) } 
-  $Is(s0, t) && $Is(s1, t) ==> $Is(Seq#Append(s0, s1), t));
+revealed function Seq#Index(s: Seq, i: int) : Box;
 
-function Seq#Index<T>(Seq T, int) : T;
-
-axiom (forall<T> t: T :: 
-  { Seq#Index(Seq#Singleton(t), 0) } 
-  Seq#Index(Seq#Singleton(t), 0) == t);
-
-axiom (forall<T> s0: Seq T, s1: Seq T, n: int :: 
+axiom (forall s0: Seq, s1: Seq, n: int :: 
   { Seq#Index(Seq#Append(s0, s1), n) } 
   (n < Seq#Length(s0) ==> Seq#Index(Seq#Append(s0, s1), n) == Seq#Index(s0, n))
      && (Seq#Length(s0) <= n
        ==> Seq#Index(Seq#Append(s0, s1), n) == Seq#Index(s1, n - Seq#Length(s0))));
 
-function Seq#Update<T>(Seq T, int, T) : Seq T;
+revealed function Seq#Update(s: Seq, i: int, val: Box) : Seq;
 
-axiom (forall<T> s: Seq T, i: int, v: T :: 
+axiom (forall s: Seq, i: int, v: Box :: 
   { Seq#Length(Seq#Update(s, i, v)) } 
   0 <= i && i < Seq#Length(s) ==> Seq#Length(Seq#Update(s, i, v)) == Seq#Length(s));
 
-axiom (forall<T> s: Seq T, i: int, v: T, n: int :: 
+axiom (forall s: Seq, i: int, v: Box, n: int :: 
   { Seq#Index(Seq#Update(s, i, v), n) } 
   0 <= n && n < Seq#Length(s)
      ==> (i == n ==> Seq#Index(Seq#Update(s, i, v), n) == v)
        && (i != n ==> Seq#Index(Seq#Update(s, i, v), n) == Seq#Index(s, n)));
 
-function Seq#Contains<T>(Seq T, T) : bool;
+revealed function Seq#Append(s0: Seq, s1: Seq) : Seq;
 
-axiom (forall<T> s: Seq T, x: T :: 
+revealed function Seq#Contains(s: Seq, val: Box) : bool;
+
+axiom (forall s: Seq, x: Box :: 
   { Seq#Contains(s, x) } 
   Seq#Contains(s, x)
      <==> (exists i: int :: 
       { Seq#Index(s, i) } 
       0 <= i && i < Seq#Length(s) && Seq#Index(s, i) == x));
 
-axiom (forall<T> x: T :: 
+axiom (forall x: Box :: 
   { Seq#Contains(Seq#Empty(), x) } 
   !Seq#Contains(Seq#Empty(), x));
 
-axiom (forall<T> s0: Seq T, s1: Seq T, x: T :: 
+axiom (forall s0: Seq, s1: Seq, x: Box :: 
   { Seq#Contains(Seq#Append(s0, s1), x) } 
   Seq#Contains(Seq#Append(s0, s1), x)
      <==> Seq#Contains(s0, x) || Seq#Contains(s1, x));
 
-axiom (forall<T> s: Seq T, v: T, x: T :: 
+axiom (forall s: Seq, v: Box, x: Box :: 
   { Seq#Contains(Seq#Build(s, v), x) } 
   Seq#Contains(Seq#Build(s, v), x) <==> v == x || Seq#Contains(s, x));
 
-axiom (forall<T> s: Seq T, n: int, x: T :: 
+axiom (forall s: Seq, n: int, x: Box :: 
   { Seq#Contains(Seq#Take(s, n), x) } 
   Seq#Contains(Seq#Take(s, n), x)
      <==> (exists i: int :: 
       { Seq#Index(s, i) } 
       0 <= i && i < n && i < Seq#Length(s) && Seq#Index(s, i) == x));
 
-axiom (forall<T> s: Seq T, n: int, x: T :: 
+axiom (forall s: Seq, n: int, x: Box :: 
   { Seq#Contains(Seq#Drop(s, n), x) } 
   Seq#Contains(Seq#Drop(s, n), x)
      <==> (exists i: int :: 
       { Seq#Index(s, i) } 
       0 <= n && n <= i && i < Seq#Length(s) && Seq#Index(s, i) == x));
 
-function Seq#Equal<T>(Seq T, Seq T) : bool;
+revealed function Seq#Equal(s0: Seq, s1: Seq) : bool;
 
-axiom (forall<T> s0: Seq T, s1: Seq T :: 
+axiom (forall s0: Seq, s1: Seq :: 
   { Seq#Equal(s0, s1) } 
   Seq#Equal(s0, s1)
      <==> Seq#Length(s0) == Seq#Length(s1)
@@ -1254,50 +1382,103 @@ axiom (forall<T> s0: Seq T, s1: Seq T ::
         { Seq#Index(s0, j) } { Seq#Index(s1, j) } 
         0 <= j && j < Seq#Length(s0) ==> Seq#Index(s0, j) == Seq#Index(s1, j)));
 
-axiom (forall<T> a: Seq T, b: Seq T :: { Seq#Equal(a, b) } Seq#Equal(a, b) ==> a == b);
+axiom (forall a: Seq, b: Seq :: { Seq#Equal(a, b) } Seq#Equal(a, b) ==> a == b);
 
-function Seq#SameUntil<T>(Seq T, Seq T, int) : bool;
+revealed function Seq#SameUntil(s0: Seq, s1: Seq, n: int) : bool;
 
-axiom (forall<T> s0: Seq T, s1: Seq T, n: int :: 
+axiom (forall s0: Seq, s1: Seq, n: int :: 
   { Seq#SameUntil(s0, s1, n) } 
   Seq#SameUntil(s0, s1, n)
      <==> (forall j: int :: 
       { Seq#Index(s0, j) } { Seq#Index(s1, j) } 
       0 <= j && j < n ==> Seq#Index(s0, j) == Seq#Index(s1, j)));
 
-function Seq#Take<T>(s: Seq T, howMany: int) : Seq T;
+revealed function Seq#Take(s: Seq, howMany: int) : Seq;
 
-axiom (forall<T> s: Seq T, n: int :: 
+axiom (forall s: Seq, n: int :: 
   { Seq#Length(Seq#Take(s, n)) } 
   0 <= n && n <= Seq#Length(s) ==> Seq#Length(Seq#Take(s, n)) == n);
 
-axiom (forall<T> s: Seq T, n: int, j: int :: 
-  {:weight 25} { Seq#Index(Seq#Take(s, n), j) } { Seq#Index(s, j), Seq#Take(s, n) } 
+axiom (forall s: Seq, n: int, j: int :: 
+  {:weight 11} { Seq#Index(Seq#Take(s, n), j) } { Seq#Index(s, j), Seq#Take(s, n) } 
   0 <= j && j < n && j < Seq#Length(s)
      ==> Seq#Index(Seq#Take(s, n), j) == Seq#Index(s, j));
 
-function Seq#Drop<T>(s: Seq T, howMany: int) : Seq T;
+revealed function Seq#Drop(s: Seq, howMany: int) : Seq;
 
-axiom (forall<T> s: Seq T, n: int :: 
+axiom (forall s: Seq, n: int :: 
   { Seq#Length(Seq#Drop(s, n)) } 
   0 <= n && n <= Seq#Length(s) ==> Seq#Length(Seq#Drop(s, n)) == Seq#Length(s) - n);
 
-axiom (forall<T> s: Seq T, n: int, j: int :: 
-  {:weight 25} { Seq#Index(Seq#Drop(s, n), j) } 
+axiom (forall s: Seq, n: int, j: int :: 
+  {:weight 11} { Seq#Index(Seq#Drop(s, n), j) } 
   0 <= n && 0 <= j && j < Seq#Length(s) - n
      ==> Seq#Index(Seq#Drop(s, n), j) == Seq#Index(s, j + n));
 
-axiom (forall<T> s: Seq T, n: int, k: int :: 
-  {:weight 25} { Seq#Index(s, k), Seq#Drop(s, n) } 
+axiom (forall s: Seq, n: int, k: int :: 
+  {:weight 11} { Seq#Index(s, k), Seq#Drop(s, n) } 
   0 <= n && n <= k && k < Seq#Length(s)
      ==> Seq#Index(Seq#Drop(s, n), k - n) == Seq#Index(s, k));
 
-axiom (forall<T> s: Seq T, t: Seq T, n: int :: 
+axiom (forall s: Seq, t: Seq, n: int :: 
   { Seq#Take(Seq#Append(s, t), n) } { Seq#Drop(Seq#Append(s, t), n) } 
   n == Seq#Length(s)
      ==> Seq#Take(Seq#Append(s, t), n) == s && Seq#Drop(Seq#Append(s, t), n) == t);
 
-function Seq#FromArray(h: Heap, a: ref) : Seq Box;
+axiom (forall s: Seq, i: int, v: Box, n: int :: 
+  { Seq#Take(Seq#Update(s, i, v), n) } 
+  0 <= i && i < n && n <= Seq#Length(s)
+     ==> Seq#Take(Seq#Update(s, i, v), n) == Seq#Update(Seq#Take(s, n), i, v));
+
+axiom (forall s: Seq, i: int, v: Box, n: int :: 
+  { Seq#Take(Seq#Update(s, i, v), n) } 
+  n <= i && i < Seq#Length(s)
+     ==> Seq#Take(Seq#Update(s, i, v), n) == Seq#Take(s, n));
+
+axiom (forall s: Seq, i: int, v: Box, n: int :: 
+  { Seq#Drop(Seq#Update(s, i, v), n) } 
+  0 <= n && n <= i && i < Seq#Length(s)
+     ==> Seq#Drop(Seq#Update(s, i, v), n) == Seq#Update(Seq#Drop(s, n), i - n, v));
+
+axiom (forall s: Seq, i: int, v: Box, n: int :: 
+  { Seq#Drop(Seq#Update(s, i, v), n) } 
+  0 <= i && i < n && n <= Seq#Length(s)
+     ==> Seq#Drop(Seq#Update(s, i, v), n) == Seq#Drop(s, n));
+
+axiom (forall s: Seq, v: Box, n: int :: 
+  { Seq#Drop(Seq#Build(s, v), n) } 
+  0 <= n && n <= Seq#Length(s)
+     ==> Seq#Drop(Seq#Build(s, v), n) == Seq#Build(Seq#Drop(s, n), v));
+
+axiom (forall s: Seq, n: int :: { Seq#Drop(s, n) } n == 0 ==> Seq#Drop(s, n) == s);
+
+axiom (forall s: Seq, n: int :: 
+  { Seq#Take(s, n) } 
+  n == 0 ==> Seq#Take(s, n) == Seq#Empty());
+
+axiom (forall s: Seq, m: int, n: int :: 
+  { Seq#Drop(Seq#Drop(s, m), n) } 
+  0 <= m && 0 <= n && m + n <= Seq#Length(s)
+     ==> Seq#Drop(Seq#Drop(s, m), n) == Seq#Drop(s, m + n));
+
+axiom (forall s: Seq, bx: Box, t: Ty :: 
+  { $Is(Seq#Build(s, bx), TSeq(t)) } 
+  $Is(s, TSeq(t)) && $IsBox(bx, t) ==> $Is(Seq#Build(s, bx), TSeq(t)));
+
+revealed function Seq#Create(ty: Ty, heap: Heap, len: int, init: HandleType) : Seq;
+
+axiom (forall ty: Ty, heap: Heap, len: int, init: HandleType :: 
+  { Seq#Length(Seq#Create(ty, heap, len, init): Seq) } 
+  $IsGoodHeap(heap) && 0 <= len
+     ==> Seq#Length(Seq#Create(ty, heap, len, init): Seq) == len);
+
+axiom (forall ty: Ty, heap: Heap, len: int, init: HandleType, i: int :: 
+  { Seq#Index(Seq#Create(ty, heap, len, init), i) } 
+  $IsGoodHeap(heap) && 0 <= i && i < len
+     ==> Seq#Index(Seq#Create(ty, heap, len, init), i)
+       == Apply1(TInt, ty, heap, init, $Box(i)));
+
+revealed function Seq#FromArray(h: Heap, a: ref) : Seq;
 
 axiom (forall h: Heap, a: ref :: 
   { Seq#Length(Seq#FromArray(h, a)) } 
@@ -1306,18 +1487,13 @@ axiom (forall h: Heap, a: ref ::
 axiom (forall h: Heap, a: ref :: 
   { Seq#FromArray(h, a) } 
   (forall i: int :: 
-    { read(h, a, IndexField(i)) } { Seq#Index(Seq#FromArray(h, a): Seq Box, i) } 
+    { read(h, a, IndexField(i)) } { Seq#Index(Seq#FromArray(h, a): Seq, i) } 
     0 <= i && i < Seq#Length(Seq#FromArray(h, a))
        ==> Seq#Index(Seq#FromArray(h, a), i) == read(h, a, IndexField(i))));
 
 axiom (forall h0: Heap, h1: Heap, a: ref :: 
   { Seq#FromArray(h1, a), $HeapSucc(h0, h1) } 
-  $IsGoodHeap(h0)
-       && $IsGoodHeap(h1)
-       && $HeapSucc(h0, h1)
-       && (forall i: int :: 
-        0 <= i && i < _System.array.Length(a)
-           ==> read(h0, a, IndexField(i)) == read(h1, a, IndexField(i)))
+  $IsGoodHeap(h0) && $IsGoodHeap(h1) && $HeapSucc(h0, h1) && h0[a] == h1[a]
      ==> Seq#FromArray(h0, a) == Seq#FromArray(h1, a));
 
 axiom (forall h: Heap, i: int, v: Box, a: ref :: 
@@ -1326,221 +1502,256 @@ axiom (forall h: Heap, i: int, v: Box, a: ref ::
      ==> Seq#FromArray(update(h, a, IndexField(i), v), a)
        == Seq#Update(Seq#FromArray(h, a), i, v));
 
-axiom (forall<T> s: Seq T, i: int, v: T, n: int :: 
-  { Seq#Take(Seq#Update(s, i, v), n) } 
-  0 <= i && i < n && n <= Seq#Length(s)
-     ==> Seq#Take(Seq#Update(s, i, v), n) == Seq#Update(Seq#Take(s, n), i, v));
-
-axiom (forall<T> s: Seq T, i: int, v: T, n: int :: 
-  { Seq#Take(Seq#Update(s, i, v), n) } 
-  n <= i && i < Seq#Length(s)
-     ==> Seq#Take(Seq#Update(s, i, v), n) == Seq#Take(s, n));
-
-axiom (forall<T> s: Seq T, i: int, v: T, n: int :: 
-  { Seq#Drop(Seq#Update(s, i, v), n) } 
-  0 <= n && n <= i && i < Seq#Length(s)
-     ==> Seq#Drop(Seq#Update(s, i, v), n) == Seq#Update(Seq#Drop(s, n), i - n, v));
-
-axiom (forall<T> s: Seq T, i: int, v: T, n: int :: 
-  { Seq#Drop(Seq#Update(s, i, v), n) } 
-  0 <= i && i < n && n < Seq#Length(s)
-     ==> Seq#Drop(Seq#Update(s, i, v), n) == Seq#Drop(s, n));
-
 axiom (forall h: Heap, a: ref, n0: int, n1: int :: 
   { Seq#Take(Seq#FromArray(h, a), n0), Seq#Take(Seq#FromArray(h, a), n1) } 
   n0 + 1 == n1 && 0 <= n0 && n1 <= _System.array.Length(a)
      ==> Seq#Take(Seq#FromArray(h, a), n1)
-       == Seq#Build(Seq#Take(Seq#FromArray(h, a), n0), read(h, a, IndexField(n0): Field Box)));
+       == Seq#Build(Seq#Take(Seq#FromArray(h, a), n0), read(h, a, IndexField(n0): Field)));
 
-axiom (forall<T> s: Seq T, v: T, n: int :: 
-  { Seq#Drop(Seq#Build(s, v), n) } 
-  0 <= n && n <= Seq#Length(s)
-     ==> Seq#Drop(Seq#Build(s, v), n) == Seq#Build(Seq#Drop(s, n), v));
+revealed function Seq#Rank(Seq) : int;
 
-function Seq#Rank<T>(Seq T) : int;
-
-axiom (forall s: Seq Box, i: int :: 
+axiom (forall s: Seq, i: int :: 
   { DtRank($Unbox(Seq#Index(s, i)): DatatypeType) } 
   0 <= i && i < Seq#Length(s)
      ==> DtRank($Unbox(Seq#Index(s, i)): DatatypeType) < Seq#Rank(s));
 
-axiom (forall<T> s: Seq T, i: int :: 
+axiom (forall s: Seq, i: int :: 
   { Seq#Rank(Seq#Drop(s, i)) } 
   0 < i && i <= Seq#Length(s) ==> Seq#Rank(Seq#Drop(s, i)) < Seq#Rank(s));
 
-axiom (forall<T> s: Seq T, i: int :: 
+axiom (forall s: Seq, i: int :: 
   { Seq#Rank(Seq#Take(s, i)) } 
   0 <= i && i < Seq#Length(s) ==> Seq#Rank(Seq#Take(s, i)) < Seq#Rank(s));
 
-axiom (forall<T> s: Seq T, i: int, j: int :: 
+axiom (forall s: Seq, i: int, j: int :: 
   { Seq#Rank(Seq#Append(Seq#Take(s, i), Seq#Drop(s, j))) } 
   0 <= i && i < j && j <= Seq#Length(s)
      ==> Seq#Rank(Seq#Append(Seq#Take(s, i), Seq#Drop(s, j))) < Seq#Rank(s));
 
-axiom (forall<T> s: Seq T, n: int :: 
-  { Seq#Drop(s, n) } 
-  n == 0 ==> Seq#Drop(s, n) == s);
+type Map;
 
-axiom (forall<T> s: Seq T, n: int :: 
-  { Seq#Take(s, n) } 
-  n == 0 ==> Seq#Take(s, n) == Seq#Empty());
+revealed function Map#Domain(Map) : Set;
 
-axiom (forall<T> s: Seq T, m: int, n: int :: 
-  { Seq#Drop(Seq#Drop(s, m), n) } 
-  0 <= m && 0 <= n && m + n <= Seq#Length(s)
-     ==> Seq#Drop(Seq#Drop(s, m), n) == Seq#Drop(s, m + n));
+revealed function Map#Elements(Map) : [Box]Box;
 
-type Map _ _;
+revealed function Map#Card(Map) : int;
 
-function Map#Domain<U,V>(Map U V) : Set U;
+axiom (forall m: Map :: { Map#Card(m) } 0 <= Map#Card(m));
 
-function Map#Elements<U,V>(Map U V) : [U]V;
+axiom (forall m: Map :: { Map#Card(m) } Map#Card(m) == 0 <==> m == Map#Empty());
 
-function Map#Card<U,V>(Map U V) : int;
+axiom (forall m: Map :: 
+  { Map#Domain(m) } 
+  m == Map#Empty() || (exists k: Box :: Set#IsMember(Map#Domain(m), k)));
 
-axiom (forall<U,V> m: Map U V :: { Map#Card(m) } 0 <= Map#Card(m));
+axiom (forall m: Map :: 
+  { Map#Values(m) } 
+  m == Map#Empty() || (exists v: Box :: Set#IsMember(Map#Values(m), v)));
 
-axiom (forall<U,V> m: Map U V :: 
-  { Set#Card(Map#Domain(m)) } 
+axiom (forall m: Map :: 
+  { Map#Items(m) } 
+  m == Map#Empty()
+     || (exists k: Box, v: Box :: 
+      Set#IsMember(Map#Items(m), $Box(#_System._tuple#2._#Make2(k, v)))));
+
+axiom (forall m: Map :: 
+  { Set#Card(Map#Domain(m)) } { Map#Card(m) } 
   Set#Card(Map#Domain(m)) == Map#Card(m));
 
-function Map#Values<U,V>(Map U V) : Set V;
+axiom (forall m: Map :: 
+  { Set#Card(Map#Values(m)) } { Map#Card(m) } 
+  Set#Card(Map#Values(m)) <= Map#Card(m));
 
-axiom (forall<U,V> m: Map U V, v: V :: 
-  { Map#Values(m)[v] } 
-  Map#Values(m)[v]
-     == (exists u: U :: 
-      { Map#Domain(m)[u] } { Map#Elements(m)[u] } 
-      Map#Domain(m)[u] && v == Map#Elements(m)[u]));
-
-function Map#Items<U,V>(Map U V) : Set Box;
-
-function _System.Tuple2._0(DatatypeType) : Box;
-
-function _System.Tuple2._1(DatatypeType) : Box;
-
-axiom (forall<U,V> m: Map U V :: 
-  { Set#Card(Map#Items(m)) } 
+axiom (forall m: Map :: 
+  { Set#Card(Map#Items(m)) } { Map#Card(m) } 
   Set#Card(Map#Items(m)) == Map#Card(m));
 
-axiom (forall m: Map Box Box, item: Box :: 
-  { Map#Items(m)[item] } 
-  Map#Items(m)[item]
-     <==> Map#Domain(m)[_System.Tuple2._0($Unbox(item))]
+revealed function Map#Values(Map) : Set;
+
+axiom (forall m: Map, v: Box :: 
+  { Set#IsMember(Map#Values(m), v) } 
+  Set#IsMember(Map#Values(m), v)
+     == (exists u: Box :: 
+      { Set#IsMember(Map#Domain(m), u) } { Map#Elements(m)[u] } 
+      Set#IsMember(Map#Domain(m), u) && v == Map#Elements(m)[u]));
+
+revealed function Map#Items(Map) : Set;
+
+revealed function #_System._tuple#2._#Make2(Box, Box) : DatatypeType;
+
+revealed function _System.Tuple2._0(DatatypeType) : Box;
+
+revealed function _System.Tuple2._1(DatatypeType) : Box;
+
+axiom (forall m: Map, item: Box :: 
+  { Set#IsMember(Map#Items(m), item) } 
+  Set#IsMember(Map#Items(m), item)
+     <==> Set#IsMember(Map#Domain(m), _System.Tuple2._0($Unbox(item)))
        && Map#Elements(m)[_System.Tuple2._0($Unbox(item))]
          == _System.Tuple2._1($Unbox(item)));
 
-function Map#Empty<U,V>() : Map U V;
+revealed function Map#Empty() : Map;
 
-axiom (forall<U,V> u: U :: 
-  { Map#Domain(Map#Empty(): Map U V)[u] } 
-  !Map#Domain(Map#Empty(): Map U V)[u]);
+axiom (forall u: Box :: 
+  { Set#IsMember(Map#Domain(Map#Empty(): Map), u) } 
+  !Set#IsMember(Map#Domain(Map#Empty(): Map), u));
 
-axiom (forall<U,V> m: Map U V :: 
-  { Map#Card(m) } 
-  (Map#Card(m) == 0 <==> m == Map#Empty())
-     && (Map#Card(m) != 0 ==> (exists x: U :: Map#Domain(m)[x])));
+revealed function Map#Glue(Set, [Box]Box, Ty) : Map;
 
-function Map#Glue<U,V>([U]bool, [U]V, Ty) : Map U V;
-
-axiom (forall<U,V> a: [U]bool, b: [U]V, t: Ty :: 
+axiom (forall a: Set, b: [Box]Box, t: Ty :: 
   { Map#Domain(Map#Glue(a, b, t)) } 
   Map#Domain(Map#Glue(a, b, t)) == a);
 
-axiom (forall<U,V> a: [U]bool, b: [U]V, t: Ty :: 
+axiom (forall a: Set, b: [Box]Box, t: Ty :: 
   { Map#Elements(Map#Glue(a, b, t)) } 
   Map#Elements(Map#Glue(a, b, t)) == b);
 
-axiom (forall<U,V> a: [U]bool, b: [U]V, t: Ty :: 
-  { $Is(Map#Glue(a, b, t), t) } 
-  $Is(Map#Glue(a, b, t), t));
+axiom (forall a: Set, b: [Box]Box, t0: Ty, t1: Ty :: 
+  { Map#Glue(a, b, TMap(t0, t1)) } 
+  (forall bx: Box :: Set#IsMember(a, bx) ==> $IsBox(bx, t0) && $IsBox(b[bx], t1))
+     ==> $Is(Map#Glue(a, b, TMap(t0, t1)), TMap(t0, t1)));
 
-function Map#Build<U,V>(Map U V, U, V) : Map U V;
+revealed function Map#Build(Map, Box, Box) : Map;
 
-axiom (forall<U,V> m: Map U V, u: U, u': U, v: V :: 
-  { Map#Domain(Map#Build(m, u, v))[u'] } { Map#Elements(Map#Build(m, u, v))[u'] } 
+axiom (forall m: Map, u: Box, u': Box, v: Box :: 
+  { Set#IsMember(Map#Domain(Map#Build(m, u, v)), u') } 
+    { Map#Elements(Map#Build(m, u, v))[u'] } 
   (u' == u
-       ==> Map#Domain(Map#Build(m, u, v))[u'] && Map#Elements(Map#Build(m, u, v))[u'] == v)
+       ==> Set#IsMember(Map#Domain(Map#Build(m, u, v)), u')
+         && Map#Elements(Map#Build(m, u, v))[u'] == v)
      && (u' != u
-       ==> Map#Domain(Map#Build(m, u, v))[u'] == Map#Domain(m)[u']
+       ==> Set#IsMember(Map#Domain(Map#Build(m, u, v)), u')
+           == Set#IsMember(Map#Domain(m), u')
          && Map#Elements(Map#Build(m, u, v))[u'] == Map#Elements(m)[u']));
 
-axiom (forall<U,V> m: Map U V, u: U, v: V :: 
+axiom (forall m: Map, u: Box, v: Box :: 
   { Map#Card(Map#Build(m, u, v)) } 
-  Map#Domain(m)[u] ==> Map#Card(Map#Build(m, u, v)) == Map#Card(m));
+  Set#IsMember(Map#Domain(m), u) ==> Map#Card(Map#Build(m, u, v)) == Map#Card(m));
 
-axiom (forall<U,V> m: Map U V, u: U, v: V :: 
+axiom (forall m: Map, u: Box, v: Box :: 
   { Map#Card(Map#Build(m, u, v)) } 
-  !Map#Domain(m)[u] ==> Map#Card(Map#Build(m, u, v)) == Map#Card(m) + 1);
+  !Set#IsMember(Map#Domain(m), u)
+     ==> Map#Card(Map#Build(m, u, v)) == Map#Card(m) + 1);
 
-function Map#Equal<U,V>(Map U V, Map U V) : bool;
+revealed function Map#Merge(Map, Map) : Map;
 
-axiom (forall<U,V> m: Map U V, m': Map U V :: 
+axiom (forall m: Map, n: Map :: 
+  { Map#Domain(Map#Merge(m, n)) } 
+  Map#Domain(Map#Merge(m, n)) == Set#Union(Map#Domain(m), Map#Domain(n)));
+
+axiom (forall m: Map, n: Map, u: Box :: 
+  { Map#Elements(Map#Merge(m, n))[u] } 
+  Set#IsMember(Map#Domain(Map#Merge(m, n)), u)
+     ==> (!Set#IsMember(Map#Domain(n), u)
+         ==> Map#Elements(Map#Merge(m, n))[u] == Map#Elements(m)[u])
+       && (Set#IsMember(Map#Domain(n), u)
+         ==> Map#Elements(Map#Merge(m, n))[u] == Map#Elements(n)[u]));
+
+revealed function Map#Subtract(Map, Set) : Map;
+
+axiom (forall m: Map, s: Set :: 
+  { Map#Domain(Map#Subtract(m, s)) } 
+  Map#Domain(Map#Subtract(m, s)) == Set#Difference(Map#Domain(m), s));
+
+axiom (forall m: Map, s: Set, u: Box :: 
+  { Map#Elements(Map#Subtract(m, s))[u] } 
+  Set#IsMember(Map#Domain(Map#Subtract(m, s)), u)
+     ==> Map#Elements(Map#Subtract(m, s))[u] == Map#Elements(m)[u]);
+
+revealed function Map#Equal(Map, Map) : bool;
+
+axiom (forall m: Map, m': Map :: 
   { Map#Equal(m, m') } 
   Map#Equal(m, m')
-     <==> (forall u: U :: Map#Domain(m)[u] == Map#Domain(m')[u])
-       && (forall u: U :: Map#Domain(m)[u] ==> Map#Elements(m)[u] == Map#Elements(m')[u]));
+     <==> (forall u: Box :: 
+        Set#IsMember(Map#Domain(m), u) == Set#IsMember(Map#Domain(m'), u))
+       && (forall u: Box :: 
+        Set#IsMember(Map#Domain(m), u) ==> Map#Elements(m)[u] == Map#Elements(m')[u]));
 
-axiom (forall<U,V> m: Map U V, m': Map U V :: 
-  { Map#Equal(m, m') } 
-  Map#Equal(m, m') ==> m == m');
+axiom (forall m: Map, m': Map :: { Map#Equal(m, m') } Map#Equal(m, m') ==> m == m');
 
-function Map#Disjoint<U,V>(Map U V, Map U V) : bool;
+revealed function Map#Disjoint(Map, Map) : bool;
 
-axiom (forall<U,V> m: Map U V, m': Map U V :: 
+axiom (forall m: Map, m': Map :: 
   { Map#Disjoint(m, m') } 
   Map#Disjoint(m, m')
-     <==> (forall o: U :: 
-      { Map#Domain(m)[o] } { Map#Domain(m')[o] } 
-      !Map#Domain(m)[o] || !Map#Domain(m')[o]));
+     <==> (forall o: Box :: 
+      { Set#IsMember(Map#Domain(m), o) } { Set#IsMember(Map#Domain(m'), o) } 
+      !Set#IsMember(Map#Domain(m), o) || !Set#IsMember(Map#Domain(m'), o)));
 
-type IMap _ _;
+type IMap;
 
-function IMap#Domain<U,V>(IMap U V) : Set U;
+revealed function IMap#Domain(IMap) : ISet;
 
-function IMap#Elements<U,V>(IMap U V) : [U]V;
+revealed function IMap#Elements(IMap) : [Box]Box;
 
-function IMap#Values<U,V>(IMap U V) : Set V;
+axiom (forall m: IMap :: 
+  { IMap#Domain(m) } 
+  m == IMap#Empty() || (exists k: Box :: IMap#Domain(m)[k]));
 
-axiom (forall<U,V> m: IMap U V, v: V :: 
+axiom (forall m: IMap :: 
+  { IMap#Values(m) } 
+  m == IMap#Empty() || (exists v: Box :: IMap#Values(m)[v]));
+
+axiom (forall m: IMap :: 
+  { IMap#Items(m) } 
+  m == IMap#Empty()
+     || (exists k: Box, v: Box :: IMap#Items(m)[$Box(#_System._tuple#2._#Make2(k, v))]));
+
+axiom (forall m: IMap :: 
+  { IMap#Domain(m) } 
+  m == IMap#Empty() <==> IMap#Domain(m) == ISet#Empty());
+
+axiom (forall m: IMap :: 
+  { IMap#Values(m) } 
+  m == IMap#Empty() <==> IMap#Values(m) == ISet#Empty());
+
+axiom (forall m: IMap :: 
+  { IMap#Items(m) } 
+  m == IMap#Empty() <==> IMap#Items(m) == ISet#Empty());
+
+revealed function IMap#Values(IMap) : ISet;
+
+axiom (forall m: IMap, v: Box :: 
   { IMap#Values(m)[v] } 
   IMap#Values(m)[v]
-     == (exists u: U :: 
+     == (exists u: Box :: 
       { IMap#Domain(m)[u] } { IMap#Elements(m)[u] } 
       IMap#Domain(m)[u] && v == IMap#Elements(m)[u]));
 
-function IMap#Items<U,V>(IMap U V) : Set Box;
+revealed function IMap#Items(IMap) : ISet;
 
-axiom (forall m: IMap Box Box, item: Box :: 
+axiom (forall m: IMap, item: Box :: 
   { IMap#Items(m)[item] } 
   IMap#Items(m)[item]
      <==> IMap#Domain(m)[_System.Tuple2._0($Unbox(item))]
        && IMap#Elements(m)[_System.Tuple2._0($Unbox(item))]
          == _System.Tuple2._1($Unbox(item)));
 
-function IMap#Empty<U,V>() : IMap U V;
+revealed function IMap#Empty() : IMap;
 
-axiom (forall<U,V> u: U :: 
-  { IMap#Domain(IMap#Empty(): IMap U V)[u] } 
-  !IMap#Domain(IMap#Empty(): IMap U V)[u]);
+axiom (forall u: Box :: 
+  { IMap#Domain(IMap#Empty(): IMap)[u] } 
+  !IMap#Domain(IMap#Empty(): IMap)[u]);
 
-function IMap#Glue<U,V>([U]bool, [U]V, Ty) : IMap U V;
+revealed function IMap#Glue([Box]bool, [Box]Box, Ty) : IMap;
 
-axiom (forall<U,V> a: [U]bool, b: [U]V, t: Ty :: 
+axiom (forall a: [Box]bool, b: [Box]Box, t: Ty :: 
   { IMap#Domain(IMap#Glue(a, b, t)) } 
   IMap#Domain(IMap#Glue(a, b, t)) == a);
 
-axiom (forall<U,V> a: [U]bool, b: [U]V, t: Ty :: 
+axiom (forall a: [Box]bool, b: [Box]Box, t: Ty :: 
   { IMap#Elements(IMap#Glue(a, b, t)) } 
   IMap#Elements(IMap#Glue(a, b, t)) == b);
 
-axiom (forall<U,V> a: [U]bool, b: [U]V, t: Ty :: 
-  { $Is(IMap#Glue(a, b, t), t) } 
-  $Is(IMap#Glue(a, b, t), t));
+axiom (forall a: [Box]bool, b: [Box]Box, t0: Ty, t1: Ty :: 
+  { IMap#Glue(a, b, TIMap(t0, t1)) } 
+  (forall bx: Box :: a[bx] ==> $IsBox(bx, t0) && $IsBox(b[bx], t1))
+     ==> $Is(IMap#Glue(a, b, TIMap(t0, t1)), TIMap(t0, t1)));
 
-function IMap#Build<U,V>(IMap U V, U, V) : IMap U V;
+revealed function IMap#Build(IMap, Box, Box) : IMap;
 
-axiom (forall<U,V> m: IMap U V, u: U, u': U, v: V :: 
+axiom (forall m: IMap, u: Box, u': Box, v: Box :: 
   { IMap#Domain(IMap#Build(m, u, v))[u'] } 
     { IMap#Elements(IMap#Build(m, u, v))[u'] } 
   (u' == u
@@ -1550,97 +1761,139 @@ axiom (forall<U,V> m: IMap U V, u: U, u': U, v: V ::
        ==> IMap#Domain(IMap#Build(m, u, v))[u'] == IMap#Domain(m)[u']
          && IMap#Elements(IMap#Build(m, u, v))[u'] == IMap#Elements(m)[u']));
 
-function IMap#Equal<U,V>(IMap U V, IMap U V) : bool;
+revealed function IMap#Equal(IMap, IMap) : bool;
 
-axiom (forall<U,V> m: IMap U V, m': IMap U V :: 
+axiom (forall m: IMap, m': IMap :: 
   { IMap#Equal(m, m') } 
   IMap#Equal(m, m')
-     <==> (forall u: U :: IMap#Domain(m)[u] == IMap#Domain(m')[u])
-       && (forall u: U :: 
+     <==> (forall u: Box :: IMap#Domain(m)[u] == IMap#Domain(m')[u])
+       && (forall u: Box :: 
         IMap#Domain(m)[u] ==> IMap#Elements(m)[u] == IMap#Elements(m')[u]));
 
-axiom (forall<U,V> m: IMap U V, m': IMap U V :: 
+axiom (forall m: IMap, m': IMap :: 
   { IMap#Equal(m, m') } 
   IMap#Equal(m, m') ==> m == m');
 
-function INTERNAL_add_boogie(x: int, y: int) : int;
+revealed function IMap#Merge(IMap, IMap) : IMap;
 
+axiom (forall m: IMap, n: IMap :: 
+  { IMap#Domain(IMap#Merge(m, n)) } 
+  IMap#Domain(IMap#Merge(m, n)) == ISet#Union(IMap#Domain(m), IMap#Domain(n)));
+
+axiom (forall m: IMap, n: IMap, u: Box :: 
+  { IMap#Elements(IMap#Merge(m, n))[u] } 
+  IMap#Domain(IMap#Merge(m, n))[u]
+     ==> (!IMap#Domain(n)[u]
+         ==> IMap#Elements(IMap#Merge(m, n))[u] == IMap#Elements(m)[u])
+       && (IMap#Domain(n)[u]
+         ==> IMap#Elements(IMap#Merge(m, n))[u] == IMap#Elements(n)[u]));
+
+revealed function IMap#Subtract(IMap, Set) : IMap;
+
+axiom (forall m: IMap, s: Set :: 
+  { IMap#Domain(IMap#Subtract(m, s)) } 
+  IMap#Domain(IMap#Subtract(m, s))
+     == ISet#Difference(IMap#Domain(m), ISet#FromSet(s)));
+
+axiom (forall m: IMap, s: Set, u: Box :: 
+  { IMap#Elements(IMap#Subtract(m, s))[u] } 
+  IMap#Domain(IMap#Subtract(m, s))[u]
+     ==> IMap#Elements(IMap#Subtract(m, s))[u] == IMap#Elements(m)[u]);
+
+revealed function INTERNAL_add_boogie(x: int, y: int) : int
+uses {
 axiom (forall x: int, y: int :: 
   { INTERNAL_add_boogie(x, y): int } 
   INTERNAL_add_boogie(x, y): int == x + y);
+}
 
-function INTERNAL_sub_boogie(x: int, y: int) : int;
-
+revealed function INTERNAL_sub_boogie(x: int, y: int) : int
+uses {
 axiom (forall x: int, y: int :: 
   { INTERNAL_sub_boogie(x, y): int } 
   INTERNAL_sub_boogie(x, y): int == x - y);
+}
 
-function INTERNAL_mul_boogie(x: int, y: int) : int;
-
+revealed function INTERNAL_mul_boogie(x: int, y: int) : int
+uses {
 axiom (forall x: int, y: int :: 
   { INTERNAL_mul_boogie(x, y): int } 
   INTERNAL_mul_boogie(x, y): int == x * y);
+}
 
-function INTERNAL_div_boogie(x: int, y: int) : int;
-
+revealed function INTERNAL_div_boogie(x: int, y: int) : int
+uses {
 axiom (forall x: int, y: int :: 
   { INTERNAL_div_boogie(x, y): int } 
   INTERNAL_div_boogie(x, y): int == x div y);
+}
 
-function INTERNAL_mod_boogie(x: int, y: int) : int;
-
+revealed function INTERNAL_mod_boogie(x: int, y: int) : int
+uses {
 axiom (forall x: int, y: int :: 
   { INTERNAL_mod_boogie(x, y): int } 
   INTERNAL_mod_boogie(x, y): int == x mod y);
+}
 
-function {:never_pattern true} INTERNAL_lt_boogie(x: int, y: int) : bool;
-
+revealed function {:never_pattern true} INTERNAL_lt_boogie(x: int, y: int) : bool
+uses {
 axiom (forall x: int, y: int :: 
   {:never_pattern true} { INTERNAL_lt_boogie(x, y): bool } 
   INTERNAL_lt_boogie(x, y): bool == (x < y));
+}
 
-function {:never_pattern true} INTERNAL_le_boogie(x: int, y: int) : bool;
-
+revealed function {:never_pattern true} INTERNAL_le_boogie(x: int, y: int) : bool
+uses {
 axiom (forall x: int, y: int :: 
   {:never_pattern true} { INTERNAL_le_boogie(x, y): bool } 
   INTERNAL_le_boogie(x, y): bool == (x <= y));
+}
 
-function {:never_pattern true} INTERNAL_gt_boogie(x: int, y: int) : bool;
-
+revealed function {:never_pattern true} INTERNAL_gt_boogie(x: int, y: int) : bool
+uses {
 axiom (forall x: int, y: int :: 
   {:never_pattern true} { INTERNAL_gt_boogie(x, y): bool } 
   INTERNAL_gt_boogie(x, y): bool == (x > y));
+}
 
-function {:never_pattern true} INTERNAL_ge_boogie(x: int, y: int) : bool;
-
+revealed function {:never_pattern true} INTERNAL_ge_boogie(x: int, y: int) : bool
+uses {
 axiom (forall x: int, y: int :: 
   {:never_pattern true} { INTERNAL_ge_boogie(x, y): bool } 
   INTERNAL_ge_boogie(x, y): bool == (x >= y));
+}
 
-function Mul(x: int, y: int) : int;
-
+revealed function Mul(x: int, y: int) : int
+uses {
 axiom (forall x: int, y: int :: { Mul(x, y): int } Mul(x, y): int == x * y);
+}
 
-function Div(x: int, y: int) : int;
-
+revealed function Div(x: int, y: int) : int
+uses {
 axiom (forall x: int, y: int :: { Div(x, y): int } Div(x, y): int == x div y);
+}
 
-function Mod(x: int, y: int) : int;
-
+revealed function Mod(x: int, y: int) : int
+uses {
 axiom (forall x: int, y: int :: { Mod(x, y): int } Mod(x, y): int == x mod y);
+}
 
-function Add(x: int, y: int) : int;
-
+revealed function Add(x: int, y: int) : int
+uses {
 axiom (forall x: int, y: int :: { Add(x, y): int } Add(x, y): int == x + y);
+}
 
-function Sub(x: int, y: int) : int;
-
+revealed function Sub(x: int, y: int) : int
+uses {
 axiom (forall x: int, y: int :: { Sub(x, y): int } Sub(x, y): int == x - y);
+}
 
-function Tclass._System.nat() : Ty;
-
+function Tclass._System.nat() : Ty
+uses {
 // Tclass._System.nat Tag
-axiom Tag(Tclass._System.nat()) == Tagclass._System.nat;
+axiom Tag(Tclass._System.nat()) == Tagclass._System.nat
+   && TagFamily(Tclass._System.nat()) == tytagFamily$nat;
+}
 
 const unique Tagclass._System.nat: TyTag;
 
@@ -1650,20 +1903,17 @@ axiom (forall bx: Box ::
   $IsBox(bx, Tclass._System.nat())
      ==> $Box($Unbox(bx): int) == bx && $Is($Unbox(bx): int, Tclass._System.nat()));
 
-// _System.nat: subset type $Is
+// $Is axiom for subset type _System.nat
 axiom (forall x#0: int :: 
   { $Is(x#0, Tclass._System.nat()) } 
   $Is(x#0, Tclass._System.nat()) <==> LitInt(0) <= x#0);
 
-// _System.nat: subset type $IsAlloc
+// $IsAlloc axiom for subset type _System.nat
 axiom (forall x#0: int, $h: Heap :: 
   { $IsAlloc(x#0, Tclass._System.nat(), $h) } 
   $IsAlloc(x#0, Tclass._System.nat(), $h));
 
 const unique class._System.object?: ClassName;
-
-// Tclass._System.object? Tag
-axiom Tag(Tclass._System.object?()) == Tagclass._System.object?;
 
 const unique Tagclass._System.object?: TyTag;
 
@@ -1673,23 +1923,25 @@ axiom (forall bx: Box ::
   $IsBox(bx, Tclass._System.object?())
      ==> $Box($Unbox(bx): ref) == bx && $Is($Unbox(bx): ref, Tclass._System.object?()));
 
-// object: Class $Is
+// $Is axiom for trait object
 axiom (forall $o: ref :: 
   { $Is($o, Tclass._System.object?()) } 
   $Is($o, Tclass._System.object?()));
 
-// object: Class $IsAlloc
+// $IsAlloc axiom for trait object
 axiom (forall $o: ref, $h: Heap :: 
   { $IsAlloc($o, Tclass._System.object?(), $h) } 
   $IsAlloc($o, Tclass._System.object?(), $h)
-     <==> $o == null || read($h, $o, alloc));
+     <==> $o == null || $Unbox(read($h, $o, alloc)): bool);
 
-function implements$_System.object(Ty) : bool;
+function implements$_System.object(ty: Ty) : bool;
 
-function Tclass._System.object() : Ty;
-
+function Tclass._System.object() : Ty
+uses {
 // Tclass._System.object Tag
-axiom Tag(Tclass._System.object()) == Tagclass._System.object;
+axiom Tag(Tclass._System.object()) == Tagclass._System.object
+   && TagFamily(Tclass._System.object()) == tytagFamily$object;
+}
 
 const unique Tagclass._System.object: TyTag;
 
@@ -1699,13 +1951,13 @@ axiom (forall bx: Box ::
   $IsBox(bx, Tclass._System.object())
      ==> $Box($Unbox(bx): ref) == bx && $Is($Unbox(bx): ref, Tclass._System.object()));
 
-// _System.object: subset type $Is
+// $Is axiom for non-null type _System.object
 axiom (forall c#0: ref :: 
-  { $Is(c#0, Tclass._System.object()) } 
+  { $Is(c#0, Tclass._System.object()) } { $Is(c#0, Tclass._System.object?()) } 
   $Is(c#0, Tclass._System.object())
      <==> $Is(c#0, Tclass._System.object?()) && c#0 != null);
 
-// _System.object: subset type $IsAlloc
+// $IsAlloc axiom for non-null type _System.object
 axiom (forall c#0: ref, $h: Heap :: 
   { $IsAlloc(c#0, Tclass._System.object(), $h) } 
   $IsAlloc(c#0, Tclass._System.object(), $h)
@@ -1715,96 +1967,99 @@ const unique class._System.array?: ClassName;
 
 function Tclass._System.array?(Ty) : Ty;
 
-// Tclass._System.array? Tag
-axiom (forall #$arg: Ty :: 
-  { Tclass._System.array?(#$arg) } 
-  Tag(Tclass._System.array?(#$arg)) == Tagclass._System.array?);
-
 const unique Tagclass._System.array?: TyTag;
 
-// Tclass._System.array? injectivity 0
-axiom (forall #$arg: Ty :: 
-  { Tclass._System.array?(#$arg) } 
-  Tclass._System.array?_0(Tclass._System.array?(#$arg)) == #$arg);
+// Tclass._System.array? Tag
+axiom (forall _System.array$arg: Ty :: 
+  { Tclass._System.array?(_System.array$arg) } 
+  Tag(Tclass._System.array?(_System.array$arg)) == Tagclass._System.array?
+     && TagFamily(Tclass._System.array?(_System.array$arg)) == tytagFamily$array);
 
 function Tclass._System.array?_0(Ty) : Ty;
 
+// Tclass._System.array? injectivity 0
+axiom (forall _System.array$arg: Ty :: 
+  { Tclass._System.array?(_System.array$arg) } 
+  Tclass._System.array?_0(Tclass._System.array?(_System.array$arg))
+     == _System.array$arg);
+
 // Box/unbox axiom for Tclass._System.array?
-axiom (forall #$arg: Ty, bx: Box :: 
-  { $IsBox(bx, Tclass._System.array?(#$arg)) } 
-  $IsBox(bx, Tclass._System.array?(#$arg))
+axiom (forall _System.array$arg: Ty, bx: Box :: 
+  { $IsBox(bx, Tclass._System.array?(_System.array$arg)) } 
+  $IsBox(bx, Tclass._System.array?(_System.array$arg))
      ==> $Box($Unbox(bx): ref) == bx
-       && $Is($Unbox(bx): ref, Tclass._System.array?(#$arg)));
+       && $Is($Unbox(bx): ref, Tclass._System.array?(_System.array$arg)));
 
 // array.: Type axiom
-axiom (forall #$arg: Ty, $h: Heap, $o: ref, $i0: int :: 
-  { read($h, $o, IndexField($i0)), Tclass._System.array?(#$arg) } 
+axiom (forall _System.array$arg: Ty, $h: Heap, $o: ref, $i0: int :: 
+  { read($h, $o, IndexField($i0)), Tclass._System.array?(_System.array$arg) } 
   $IsGoodHeap($h)
        && 
       $o != null
-       && dtype($o) == Tclass._System.array?(#$arg)
+       && dtype($o) == Tclass._System.array?(_System.array$arg)
        && 
       0 <= $i0
        && $i0 < _System.array.Length($o)
-     ==> $IsBox(read($h, $o, IndexField($i0)), #$arg));
+     ==> $IsBox(read($h, $o, IndexField($i0)), _System.array$arg));
 
 // array.: Allocation axiom
-axiom (forall #$arg: Ty, $h: Heap, $o: ref, $i0: int :: 
-  { read($h, $o, IndexField($i0)), Tclass._System.array?(#$arg) } 
+axiom (forall _System.array$arg: Ty, $h: Heap, $o: ref, $i0: int :: 
+  { read($h, $o, IndexField($i0)), Tclass._System.array?(_System.array$arg) } 
   $IsGoodHeap($h)
        && 
       $o != null
-       && dtype($o) == Tclass._System.array?(#$arg)
+       && dtype($o) == Tclass._System.array?(_System.array$arg)
        && 
       0 <= $i0
        && $i0 < _System.array.Length($o)
-       && read($h, $o, alloc)
-     ==> $IsAllocBox(read($h, $o, IndexField($i0)), #$arg, $h));
+       && $Unbox(read($h, $o, alloc)): bool
+     ==> $IsAllocBox(read($h, $o, IndexField($i0)), _System.array$arg, $h));
 
-// array: Class $Is
-axiom (forall #$arg: Ty, $o: ref :: 
-  { $Is($o, Tclass._System.array?(#$arg)) } 
-  $Is($o, Tclass._System.array?(#$arg))
-     <==> $o == null || dtype($o) == Tclass._System.array?(#$arg));
+// $Is axiom for array type array
+axiom (forall _System.array$arg: Ty, $o: ref :: 
+  { $Is($o, Tclass._System.array?(_System.array$arg)) } 
+  $Is($o, Tclass._System.array?(_System.array$arg))
+     <==> $o == null || dtype($o) == Tclass._System.array?(_System.array$arg));
 
-// array: Class $IsAlloc
-axiom (forall #$arg: Ty, $o: ref, $h: Heap :: 
-  { $IsAlloc($o, Tclass._System.array?(#$arg), $h) } 
-  $IsAlloc($o, Tclass._System.array?(#$arg), $h)
-     <==> $o == null || read($h, $o, alloc));
+// $IsAlloc axiom for array type array
+axiom (forall _System.array$arg: Ty, $o: ref, $h: Heap :: 
+  { $IsAlloc($o, Tclass._System.array?(_System.array$arg), $h) } 
+  $IsAlloc($o, Tclass._System.array?(_System.array$arg), $h)
+     <==> $o == null || $Unbox(read($h, $o, alloc)): bool);
 
 // array.Length: Type axiom
-axiom (forall #$arg: Ty, $o: ref :: 
-  { _System.array.Length($o), Tclass._System.array?(#$arg) } 
-  $o != null && dtype($o) == Tclass._System.array?(#$arg)
+axiom (forall _System.array$arg: Ty, $o: ref :: 
+  { _System.array.Length($o), Tclass._System.array?(_System.array$arg) } 
+  $o != null && dtype($o) == Tclass._System.array?(_System.array$arg)
      ==> $Is(_System.array.Length($o), TInt));
 
 // array.Length: Allocation axiom
-axiom (forall #$arg: Ty, $h: Heap, $o: ref :: 
-  { _System.array.Length($o), read($h, $o, alloc), Tclass._System.array?(#$arg) } 
+axiom (forall _System.array$arg: Ty, $h: Heap, $o: ref :: 
+  { _System.array.Length($o), $Unbox(read($h, $o, alloc)): bool, Tclass._System.array?(_System.array$arg) } 
   $IsGoodHeap($h)
        && 
       $o != null
-       && dtype($o) == Tclass._System.array?(#$arg)
-       && read($h, $o, alloc)
+       && dtype($o) == Tclass._System.array?(_System.array$arg)
+       && $Unbox(read($h, $o, alloc)): bool
      ==> $IsAlloc(_System.array.Length($o), TInt, $h));
 
 function Tclass._System.array(Ty) : Ty;
 
+const unique Tagclass._System.array: TyTag;
+
 // Tclass._System.array Tag
 axiom (forall _System.array$arg: Ty :: 
   { Tclass._System.array(_System.array$arg) } 
-  Tag(Tclass._System.array(_System.array$arg)) == Tagclass._System.array);
+  Tag(Tclass._System.array(_System.array$arg)) == Tagclass._System.array
+     && TagFamily(Tclass._System.array(_System.array$arg)) == tytagFamily$array);
 
-const unique Tagclass._System.array: TyTag;
+function Tclass._System.array_0(Ty) : Ty;
 
 // Tclass._System.array injectivity 0
 axiom (forall _System.array$arg: Ty :: 
   { Tclass._System.array(_System.array$arg) } 
   Tclass._System.array_0(Tclass._System.array(_System.array$arg))
      == _System.array$arg);
-
-function Tclass._System.array_0(Ty) : Ty;
 
 // Box/unbox axiom for Tclass._System.array
 axiom (forall _System.array$arg: Ty, bx: Box :: 
@@ -1813,660 +2068,42 @@ axiom (forall _System.array$arg: Ty, bx: Box ::
      ==> $Box($Unbox(bx): ref) == bx
        && $Is($Unbox(bx): ref, Tclass._System.array(_System.array$arg)));
 
-// _System.array: subset type $Is
+// $Is axiom for non-null type _System.array
 axiom (forall _System.array$arg: Ty, c#0: ref :: 
   { $Is(c#0, Tclass._System.array(_System.array$arg)) } 
+    { $Is(c#0, Tclass._System.array?(_System.array$arg)) } 
   $Is(c#0, Tclass._System.array(_System.array$arg))
      <==> $Is(c#0, Tclass._System.array?(_System.array$arg)) && c#0 != null);
 
-// _System.array: subset type $IsAlloc
+// $IsAlloc axiom for non-null type _System.array
 axiom (forall _System.array$arg: Ty, c#0: ref, $h: Heap :: 
   { $IsAlloc(c#0, Tclass._System.array(_System.array$arg), $h) } 
   $IsAlloc(c#0, Tclass._System.array(_System.array$arg), $h)
      <==> $IsAlloc(c#0, Tclass._System.array?(_System.array$arg), $h));
 
-function Tclass._System.___hFunc0(Ty) : Ty;
-
-// Tclass._System.___hFunc0 Tag
-axiom (forall #$R: Ty :: 
-  { Tclass._System.___hFunc0(#$R) } 
-  Tag(Tclass._System.___hFunc0(#$R)) == Tagclass._System.___hFunc0);
-
-const unique Tagclass._System.___hFunc0: TyTag;
-
-// Tclass._System.___hFunc0 injectivity 0
-axiom (forall #$R: Ty :: 
-  { Tclass._System.___hFunc0(#$R) } 
-  Tclass._System.___hFunc0_0(Tclass._System.___hFunc0(#$R)) == #$R);
-
-function Tclass._System.___hFunc0_0(Ty) : Ty;
-
-// Box/unbox axiom for Tclass._System.___hFunc0
-axiom (forall #$R: Ty, bx: Box :: 
-  { $IsBox(bx, Tclass._System.___hFunc0(#$R)) } 
-  $IsBox(bx, Tclass._System.___hFunc0(#$R))
-     ==> $Box($Unbox(bx): HandleType) == bx
-       && $Is($Unbox(bx): HandleType, Tclass._System.___hFunc0(#$R)));
-
-function Handle0([Heap]Box, [Heap]bool, [Heap]Set Box) : HandleType;
-
-function Apply0(Ty, Heap, HandleType) : Box;
-
-function Requires0(Ty, Heap, HandleType) : bool;
-
-function Reads0(Ty, Heap, HandleType) : Set Box;
-
-axiom (forall t0: Ty, heap: Heap, h: [Heap]Box, r: [Heap]bool, rd: [Heap]Set Box :: 
-  { Apply0(t0, heap, Handle0(h, r, rd)) } 
-  Apply0(t0, heap, Handle0(h, r, rd)) == h[heap]);
-
-axiom (forall t0: Ty, heap: Heap, h: [Heap]Box, r: [Heap]bool, rd: [Heap]Set Box :: 
-  { Requires0(t0, heap, Handle0(h, r, rd)) } 
-  r[heap] ==> Requires0(t0, heap, Handle0(h, r, rd)));
-
-axiom (forall t0: Ty, heap: Heap, h: [Heap]Box, r: [Heap]bool, rd: [Heap]Set Box, bx: Box :: 
-  { Reads0(t0, heap, Handle0(h, r, rd))[bx] } 
-  Reads0(t0, heap, Handle0(h, r, rd))[bx] == rd[heap][bx]);
-
-function {:inline} Requires0#canCall(t0: Ty, heap: Heap, f: HandleType) : bool
-{
-  true
-}
-
-function {:inline} Reads0#canCall(t0: Ty, heap: Heap, f: HandleType) : bool
-{
-  true
-}
-
-// frame axiom for Reads0
-axiom (forall t0: Ty, h0: Heap, h1: Heap, f: HandleType :: 
-  { $HeapSucc(h0, h1), Reads0(t0, h1, f) } 
-  $HeapSucc(h0, h1)
-       && 
-      $IsGoodHeap(h0)
-       && $IsGoodHeap(h1)
-       && $Is(f, Tclass._System.___hFunc0(t0))
-       && (forall<a> o: ref, fld: Field a :: 
-        o != null && Reads0(t0, h0, f)[$Box(o)] ==> read(h0, o, fld) == read(h1, o, fld))
-     ==> Reads0(t0, h0, f) == Reads0(t0, h1, f));
-
-// frame axiom for Reads0
-axiom (forall t0: Ty, h0: Heap, h1: Heap, f: HandleType :: 
-  { $HeapSucc(h0, h1), Reads0(t0, h1, f) } 
-  $HeapSucc(h0, h1)
-       && 
-      $IsGoodHeap(h0)
-       && $IsGoodHeap(h1)
-       && $Is(f, Tclass._System.___hFunc0(t0))
-       && (forall<a> o: ref, fld: Field a :: 
-        o != null && Reads0(t0, h1, f)[$Box(o)] ==> read(h0, o, fld) == read(h1, o, fld))
-     ==> Reads0(t0, h0, f) == Reads0(t0, h1, f));
-
-// frame axiom for Requires0
-axiom (forall t0: Ty, h0: Heap, h1: Heap, f: HandleType :: 
-  { $HeapSucc(h0, h1), Requires0(t0, h1, f) } 
-  $HeapSucc(h0, h1)
-       && 
-      $IsGoodHeap(h0)
-       && $IsGoodHeap(h1)
-       && $Is(f, Tclass._System.___hFunc0(t0))
-       && (forall<a> o: ref, fld: Field a :: 
-        o != null && Reads0(t0, h0, f)[$Box(o)] ==> read(h0, o, fld) == read(h1, o, fld))
-     ==> Requires0(t0, h0, f) == Requires0(t0, h1, f));
-
-// frame axiom for Requires0
-axiom (forall t0: Ty, h0: Heap, h1: Heap, f: HandleType :: 
-  { $HeapSucc(h0, h1), Requires0(t0, h1, f) } 
-  $HeapSucc(h0, h1)
-       && 
-      $IsGoodHeap(h0)
-       && $IsGoodHeap(h1)
-       && $Is(f, Tclass._System.___hFunc0(t0))
-       && (forall<a> o: ref, fld: Field a :: 
-        o != null && Reads0(t0, h1, f)[$Box(o)] ==> read(h0, o, fld) == read(h1, o, fld))
-     ==> Requires0(t0, h0, f) == Requires0(t0, h1, f));
-
-// frame axiom for Apply0
-axiom (forall t0: Ty, h0: Heap, h1: Heap, f: HandleType :: 
-  { $HeapSucc(h0, h1), Apply0(t0, h1, f) } 
-  $HeapSucc(h0, h1)
-       && 
-      $IsGoodHeap(h0)
-       && $IsGoodHeap(h1)
-       && $Is(f, Tclass._System.___hFunc0(t0))
-       && (forall<a> o: ref, fld: Field a :: 
-        o != null && Reads0(t0, h0, f)[$Box(o)] ==> read(h0, o, fld) == read(h1, o, fld))
-     ==> Apply0(t0, h0, f) == Apply0(t0, h1, f));
-
-// frame axiom for Apply0
-axiom (forall t0: Ty, h0: Heap, h1: Heap, f: HandleType :: 
-  { $HeapSucc(h0, h1), Apply0(t0, h1, f) } 
-  $HeapSucc(h0, h1)
-       && 
-      $IsGoodHeap(h0)
-       && $IsGoodHeap(h1)
-       && $Is(f, Tclass._System.___hFunc0(t0))
-       && (forall<a> o: ref, fld: Field a :: 
-        o != null && Reads0(t0, h1, f)[$Box(o)] ==> read(h0, o, fld) == read(h1, o, fld))
-     ==> Apply0(t0, h0, f) == Apply0(t0, h1, f));
-
-// empty-reads property for Reads0 
-axiom (forall t0: Ty, heap: Heap, f: HandleType :: 
-  { Reads0(t0, $OneHeap, f), $IsGoodHeap(heap) } { Reads0(t0, heap, f) } 
-  $IsGoodHeap(heap) && $Is(f, Tclass._System.___hFunc0(t0))
-     ==> (Set#Equal(Reads0(t0, $OneHeap, f), Set#Empty(): Set Box)
-       <==> Set#Equal(Reads0(t0, heap, f), Set#Empty(): Set Box)));
-
-// empty-reads property for Requires0
-axiom (forall t0: Ty, heap: Heap, f: HandleType :: 
-  { Requires0(t0, $OneHeap, f), $IsGoodHeap(heap) } { Requires0(t0, heap, f) } 
-  $IsGoodHeap(heap)
-       && $Is(f, Tclass._System.___hFunc0(t0))
-       && Set#Equal(Reads0(t0, $OneHeap, f), Set#Empty(): Set Box)
-     ==> Requires0(t0, $OneHeap, f) == Requires0(t0, heap, f));
-
-axiom (forall f: HandleType, t0: Ty :: 
-  { $Is(f, Tclass._System.___hFunc0(t0)) } 
-  $Is(f, Tclass._System.___hFunc0(t0))
-     <==> (forall h: Heap :: 
-      { Apply0(t0, h, f) } 
-      $IsGoodHeap(h) && Requires0(t0, h, f) ==> $IsBox(Apply0(t0, h, f), t0)));
-
-axiom (forall f: HandleType, t0: Ty, u0: Ty :: 
-  { $Is(f, Tclass._System.___hFunc0(t0)), $Is(f, Tclass._System.___hFunc0(u0)) } 
-  $Is(f, Tclass._System.___hFunc0(t0))
-       && (forall bx: Box :: 
-        { $IsBox(bx, t0) } { $IsBox(bx, u0) } 
-        $IsBox(bx, t0) ==> $IsBox(bx, u0))
-     ==> $Is(f, Tclass._System.___hFunc0(u0)));
-
-axiom (forall f: HandleType, t0: Ty, h: Heap :: 
-  { $IsAlloc(f, Tclass._System.___hFunc0(t0), h) } 
-  $IsGoodHeap(h)
-     ==> ($IsAlloc(f, Tclass._System.___hFunc0(t0), h)
-       <==> Requires0(t0, h, f)
-         ==> (forall r: ref :: 
-          { Reads0(t0, h, f)[$Box(r)] } 
-          r != null && Reads0(t0, h, f)[$Box(r)] ==> read(h, r, alloc))));
-
-axiom (forall f: HandleType, t0: Ty, h: Heap :: 
-  { $IsAlloc(f, Tclass._System.___hFunc0(t0), h) } 
-  $IsGoodHeap(h) && $IsAlloc(f, Tclass._System.___hFunc0(t0), h)
-     ==> 
-    Requires0(t0, h, f)
-     ==> $IsAllocBox(Apply0(t0, h, f), t0, h));
-
-function Tclass._System.___hPartialFunc0(Ty) : Ty;
-
-// Tclass._System.___hPartialFunc0 Tag
-axiom (forall #$R: Ty :: 
-  { Tclass._System.___hPartialFunc0(#$R) } 
-  Tag(Tclass._System.___hPartialFunc0(#$R)) == Tagclass._System.___hPartialFunc0);
-
-const unique Tagclass._System.___hPartialFunc0: TyTag;
-
-// Tclass._System.___hPartialFunc0 injectivity 0
-axiom (forall #$R: Ty :: 
-  { Tclass._System.___hPartialFunc0(#$R) } 
-  Tclass._System.___hPartialFunc0_0(Tclass._System.___hPartialFunc0(#$R)) == #$R);
-
-function Tclass._System.___hPartialFunc0_0(Ty) : Ty;
-
-// Box/unbox axiom for Tclass._System.___hPartialFunc0
-axiom (forall #$R: Ty, bx: Box :: 
-  { $IsBox(bx, Tclass._System.___hPartialFunc0(#$R)) } 
-  $IsBox(bx, Tclass._System.___hPartialFunc0(#$R))
-     ==> $Box($Unbox(bx): HandleType) == bx
-       && $Is($Unbox(bx): HandleType, Tclass._System.___hPartialFunc0(#$R)));
-
-// _System._#PartialFunc0: subset type $Is
-axiom (forall #$R: Ty, f#0: HandleType :: 
-  { $Is(f#0, Tclass._System.___hPartialFunc0(#$R)) } 
-  $Is(f#0, Tclass._System.___hPartialFunc0(#$R))
-     <==> $Is(f#0, Tclass._System.___hFunc0(#$R))
-       && Set#Equal(Reads0(#$R, $OneHeap, f#0), Set#Empty(): Set Box));
-
-// _System._#PartialFunc0: subset type $IsAlloc
-axiom (forall #$R: Ty, f#0: HandleType, $h: Heap :: 
-  { $IsAlloc(f#0, Tclass._System.___hPartialFunc0(#$R), $h) } 
-  $IsAlloc(f#0, Tclass._System.___hPartialFunc0(#$R), $h)
-     <==> $IsAlloc(f#0, Tclass._System.___hFunc0(#$R), $h));
-
-function Tclass._System.___hTotalFunc0(Ty) : Ty;
-
-// Tclass._System.___hTotalFunc0 Tag
-axiom (forall #$R: Ty :: 
-  { Tclass._System.___hTotalFunc0(#$R) } 
-  Tag(Tclass._System.___hTotalFunc0(#$R)) == Tagclass._System.___hTotalFunc0);
-
-const unique Tagclass._System.___hTotalFunc0: TyTag;
-
-// Tclass._System.___hTotalFunc0 injectivity 0
-axiom (forall #$R: Ty :: 
-  { Tclass._System.___hTotalFunc0(#$R) } 
-  Tclass._System.___hTotalFunc0_0(Tclass._System.___hTotalFunc0(#$R)) == #$R);
-
-function Tclass._System.___hTotalFunc0_0(Ty) : Ty;
-
-// Box/unbox axiom for Tclass._System.___hTotalFunc0
-axiom (forall #$R: Ty, bx: Box :: 
-  { $IsBox(bx, Tclass._System.___hTotalFunc0(#$R)) } 
-  $IsBox(bx, Tclass._System.___hTotalFunc0(#$R))
-     ==> $Box($Unbox(bx): HandleType) == bx
-       && $Is($Unbox(bx): HandleType, Tclass._System.___hTotalFunc0(#$R)));
-
-// _System._#TotalFunc0: subset type $Is
-axiom (forall #$R: Ty, f#0: HandleType :: 
-  { $Is(f#0, Tclass._System.___hTotalFunc0(#$R)) } 
-  $Is(f#0, Tclass._System.___hTotalFunc0(#$R))
-     <==> $Is(f#0, Tclass._System.___hPartialFunc0(#$R)) && Requires0(#$R, $OneHeap, f#0));
-
-// _System._#TotalFunc0: subset type $IsAlloc
-axiom (forall #$R: Ty, f#0: HandleType, $h: Heap :: 
-  { $IsAlloc(f#0, Tclass._System.___hTotalFunc0(#$R), $h) } 
-  $IsAlloc(f#0, Tclass._System.___hTotalFunc0(#$R), $h)
-     <==> $IsAlloc(f#0, Tclass._System.___hPartialFunc0(#$R), $h));
-
-function Tclass._System.___hFunc2(Ty, Ty, Ty) : Ty;
-
-// Tclass._System.___hFunc2 Tag
-axiom (forall #$T0: Ty, #$T1: Ty, #$R: Ty :: 
-  { Tclass._System.___hFunc2(#$T0, #$T1, #$R) } 
-  Tag(Tclass._System.___hFunc2(#$T0, #$T1, #$R)) == Tagclass._System.___hFunc2);
-
-const unique Tagclass._System.___hFunc2: TyTag;
-
-// Tclass._System.___hFunc2 injectivity 0
-axiom (forall #$T0: Ty, #$T1: Ty, #$R: Ty :: 
-  { Tclass._System.___hFunc2(#$T0, #$T1, #$R) } 
-  Tclass._System.___hFunc2_0(Tclass._System.___hFunc2(#$T0, #$T1, #$R)) == #$T0);
-
-function Tclass._System.___hFunc2_0(Ty) : Ty;
-
-// Tclass._System.___hFunc2 injectivity 1
-axiom (forall #$T0: Ty, #$T1: Ty, #$R: Ty :: 
-  { Tclass._System.___hFunc2(#$T0, #$T1, #$R) } 
-  Tclass._System.___hFunc2_1(Tclass._System.___hFunc2(#$T0, #$T1, #$R)) == #$T1);
-
-function Tclass._System.___hFunc2_1(Ty) : Ty;
-
-// Tclass._System.___hFunc2 injectivity 2
-axiom (forall #$T0: Ty, #$T1: Ty, #$R: Ty :: 
-  { Tclass._System.___hFunc2(#$T0, #$T1, #$R) } 
-  Tclass._System.___hFunc2_2(Tclass._System.___hFunc2(#$T0, #$T1, #$R)) == #$R);
-
-function Tclass._System.___hFunc2_2(Ty) : Ty;
-
-// Box/unbox axiom for Tclass._System.___hFunc2
-axiom (forall #$T0: Ty, #$T1: Ty, #$R: Ty, bx: Box :: 
-  { $IsBox(bx, Tclass._System.___hFunc2(#$T0, #$T1, #$R)) } 
-  $IsBox(bx, Tclass._System.___hFunc2(#$T0, #$T1, #$R))
-     ==> $Box($Unbox(bx): HandleType) == bx
-       && $Is($Unbox(bx): HandleType, Tclass._System.___hFunc2(#$T0, #$T1, #$R)));
-
-function Handle2([Heap,Box,Box]Box, [Heap,Box,Box]bool, [Heap,Box,Box]Set Box) : HandleType;
-
-function Apply2(Ty, Ty, Ty, Heap, HandleType, Box, Box) : Box;
-
-function Requires2(Ty, Ty, Ty, Heap, HandleType, Box, Box) : bool;
-
-function Reads2(Ty, Ty, Ty, Heap, HandleType, Box, Box) : Set Box;
-
-axiom (forall t0: Ty, 
-    t1: Ty, 
-    t2: Ty, 
-    heap: Heap, 
-    h: [Heap,Box,Box]Box, 
-    r: [Heap,Box,Box]bool, 
-    rd: [Heap,Box,Box]Set Box, 
-    bx0: Box, 
-    bx1: Box :: 
-  { Apply2(t0, t1, t2, heap, Handle2(h, r, rd), bx0, bx1) } 
-  Apply2(t0, t1, t2, heap, Handle2(h, r, rd), bx0, bx1) == h[heap, bx0, bx1]);
-
-axiom (forall t0: Ty, 
-    t1: Ty, 
-    t2: Ty, 
-    heap: Heap, 
-    h: [Heap,Box,Box]Box, 
-    r: [Heap,Box,Box]bool, 
-    rd: [Heap,Box,Box]Set Box, 
-    bx0: Box, 
-    bx1: Box :: 
-  { Requires2(t0, t1, t2, heap, Handle2(h, r, rd), bx0, bx1) } 
-  r[heap, bx0, bx1] ==> Requires2(t0, t1, t2, heap, Handle2(h, r, rd), bx0, bx1));
-
-axiom (forall t0: Ty, 
-    t1: Ty, 
-    t2: Ty, 
-    heap: Heap, 
-    h: [Heap,Box,Box]Box, 
-    r: [Heap,Box,Box]bool, 
-    rd: [Heap,Box,Box]Set Box, 
-    bx0: Box, 
-    bx1: Box, 
-    bx: Box :: 
-  { Reads2(t0, t1, t2, heap, Handle2(h, r, rd), bx0, bx1)[bx] } 
-  Reads2(t0, t1, t2, heap, Handle2(h, r, rd), bx0, bx1)[bx]
-     == rd[heap, bx0, bx1][bx]);
-
-function {:inline} Requires2#canCall(t0: Ty, t1: Ty, t2: Ty, heap: Heap, f: HandleType, bx0: Box, bx1: Box) : bool
-{
-  true
-}
-
-function {:inline} Reads2#canCall(t0: Ty, t1: Ty, t2: Ty, heap: Heap, f: HandleType, bx0: Box, bx1: Box) : bool
-{
-  true
-}
-
-// frame axiom for Reads2
-axiom (forall t0: Ty, t1: Ty, t2: Ty, h0: Heap, h1: Heap, f: HandleType, bx0: Box, bx1: Box :: 
-  { $HeapSucc(h0, h1), Reads2(t0, t1, t2, h1, f, bx0, bx1) } 
-  $HeapSucc(h0, h1)
-       && 
-      $IsGoodHeap(h0)
-       && $IsGoodHeap(h1)
-       && 
-      $IsBox(bx0, t0)
-       && $IsBox(bx1, t1)
-       && $Is(f, Tclass._System.___hFunc2(t0, t1, t2))
-       && (forall<a> o: ref, fld: Field a :: 
-        o != null && Reads2(t0, t1, t2, h0, f, bx0, bx1)[$Box(o)]
-           ==> read(h0, o, fld) == read(h1, o, fld))
-     ==> Reads2(t0, t1, t2, h0, f, bx0, bx1) == Reads2(t0, t1, t2, h1, f, bx0, bx1));
-
-// frame axiom for Reads2
-axiom (forall t0: Ty, t1: Ty, t2: Ty, h0: Heap, h1: Heap, f: HandleType, bx0: Box, bx1: Box :: 
-  { $HeapSucc(h0, h1), Reads2(t0, t1, t2, h1, f, bx0, bx1) } 
-  $HeapSucc(h0, h1)
-       && 
-      $IsGoodHeap(h0)
-       && $IsGoodHeap(h1)
-       && 
-      $IsBox(bx0, t0)
-       && $IsBox(bx1, t1)
-       && $Is(f, Tclass._System.___hFunc2(t0, t1, t2))
-       && (forall<a> o: ref, fld: Field a :: 
-        o != null && Reads2(t0, t1, t2, h1, f, bx0, bx1)[$Box(o)]
-           ==> read(h0, o, fld) == read(h1, o, fld))
-     ==> Reads2(t0, t1, t2, h0, f, bx0, bx1) == Reads2(t0, t1, t2, h1, f, bx0, bx1));
-
-// frame axiom for Requires2
-axiom (forall t0: Ty, t1: Ty, t2: Ty, h0: Heap, h1: Heap, f: HandleType, bx0: Box, bx1: Box :: 
-  { $HeapSucc(h0, h1), Requires2(t0, t1, t2, h1, f, bx0, bx1) } 
-  $HeapSucc(h0, h1)
-       && 
-      $IsGoodHeap(h0)
-       && $IsGoodHeap(h1)
-       && 
-      $IsBox(bx0, t0)
-       && $IsBox(bx1, t1)
-       && $Is(f, Tclass._System.___hFunc2(t0, t1, t2))
-       && (forall<a> o: ref, fld: Field a :: 
-        o != null && Reads2(t0, t1, t2, h0, f, bx0, bx1)[$Box(o)]
-           ==> read(h0, o, fld) == read(h1, o, fld))
-     ==> Requires2(t0, t1, t2, h0, f, bx0, bx1) == Requires2(t0, t1, t2, h1, f, bx0, bx1));
-
-// frame axiom for Requires2
-axiom (forall t0: Ty, t1: Ty, t2: Ty, h0: Heap, h1: Heap, f: HandleType, bx0: Box, bx1: Box :: 
-  { $HeapSucc(h0, h1), Requires2(t0, t1, t2, h1, f, bx0, bx1) } 
-  $HeapSucc(h0, h1)
-       && 
-      $IsGoodHeap(h0)
-       && $IsGoodHeap(h1)
-       && 
-      $IsBox(bx0, t0)
-       && $IsBox(bx1, t1)
-       && $Is(f, Tclass._System.___hFunc2(t0, t1, t2))
-       && (forall<a> o: ref, fld: Field a :: 
-        o != null && Reads2(t0, t1, t2, h1, f, bx0, bx1)[$Box(o)]
-           ==> read(h0, o, fld) == read(h1, o, fld))
-     ==> Requires2(t0, t1, t2, h0, f, bx0, bx1) == Requires2(t0, t1, t2, h1, f, bx0, bx1));
-
-// frame axiom for Apply2
-axiom (forall t0: Ty, t1: Ty, t2: Ty, h0: Heap, h1: Heap, f: HandleType, bx0: Box, bx1: Box :: 
-  { $HeapSucc(h0, h1), Apply2(t0, t1, t2, h1, f, bx0, bx1) } 
-  $HeapSucc(h0, h1)
-       && 
-      $IsGoodHeap(h0)
-       && $IsGoodHeap(h1)
-       && 
-      $IsBox(bx0, t0)
-       && $IsBox(bx1, t1)
-       && $Is(f, Tclass._System.___hFunc2(t0, t1, t2))
-       && (forall<a> o: ref, fld: Field a :: 
-        o != null && Reads2(t0, t1, t2, h0, f, bx0, bx1)[$Box(o)]
-           ==> read(h0, o, fld) == read(h1, o, fld))
-     ==> Apply2(t0, t1, t2, h0, f, bx0, bx1) == Apply2(t0, t1, t2, h1, f, bx0, bx1));
-
-// frame axiom for Apply2
-axiom (forall t0: Ty, t1: Ty, t2: Ty, h0: Heap, h1: Heap, f: HandleType, bx0: Box, bx1: Box :: 
-  { $HeapSucc(h0, h1), Apply2(t0, t1, t2, h1, f, bx0, bx1) } 
-  $HeapSucc(h0, h1)
-       && 
-      $IsGoodHeap(h0)
-       && $IsGoodHeap(h1)
-       && 
-      $IsBox(bx0, t0)
-       && $IsBox(bx1, t1)
-       && $Is(f, Tclass._System.___hFunc2(t0, t1, t2))
-       && (forall<a> o: ref, fld: Field a :: 
-        o != null && Reads2(t0, t1, t2, h1, f, bx0, bx1)[$Box(o)]
-           ==> read(h0, o, fld) == read(h1, o, fld))
-     ==> Apply2(t0, t1, t2, h0, f, bx0, bx1) == Apply2(t0, t1, t2, h1, f, bx0, bx1));
-
-// empty-reads property for Reads2 
-axiom (forall t0: Ty, t1: Ty, t2: Ty, heap: Heap, f: HandleType, bx0: Box, bx1: Box :: 
-  { Reads2(t0, t1, t2, $OneHeap, f, bx0, bx1), $IsGoodHeap(heap) } 
-    { Reads2(t0, t1, t2, heap, f, bx0, bx1) } 
-  $IsGoodHeap(heap)
-       && 
-      $IsBox(bx0, t0)
-       && $IsBox(bx1, t1)
-       && $Is(f, Tclass._System.___hFunc2(t0, t1, t2))
-     ==> (Set#Equal(Reads2(t0, t1, t2, $OneHeap, f, bx0, bx1), Set#Empty(): Set Box)
-       <==> Set#Equal(Reads2(t0, t1, t2, heap, f, bx0, bx1), Set#Empty(): Set Box)));
-
-// empty-reads property for Requires2
-axiom (forall t0: Ty, t1: Ty, t2: Ty, heap: Heap, f: HandleType, bx0: Box, bx1: Box :: 
-  { Requires2(t0, t1, t2, $OneHeap, f, bx0, bx1), $IsGoodHeap(heap) } 
-    { Requires2(t0, t1, t2, heap, f, bx0, bx1) } 
-  $IsGoodHeap(heap)
-       && 
-      $IsBox(bx0, t0)
-       && $IsBox(bx1, t1)
-       && $Is(f, Tclass._System.___hFunc2(t0, t1, t2))
-       && Set#Equal(Reads2(t0, t1, t2, $OneHeap, f, bx0, bx1), Set#Empty(): Set Box)
-     ==> Requires2(t0, t1, t2, $OneHeap, f, bx0, bx1)
-       == Requires2(t0, t1, t2, heap, f, bx0, bx1));
-
-axiom (forall f: HandleType, t0: Ty, t1: Ty, t2: Ty :: 
-  { $Is(f, Tclass._System.___hFunc2(t0, t1, t2)) } 
-  $Is(f, Tclass._System.___hFunc2(t0, t1, t2))
-     <==> (forall h: Heap, bx0: Box, bx1: Box :: 
-      { Apply2(t0, t1, t2, h, f, bx0, bx1) } 
-      $IsGoodHeap(h)
-           && 
-          $IsBox(bx0, t0)
-           && $IsBox(bx1, t1)
-           && Requires2(t0, t1, t2, h, f, bx0, bx1)
-         ==> $IsBox(Apply2(t0, t1, t2, h, f, bx0, bx1), t2)));
-
-axiom (forall f: HandleType, t0: Ty, t1: Ty, t2: Ty, u0: Ty, u1: Ty, u2: Ty :: 
-  { $Is(f, Tclass._System.___hFunc2(t0, t1, t2)), $Is(f, Tclass._System.___hFunc2(u0, u1, u2)) } 
-  $Is(f, Tclass._System.___hFunc2(t0, t1, t2))
-       && (forall bx: Box :: 
-        { $IsBox(bx, u0) } { $IsBox(bx, t0) } 
-        $IsBox(bx, u0) ==> $IsBox(bx, t0))
-       && (forall bx: Box :: 
-        { $IsBox(bx, u1) } { $IsBox(bx, t1) } 
-        $IsBox(bx, u1) ==> $IsBox(bx, t1))
-       && (forall bx: Box :: 
-        { $IsBox(bx, t2) } { $IsBox(bx, u2) } 
-        $IsBox(bx, t2) ==> $IsBox(bx, u2))
-     ==> $Is(f, Tclass._System.___hFunc2(u0, u1, u2)));
-
-axiom (forall f: HandleType, t0: Ty, t1: Ty, t2: Ty, h: Heap :: 
-  { $IsAlloc(f, Tclass._System.___hFunc2(t0, t1, t2), h) } 
-  $IsGoodHeap(h)
-     ==> ($IsAlloc(f, Tclass._System.___hFunc2(t0, t1, t2), h)
-       <==> (forall bx0: Box, bx1: Box :: 
-        { Apply2(t0, t1, t2, h, f, bx0, bx1) } { Reads2(t0, t1, t2, h, f, bx0, bx1) } 
-        $IsBox(bx0, t0)
-             && $IsAllocBox(bx0, t0, h)
-             && 
-            $IsBox(bx1, t1)
-             && $IsAllocBox(bx1, t1, h)
-             && Requires2(t0, t1, t2, h, f, bx0, bx1)
-           ==> (forall r: ref :: 
-            { Reads2(t0, t1, t2, h, f, bx0, bx1)[$Box(r)] } 
-            r != null && Reads2(t0, t1, t2, h, f, bx0, bx1)[$Box(r)] ==> read(h, r, alloc)))));
-
-axiom (forall f: HandleType, t0: Ty, t1: Ty, t2: Ty, h: Heap :: 
-  { $IsAlloc(f, Tclass._System.___hFunc2(t0, t1, t2), h) } 
-  $IsGoodHeap(h) && $IsAlloc(f, Tclass._System.___hFunc2(t0, t1, t2), h)
-     ==> (forall bx0: Box, bx1: Box :: 
-      { Apply2(t0, t1, t2, h, f, bx0, bx1) } 
-      $IsAllocBox(bx0, t0, h)
-           && $IsAllocBox(bx1, t1, h)
-           && Requires2(t0, t1, t2, h, f, bx0, bx1)
-         ==> $IsAllocBox(Apply2(t0, t1, t2, h, f, bx0, bx1), t2, h)));
-
-function Tclass._System.___hPartialFunc2(Ty, Ty, Ty) : Ty;
-
-// Tclass._System.___hPartialFunc2 Tag
-axiom (forall #$T0: Ty, #$T1: Ty, #$R: Ty :: 
-  { Tclass._System.___hPartialFunc2(#$T0, #$T1, #$R) } 
-  Tag(Tclass._System.___hPartialFunc2(#$T0, #$T1, #$R))
-     == Tagclass._System.___hPartialFunc2);
-
-const unique Tagclass._System.___hPartialFunc2: TyTag;
-
-// Tclass._System.___hPartialFunc2 injectivity 0
-axiom (forall #$T0: Ty, #$T1: Ty, #$R: Ty :: 
-  { Tclass._System.___hPartialFunc2(#$T0, #$T1, #$R) } 
-  Tclass._System.___hPartialFunc2_0(Tclass._System.___hPartialFunc2(#$T0, #$T1, #$R))
-     == #$T0);
-
-function Tclass._System.___hPartialFunc2_0(Ty) : Ty;
-
-// Tclass._System.___hPartialFunc2 injectivity 1
-axiom (forall #$T0: Ty, #$T1: Ty, #$R: Ty :: 
-  { Tclass._System.___hPartialFunc2(#$T0, #$T1, #$R) } 
-  Tclass._System.___hPartialFunc2_1(Tclass._System.___hPartialFunc2(#$T0, #$T1, #$R))
-     == #$T1);
-
-function Tclass._System.___hPartialFunc2_1(Ty) : Ty;
-
-// Tclass._System.___hPartialFunc2 injectivity 2
-axiom (forall #$T0: Ty, #$T1: Ty, #$R: Ty :: 
-  { Tclass._System.___hPartialFunc2(#$T0, #$T1, #$R) } 
-  Tclass._System.___hPartialFunc2_2(Tclass._System.___hPartialFunc2(#$T0, #$T1, #$R))
-     == #$R);
-
-function Tclass._System.___hPartialFunc2_2(Ty) : Ty;
-
-// Box/unbox axiom for Tclass._System.___hPartialFunc2
-axiom (forall #$T0: Ty, #$T1: Ty, #$R: Ty, bx: Box :: 
-  { $IsBox(bx, Tclass._System.___hPartialFunc2(#$T0, #$T1, #$R)) } 
-  $IsBox(bx, Tclass._System.___hPartialFunc2(#$T0, #$T1, #$R))
-     ==> $Box($Unbox(bx): HandleType) == bx
-       && $Is($Unbox(bx): HandleType, Tclass._System.___hPartialFunc2(#$T0, #$T1, #$R)));
-
-// _System._#PartialFunc2: subset type $Is
-axiom (forall #$T0: Ty, #$T1: Ty, #$R: Ty, f#0: HandleType :: 
-  { $Is(f#0, Tclass._System.___hPartialFunc2(#$T0, #$T1, #$R)) } 
-  $Is(f#0, Tclass._System.___hPartialFunc2(#$T0, #$T1, #$R))
-     <==> $Is(f#0, Tclass._System.___hFunc2(#$T0, #$T1, #$R))
-       && (forall x0#0: Box, x1#0: Box :: 
-        $IsBox(x0#0, #$T0) && $IsBox(x1#0, #$T1)
-           ==> Set#Equal(Reads2(#$T0, #$T1, #$R, $OneHeap, f#0, x0#0, x1#0), Set#Empty(): Set Box)));
-
-// _System._#PartialFunc2: subset type $IsAlloc
-axiom (forall #$T0: Ty, #$T1: Ty, #$R: Ty, f#0: HandleType, $h: Heap :: 
-  { $IsAlloc(f#0, Tclass._System.___hPartialFunc2(#$T0, #$T1, #$R), $h) } 
-  $IsAlloc(f#0, Tclass._System.___hPartialFunc2(#$T0, #$T1, #$R), $h)
-     <==> $IsAlloc(f#0, Tclass._System.___hFunc2(#$T0, #$T1, #$R), $h));
-
-function Tclass._System.___hTotalFunc2(Ty, Ty, Ty) : Ty;
-
-// Tclass._System.___hTotalFunc2 Tag
-axiom (forall #$T0: Ty, #$T1: Ty, #$R: Ty :: 
-  { Tclass._System.___hTotalFunc2(#$T0, #$T1, #$R) } 
-  Tag(Tclass._System.___hTotalFunc2(#$T0, #$T1, #$R))
-     == Tagclass._System.___hTotalFunc2);
-
-const unique Tagclass._System.___hTotalFunc2: TyTag;
-
-// Tclass._System.___hTotalFunc2 injectivity 0
-axiom (forall #$T0: Ty, #$T1: Ty, #$R: Ty :: 
-  { Tclass._System.___hTotalFunc2(#$T0, #$T1, #$R) } 
-  Tclass._System.___hTotalFunc2_0(Tclass._System.___hTotalFunc2(#$T0, #$T1, #$R))
-     == #$T0);
-
-function Tclass._System.___hTotalFunc2_0(Ty) : Ty;
-
-// Tclass._System.___hTotalFunc2 injectivity 1
-axiom (forall #$T0: Ty, #$T1: Ty, #$R: Ty :: 
-  { Tclass._System.___hTotalFunc2(#$T0, #$T1, #$R) } 
-  Tclass._System.___hTotalFunc2_1(Tclass._System.___hTotalFunc2(#$T0, #$T1, #$R))
-     == #$T1);
-
-function Tclass._System.___hTotalFunc2_1(Ty) : Ty;
-
-// Tclass._System.___hTotalFunc2 injectivity 2
-axiom (forall #$T0: Ty, #$T1: Ty, #$R: Ty :: 
-  { Tclass._System.___hTotalFunc2(#$T0, #$T1, #$R) } 
-  Tclass._System.___hTotalFunc2_2(Tclass._System.___hTotalFunc2(#$T0, #$T1, #$R))
-     == #$R);
-
-function Tclass._System.___hTotalFunc2_2(Ty) : Ty;
-
-// Box/unbox axiom for Tclass._System.___hTotalFunc2
-axiom (forall #$T0: Ty, #$T1: Ty, #$R: Ty, bx: Box :: 
-  { $IsBox(bx, Tclass._System.___hTotalFunc2(#$T0, #$T1, #$R)) } 
-  $IsBox(bx, Tclass._System.___hTotalFunc2(#$T0, #$T1, #$R))
-     ==> $Box($Unbox(bx): HandleType) == bx
-       && $Is($Unbox(bx): HandleType, Tclass._System.___hTotalFunc2(#$T0, #$T1, #$R)));
-
-// _System._#TotalFunc2: subset type $Is
-axiom (forall #$T0: Ty, #$T1: Ty, #$R: Ty, f#0: HandleType :: 
-  { $Is(f#0, Tclass._System.___hTotalFunc2(#$T0, #$T1, #$R)) } 
-  $Is(f#0, Tclass._System.___hTotalFunc2(#$T0, #$T1, #$R))
-     <==> $Is(f#0, Tclass._System.___hPartialFunc2(#$T0, #$T1, #$R))
-       && (forall x0#0: Box, x1#0: Box :: 
-        $IsBox(x0#0, #$T0) && $IsBox(x1#0, #$T1)
-           ==> Requires2(#$T0, #$T1, #$R, $OneHeap, f#0, x0#0, x1#0)));
-
-// _System._#TotalFunc2: subset type $IsAlloc
-axiom (forall #$T0: Ty, #$T1: Ty, #$R: Ty, f#0: HandleType, $h: Heap :: 
-  { $IsAlloc(f#0, Tclass._System.___hTotalFunc2(#$T0, #$T1, #$R), $h) } 
-  $IsAlloc(f#0, Tclass._System.___hTotalFunc2(#$T0, #$T1, #$R), $h)
-     <==> $IsAlloc(f#0, Tclass._System.___hPartialFunc2(#$T0, #$T1, #$R), $h));
-
 function Tclass._System.___hFunc1(Ty, Ty) : Ty;
+
+const unique Tagclass._System.___hFunc1: TyTag;
 
 // Tclass._System.___hFunc1 Tag
 axiom (forall #$T0: Ty, #$R: Ty :: 
   { Tclass._System.___hFunc1(#$T0, #$R) } 
-  Tag(Tclass._System.___hFunc1(#$T0, #$R)) == Tagclass._System.___hFunc1);
+  Tag(Tclass._System.___hFunc1(#$T0, #$R)) == Tagclass._System.___hFunc1
+     && TagFamily(Tclass._System.___hFunc1(#$T0, #$R)) == tytagFamily$_#Func1);
 
-const unique Tagclass._System.___hFunc1: TyTag;
+function Tclass._System.___hFunc1_0(Ty) : Ty;
 
 // Tclass._System.___hFunc1 injectivity 0
 axiom (forall #$T0: Ty, #$R: Ty :: 
   { Tclass._System.___hFunc1(#$T0, #$R) } 
   Tclass._System.___hFunc1_0(Tclass._System.___hFunc1(#$T0, #$R)) == #$T0);
 
-function Tclass._System.___hFunc1_0(Ty) : Ty;
+function Tclass._System.___hFunc1_1(Ty) : Ty;
 
 // Tclass._System.___hFunc1 injectivity 1
 axiom (forall #$T0: Ty, #$R: Ty :: 
   { Tclass._System.___hFunc1(#$T0, #$R) } 
   Tclass._System.___hFunc1_1(Tclass._System.___hFunc1(#$T0, #$R)) == #$R);
-
-function Tclass._System.___hFunc1_1(Ty) : Ty;
 
 // Box/unbox axiom for Tclass._System.___hFunc1
 axiom (forall #$T0: Ty, #$R: Ty, bx: Box :: 
@@ -2475,20 +2112,18 @@ axiom (forall #$T0: Ty, #$R: Ty, bx: Box ::
      ==> $Box($Unbox(bx): HandleType) == bx
        && $Is($Unbox(bx): HandleType, Tclass._System.___hFunc1(#$T0, #$R)));
 
-function Handle1([Heap,Box]Box, [Heap,Box]bool, [Heap,Box]Set Box) : HandleType;
-
-function Apply1(Ty, Ty, Heap, HandleType, Box) : Box;
+function Handle1([Heap,Box]Box, [Heap,Box]bool, [Heap,Box]Set) : HandleType;
 
 function Requires1(Ty, Ty, Heap, HandleType, Box) : bool;
 
-function Reads1(Ty, Ty, Heap, HandleType, Box) : Set Box;
+function Reads1(Ty, Ty, Heap, HandleType, Box) : Set;
 
 axiom (forall t0: Ty, 
     t1: Ty, 
     heap: Heap, 
     h: [Heap,Box]Box, 
     r: [Heap,Box]bool, 
-    rd: [Heap,Box]Set Box, 
+    rd: [Heap,Box]Set, 
     bx0: Box :: 
   { Apply1(t0, t1, heap, Handle1(h, r, rd), bx0) } 
   Apply1(t0, t1, heap, Handle1(h, r, rd), bx0) == h[heap, bx0]);
@@ -2498,7 +2133,7 @@ axiom (forall t0: Ty,
     heap: Heap, 
     h: [Heap,Box]Box, 
     r: [Heap,Box]bool, 
-    rd: [Heap,Box]Set Box, 
+    rd: [Heap,Box]Set, 
     bx0: Box :: 
   { Requires1(t0, t1, heap, Handle1(h, r, rd), bx0) } 
   r[heap, bx0] ==> Requires1(t0, t1, heap, Handle1(h, r, rd), bx0));
@@ -2508,11 +2143,12 @@ axiom (forall t0: Ty,
     heap: Heap, 
     h: [Heap,Box]Box, 
     r: [Heap,Box]bool, 
-    rd: [Heap,Box]Set Box, 
+    rd: [Heap,Box]Set, 
     bx0: Box, 
     bx: Box :: 
-  { Reads1(t0, t1, heap, Handle1(h, r, rd), bx0)[bx] } 
-  Reads1(t0, t1, heap, Handle1(h, r, rd), bx0)[bx] == rd[heap, bx0][bx]);
+  { Set#IsMember(Reads1(t0, t1, heap, Handle1(h, r, rd), bx0), bx) } 
+  Set#IsMember(Reads1(t0, t1, heap, Handle1(h, r, rd), bx0), bx)
+     == Set#IsMember(rd[heap, bx0], bx));
 
 function {:inline} Requires1#canCall(t0: Ty, t1: Ty, heap: Heap, f: HandleType, bx0: Box) : bool
 {
@@ -2534,8 +2170,8 @@ axiom (forall t0: Ty, t1: Ty, h0: Heap, h1: Heap, f: HandleType, bx0: Box ::
        && 
       $IsBox(bx0, t0)
        && $Is(f, Tclass._System.___hFunc1(t0, t1))
-       && (forall<a> o: ref, fld: Field a :: 
-        o != null && Reads1(t0, t1, h0, f, bx0)[$Box(o)]
+       && (forall o: ref, fld: Field :: 
+        o != null && Set#IsMember(Reads1(t0, t1, h0, f, bx0), $Box(o))
            ==> read(h0, o, fld) == read(h1, o, fld))
      ==> Reads1(t0, t1, h0, f, bx0) == Reads1(t0, t1, h1, f, bx0));
 
@@ -2549,8 +2185,8 @@ axiom (forall t0: Ty, t1: Ty, h0: Heap, h1: Heap, f: HandleType, bx0: Box ::
        && 
       $IsBox(bx0, t0)
        && $Is(f, Tclass._System.___hFunc1(t0, t1))
-       && (forall<a> o: ref, fld: Field a :: 
-        o != null && Reads1(t0, t1, h1, f, bx0)[$Box(o)]
+       && (forall o: ref, fld: Field :: 
+        o != null && Set#IsMember(Reads1(t0, t1, h1, f, bx0), $Box(o))
            ==> read(h0, o, fld) == read(h1, o, fld))
      ==> Reads1(t0, t1, h0, f, bx0) == Reads1(t0, t1, h1, f, bx0));
 
@@ -2564,8 +2200,8 @@ axiom (forall t0: Ty, t1: Ty, h0: Heap, h1: Heap, f: HandleType, bx0: Box ::
        && 
       $IsBox(bx0, t0)
        && $Is(f, Tclass._System.___hFunc1(t0, t1))
-       && (forall<a> o: ref, fld: Field a :: 
-        o != null && Reads1(t0, t1, h0, f, bx0)[$Box(o)]
+       && (forall o: ref, fld: Field :: 
+        o != null && Set#IsMember(Reads1(t0, t1, h0, f, bx0), $Box(o))
            ==> read(h0, o, fld) == read(h1, o, fld))
      ==> Requires1(t0, t1, h0, f, bx0) == Requires1(t0, t1, h1, f, bx0));
 
@@ -2579,8 +2215,8 @@ axiom (forall t0: Ty, t1: Ty, h0: Heap, h1: Heap, f: HandleType, bx0: Box ::
        && 
       $IsBox(bx0, t0)
        && $Is(f, Tclass._System.___hFunc1(t0, t1))
-       && (forall<a> o: ref, fld: Field a :: 
-        o != null && Reads1(t0, t1, h1, f, bx0)[$Box(o)]
+       && (forall o: ref, fld: Field :: 
+        o != null && Set#IsMember(Reads1(t0, t1, h1, f, bx0), $Box(o))
            ==> read(h0, o, fld) == read(h1, o, fld))
      ==> Requires1(t0, t1, h0, f, bx0) == Requires1(t0, t1, h1, f, bx0));
 
@@ -2594,8 +2230,8 @@ axiom (forall t0: Ty, t1: Ty, h0: Heap, h1: Heap, f: HandleType, bx0: Box ::
        && 
       $IsBox(bx0, t0)
        && $Is(f, Tclass._System.___hFunc1(t0, t1))
-       && (forall<a> o: ref, fld: Field a :: 
-        o != null && Reads1(t0, t1, h0, f, bx0)[$Box(o)]
+       && (forall o: ref, fld: Field :: 
+        o != null && Set#IsMember(Reads1(t0, t1, h0, f, bx0), $Box(o))
            ==> read(h0, o, fld) == read(h1, o, fld))
      ==> Apply1(t0, t1, h0, f, bx0) == Apply1(t0, t1, h1, f, bx0));
 
@@ -2609,8 +2245,8 @@ axiom (forall t0: Ty, t1: Ty, h0: Heap, h1: Heap, f: HandleType, bx0: Box ::
        && 
       $IsBox(bx0, t0)
        && $Is(f, Tclass._System.___hFunc1(t0, t1))
-       && (forall<a> o: ref, fld: Field a :: 
-        o != null && Reads1(t0, t1, h1, f, bx0)[$Box(o)]
+       && (forall o: ref, fld: Field :: 
+        o != null && Set#IsMember(Reads1(t0, t1, h1, f, bx0), $Box(o))
            ==> read(h0, o, fld) == read(h1, o, fld))
      ==> Apply1(t0, t1, h0, f, bx0) == Apply1(t0, t1, h1, f, bx0));
 
@@ -2619,8 +2255,8 @@ axiom (forall t0: Ty, t1: Ty, heap: Heap, f: HandleType, bx0: Box ::
   { Reads1(t0, t1, $OneHeap, f, bx0), $IsGoodHeap(heap) } 
     { Reads1(t0, t1, heap, f, bx0) } 
   $IsGoodHeap(heap) && $IsBox(bx0, t0) && $Is(f, Tclass._System.___hFunc1(t0, t1))
-     ==> (Set#Equal(Reads1(t0, t1, $OneHeap, f, bx0), Set#Empty(): Set Box)
-       <==> Set#Equal(Reads1(t0, t1, heap, f, bx0), Set#Empty(): Set Box)));
+     ==> (Set#Equal(Reads1(t0, t1, $OneHeap, f, bx0), Set#Empty(): Set)
+       <==> Set#Equal(Reads1(t0, t1, heap, f, bx0), Set#Empty(): Set)));
 
 // empty-reads property for Requires1
 axiom (forall t0: Ty, t1: Ty, heap: Heap, f: HandleType, bx0: Box :: 
@@ -2630,7 +2266,7 @@ axiom (forall t0: Ty, t1: Ty, heap: Heap, f: HandleType, bx0: Box ::
        && 
       $IsBox(bx0, t0)
        && $Is(f, Tclass._System.___hFunc1(t0, t1))
-       && Set#Equal(Reads1(t0, t1, $OneHeap, f, bx0), Set#Empty(): Set Box)
+       && Set#Equal(Reads1(t0, t1, $OneHeap, f, bx0), Set#Empty(): Set)
      ==> Requires1(t0, t1, $OneHeap, f, bx0) == Requires1(t0, t1, heap, f, bx0));
 
 axiom (forall f: HandleType, t0: Ty, t1: Ty :: 
@@ -2660,8 +2296,9 @@ axiom (forall f: HandleType, t0: Ty, t1: Ty, h: Heap ::
         { Apply1(t0, t1, h, f, bx0) } { Reads1(t0, t1, h, f, bx0) } 
         $IsBox(bx0, t0) && $IsAllocBox(bx0, t0, h) && Requires1(t0, t1, h, f, bx0)
            ==> (forall r: ref :: 
-            { Reads1(t0, t1, h, f, bx0)[$Box(r)] } 
-            r != null && Reads1(t0, t1, h, f, bx0)[$Box(r)] ==> read(h, r, alloc)))));
+            { Set#IsMember(Reads1(t0, t1, h, f, bx0), $Box(r)) } 
+            r != null && Set#IsMember(Reads1(t0, t1, h, f, bx0), $Box(r))
+               ==> $Unbox(read(h, r, alloc)): bool))));
 
 axiom (forall f: HandleType, t0: Ty, t1: Ty, h: Heap :: 
   { $IsAlloc(f, Tclass._System.___hFunc1(t0, t1), h) } 
@@ -2673,13 +2310,17 @@ axiom (forall f: HandleType, t0: Ty, t1: Ty, h: Heap ::
 
 function Tclass._System.___hPartialFunc1(Ty, Ty) : Ty;
 
+const unique Tagclass._System.___hPartialFunc1: TyTag;
+
 // Tclass._System.___hPartialFunc1 Tag
 axiom (forall #$T0: Ty, #$R: Ty :: 
   { Tclass._System.___hPartialFunc1(#$T0, #$R) } 
   Tag(Tclass._System.___hPartialFunc1(#$T0, #$R))
-     == Tagclass._System.___hPartialFunc1);
+       == Tagclass._System.___hPartialFunc1
+     && TagFamily(Tclass._System.___hPartialFunc1(#$T0, #$R))
+       == tytagFamily$_#PartialFunc1);
 
-const unique Tagclass._System.___hPartialFunc1: TyTag;
+function Tclass._System.___hPartialFunc1_0(Ty) : Ty;
 
 // Tclass._System.___hPartialFunc1 injectivity 0
 axiom (forall #$T0: Ty, #$R: Ty :: 
@@ -2687,15 +2328,13 @@ axiom (forall #$T0: Ty, #$R: Ty ::
   Tclass._System.___hPartialFunc1_0(Tclass._System.___hPartialFunc1(#$T0, #$R))
      == #$T0);
 
-function Tclass._System.___hPartialFunc1_0(Ty) : Ty;
+function Tclass._System.___hPartialFunc1_1(Ty) : Ty;
 
 // Tclass._System.___hPartialFunc1 injectivity 1
 axiom (forall #$T0: Ty, #$R: Ty :: 
   { Tclass._System.___hPartialFunc1(#$T0, #$R) } 
   Tclass._System.___hPartialFunc1_1(Tclass._System.___hPartialFunc1(#$T0, #$R))
      == #$R);
-
-function Tclass._System.___hPartialFunc1_1(Ty) : Ty;
 
 // Box/unbox axiom for Tclass._System.___hPartialFunc1
 axiom (forall #$T0: Ty, #$R: Ty, bx: Box :: 
@@ -2704,16 +2343,16 @@ axiom (forall #$T0: Ty, #$R: Ty, bx: Box ::
      ==> $Box($Unbox(bx): HandleType) == bx
        && $Is($Unbox(bx): HandleType, Tclass._System.___hPartialFunc1(#$T0, #$R)));
 
-// _System._#PartialFunc1: subset type $Is
+// $Is axiom for subset type _System._#PartialFunc1
 axiom (forall #$T0: Ty, #$R: Ty, f#0: HandleType :: 
   { $Is(f#0, Tclass._System.___hPartialFunc1(#$T0, #$R)) } 
   $Is(f#0, Tclass._System.___hPartialFunc1(#$T0, #$R))
      <==> $Is(f#0, Tclass._System.___hFunc1(#$T0, #$R))
        && (forall x0#0: Box :: 
         $IsBox(x0#0, #$T0)
-           ==> Set#Equal(Reads1(#$T0, #$R, $OneHeap, f#0, x0#0), Set#Empty(): Set Box)));
+           ==> Set#Equal(Reads1(#$T0, #$R, $OneHeap, f#0, x0#0), Set#Empty(): Set)));
 
-// _System._#PartialFunc1: subset type $IsAlloc
+// $IsAlloc axiom for subset type _System._#PartialFunc1
 axiom (forall #$T0: Ty, #$R: Ty, f#0: HandleType, $h: Heap :: 
   { $IsAlloc(f#0, Tclass._System.___hPartialFunc1(#$T0, #$R), $h) } 
   $IsAlloc(f#0, Tclass._System.___hPartialFunc1(#$T0, #$R), $h)
@@ -2721,12 +2360,15 @@ axiom (forall #$T0: Ty, #$R: Ty, f#0: HandleType, $h: Heap ::
 
 function Tclass._System.___hTotalFunc1(Ty, Ty) : Ty;
 
+const unique Tagclass._System.___hTotalFunc1: TyTag;
+
 // Tclass._System.___hTotalFunc1 Tag
 axiom (forall #$T0: Ty, #$R: Ty :: 
   { Tclass._System.___hTotalFunc1(#$T0, #$R) } 
-  Tag(Tclass._System.___hTotalFunc1(#$T0, #$R)) == Tagclass._System.___hTotalFunc1);
+  Tag(Tclass._System.___hTotalFunc1(#$T0, #$R)) == Tagclass._System.___hTotalFunc1
+     && TagFamily(Tclass._System.___hTotalFunc1(#$T0, #$R)) == tytagFamily$_#TotalFunc1);
 
-const unique Tagclass._System.___hTotalFunc1: TyTag;
+function Tclass._System.___hTotalFunc1_0(Ty) : Ty;
 
 // Tclass._System.___hTotalFunc1 injectivity 0
 axiom (forall #$T0: Ty, #$R: Ty :: 
@@ -2734,14 +2376,12 @@ axiom (forall #$T0: Ty, #$R: Ty ::
   Tclass._System.___hTotalFunc1_0(Tclass._System.___hTotalFunc1(#$T0, #$R))
      == #$T0);
 
-function Tclass._System.___hTotalFunc1_0(Ty) : Ty;
+function Tclass._System.___hTotalFunc1_1(Ty) : Ty;
 
 // Tclass._System.___hTotalFunc1 injectivity 1
 axiom (forall #$T0: Ty, #$R: Ty :: 
   { Tclass._System.___hTotalFunc1(#$T0, #$R) } 
   Tclass._System.___hTotalFunc1_1(Tclass._System.___hTotalFunc1(#$T0, #$R)) == #$R);
-
-function Tclass._System.___hTotalFunc1_1(Ty) : Ty;
 
 // Box/unbox axiom for Tclass._System.___hTotalFunc1
 axiom (forall #$T0: Ty, #$R: Ty, bx: Box :: 
@@ -2750,32 +2390,302 @@ axiom (forall #$T0: Ty, #$R: Ty, bx: Box ::
      ==> $Box($Unbox(bx): HandleType) == bx
        && $Is($Unbox(bx): HandleType, Tclass._System.___hTotalFunc1(#$T0, #$R)));
 
-// _System._#TotalFunc1: subset type $Is
+// $Is axioms for subset type _System._#TotalFunc1
 axiom (forall #$T0: Ty, #$R: Ty, f#0: HandleType :: 
   { $Is(f#0, Tclass._System.___hTotalFunc1(#$T0, #$R)) } 
   $Is(f#0, Tclass._System.___hTotalFunc1(#$T0, #$R))
-     <==> $Is(f#0, Tclass._System.___hPartialFunc1(#$T0, #$R))
+     ==> $Is(f#0, Tclass._System.___hPartialFunc1(#$T0, #$R))
+       && 
+      (forall x0#0: Box :: 
+        $IsBox(x0#0, #$T0) ==> Requires1#canCall(#$T0, #$R, $OneHeap, f#0, x0#0))
        && (forall x0#0: Box :: 
         $IsBox(x0#0, #$T0) ==> Requires1(#$T0, #$R, $OneHeap, f#0, x0#0)));
 
-// _System._#TotalFunc1: subset type $IsAlloc
+axiom (forall #$T0: Ty, #$R: Ty, f#0: HandleType :: 
+  { $Is(f#0, Tclass._System.___hTotalFunc1(#$T0, #$R)) } 
+  $Is(f#0, Tclass._System.___hPartialFunc1(#$T0, #$R))
+       && ((forall x0#0: Box :: 
+          $IsBox(x0#0, #$T0) ==> Requires1#canCall(#$T0, #$R, $OneHeap, f#0, x0#0))
+         ==> (forall x0#0: Box :: 
+          $IsBox(x0#0, #$T0) ==> Requires1(#$T0, #$R, $OneHeap, f#0, x0#0)))
+     ==> $Is(f#0, Tclass._System.___hTotalFunc1(#$T0, #$R)));
+
+// $IsAlloc axiom for subset type _System._#TotalFunc1
 axiom (forall #$T0: Ty, #$R: Ty, f#0: HandleType, $h: Heap :: 
   { $IsAlloc(f#0, Tclass._System.___hTotalFunc1(#$T0, #$R), $h) } 
   $IsAlloc(f#0, Tclass._System.___hTotalFunc1(#$T0, #$R), $h)
      <==> $IsAlloc(f#0, Tclass._System.___hPartialFunc1(#$T0, #$R), $h));
 
-const unique class._System.Tuple2: ClassName;
+function Tclass._System.___hFunc0(Ty) : Ty;
 
-// Constructor function declaration
-function #_System._tuple#2._#Make2(Box, Box) : DatatypeType;
+const unique Tagclass._System.___hFunc0: TyTag;
 
-const unique ##_System._tuple#2._#Make2: DtCtorId;
+// Tclass._System.___hFunc0 Tag
+axiom (forall #$R: Ty :: 
+  { Tclass._System.___hFunc0(#$R) } 
+  Tag(Tclass._System.___hFunc0(#$R)) == Tagclass._System.___hFunc0
+     && TagFamily(Tclass._System.___hFunc0(#$R)) == tytagFamily$_#Func0);
 
+function Tclass._System.___hFunc0_0(Ty) : Ty;
+
+// Tclass._System.___hFunc0 injectivity 0
+axiom (forall #$R: Ty :: 
+  { Tclass._System.___hFunc0(#$R) } 
+  Tclass._System.___hFunc0_0(Tclass._System.___hFunc0(#$R)) == #$R);
+
+// Box/unbox axiom for Tclass._System.___hFunc0
+axiom (forall #$R: Ty, bx: Box :: 
+  { $IsBox(bx, Tclass._System.___hFunc0(#$R)) } 
+  $IsBox(bx, Tclass._System.___hFunc0(#$R))
+     ==> $Box($Unbox(bx): HandleType) == bx
+       && $Is($Unbox(bx): HandleType, Tclass._System.___hFunc0(#$R)));
+
+function Handle0([Heap]Box, [Heap]bool, [Heap]Set) : HandleType;
+
+function Apply0(Ty, Heap, HandleType) : Box;
+
+function Requires0(Ty, Heap, HandleType) : bool;
+
+function Reads0(Ty, Heap, HandleType) : Set;
+
+axiom (forall t0: Ty, heap: Heap, h: [Heap]Box, r: [Heap]bool, rd: [Heap]Set :: 
+  { Apply0(t0, heap, Handle0(h, r, rd)) } 
+  Apply0(t0, heap, Handle0(h, r, rd)) == h[heap]);
+
+axiom (forall t0: Ty, heap: Heap, h: [Heap]Box, r: [Heap]bool, rd: [Heap]Set :: 
+  { Requires0(t0, heap, Handle0(h, r, rd)) } 
+  r[heap] ==> Requires0(t0, heap, Handle0(h, r, rd)));
+
+axiom (forall t0: Ty, heap: Heap, h: [Heap]Box, r: [Heap]bool, rd: [Heap]Set, bx: Box :: 
+  { Set#IsMember(Reads0(t0, heap, Handle0(h, r, rd)), bx) } 
+  Set#IsMember(Reads0(t0, heap, Handle0(h, r, rd)), bx)
+     == Set#IsMember(rd[heap], bx));
+
+function {:inline} Requires0#canCall(t0: Ty, heap: Heap, f: HandleType) : bool
+{
+  true
+}
+
+function {:inline} Reads0#canCall(t0: Ty, heap: Heap, f: HandleType) : bool
+{
+  true
+}
+
+// frame axiom for Reads0
+axiom (forall t0: Ty, h0: Heap, h1: Heap, f: HandleType :: 
+  { $HeapSucc(h0, h1), Reads0(t0, h1, f) } 
+  $HeapSucc(h0, h1)
+       && 
+      $IsGoodHeap(h0)
+       && $IsGoodHeap(h1)
+       && $Is(f, Tclass._System.___hFunc0(t0))
+       && (forall o: ref, fld: Field :: 
+        o != null && Set#IsMember(Reads0(t0, h0, f), $Box(o))
+           ==> read(h0, o, fld) == read(h1, o, fld))
+     ==> Reads0(t0, h0, f) == Reads0(t0, h1, f));
+
+// frame axiom for Reads0
+axiom (forall t0: Ty, h0: Heap, h1: Heap, f: HandleType :: 
+  { $HeapSucc(h0, h1), Reads0(t0, h1, f) } 
+  $HeapSucc(h0, h1)
+       && 
+      $IsGoodHeap(h0)
+       && $IsGoodHeap(h1)
+       && $Is(f, Tclass._System.___hFunc0(t0))
+       && (forall o: ref, fld: Field :: 
+        o != null && Set#IsMember(Reads0(t0, h1, f), $Box(o))
+           ==> read(h0, o, fld) == read(h1, o, fld))
+     ==> Reads0(t0, h0, f) == Reads0(t0, h1, f));
+
+// frame axiom for Requires0
+axiom (forall t0: Ty, h0: Heap, h1: Heap, f: HandleType :: 
+  { $HeapSucc(h0, h1), Requires0(t0, h1, f) } 
+  $HeapSucc(h0, h1)
+       && 
+      $IsGoodHeap(h0)
+       && $IsGoodHeap(h1)
+       && $Is(f, Tclass._System.___hFunc0(t0))
+       && (forall o: ref, fld: Field :: 
+        o != null && Set#IsMember(Reads0(t0, h0, f), $Box(o))
+           ==> read(h0, o, fld) == read(h1, o, fld))
+     ==> Requires0(t0, h0, f) == Requires0(t0, h1, f));
+
+// frame axiom for Requires0
+axiom (forall t0: Ty, h0: Heap, h1: Heap, f: HandleType :: 
+  { $HeapSucc(h0, h1), Requires0(t0, h1, f) } 
+  $HeapSucc(h0, h1)
+       && 
+      $IsGoodHeap(h0)
+       && $IsGoodHeap(h1)
+       && $Is(f, Tclass._System.___hFunc0(t0))
+       && (forall o: ref, fld: Field :: 
+        o != null && Set#IsMember(Reads0(t0, h1, f), $Box(o))
+           ==> read(h0, o, fld) == read(h1, o, fld))
+     ==> Requires0(t0, h0, f) == Requires0(t0, h1, f));
+
+// frame axiom for Apply0
+axiom (forall t0: Ty, h0: Heap, h1: Heap, f: HandleType :: 
+  { $HeapSucc(h0, h1), Apply0(t0, h1, f) } 
+  $HeapSucc(h0, h1)
+       && 
+      $IsGoodHeap(h0)
+       && $IsGoodHeap(h1)
+       && $Is(f, Tclass._System.___hFunc0(t0))
+       && (forall o: ref, fld: Field :: 
+        o != null && Set#IsMember(Reads0(t0, h0, f), $Box(o))
+           ==> read(h0, o, fld) == read(h1, o, fld))
+     ==> Apply0(t0, h0, f) == Apply0(t0, h1, f));
+
+// frame axiom for Apply0
+axiom (forall t0: Ty, h0: Heap, h1: Heap, f: HandleType :: 
+  { $HeapSucc(h0, h1), Apply0(t0, h1, f) } 
+  $HeapSucc(h0, h1)
+       && 
+      $IsGoodHeap(h0)
+       && $IsGoodHeap(h1)
+       && $Is(f, Tclass._System.___hFunc0(t0))
+       && (forall o: ref, fld: Field :: 
+        o != null && Set#IsMember(Reads0(t0, h1, f), $Box(o))
+           ==> read(h0, o, fld) == read(h1, o, fld))
+     ==> Apply0(t0, h0, f) == Apply0(t0, h1, f));
+
+// empty-reads property for Reads0 
+axiom (forall t0: Ty, heap: Heap, f: HandleType :: 
+  { Reads0(t0, $OneHeap, f), $IsGoodHeap(heap) } { Reads0(t0, heap, f) } 
+  $IsGoodHeap(heap) && $Is(f, Tclass._System.___hFunc0(t0))
+     ==> (Set#Equal(Reads0(t0, $OneHeap, f), Set#Empty(): Set)
+       <==> Set#Equal(Reads0(t0, heap, f), Set#Empty(): Set)));
+
+// empty-reads property for Requires0
+axiom (forall t0: Ty, heap: Heap, f: HandleType :: 
+  { Requires0(t0, $OneHeap, f), $IsGoodHeap(heap) } { Requires0(t0, heap, f) } 
+  $IsGoodHeap(heap)
+       && $Is(f, Tclass._System.___hFunc0(t0))
+       && Set#Equal(Reads0(t0, $OneHeap, f), Set#Empty(): Set)
+     ==> Requires0(t0, $OneHeap, f) == Requires0(t0, heap, f));
+
+axiom (forall f: HandleType, t0: Ty :: 
+  { $Is(f, Tclass._System.___hFunc0(t0)) } 
+  $Is(f, Tclass._System.___hFunc0(t0))
+     <==> (forall h: Heap :: 
+      { Apply0(t0, h, f) } 
+      $IsGoodHeap(h) && Requires0(t0, h, f) ==> $IsBox(Apply0(t0, h, f), t0)));
+
+axiom (forall f: HandleType, t0: Ty, u0: Ty :: 
+  { $Is(f, Tclass._System.___hFunc0(t0)), $Is(f, Tclass._System.___hFunc0(u0)) } 
+  $Is(f, Tclass._System.___hFunc0(t0))
+       && (forall bx: Box :: 
+        { $IsBox(bx, t0) } { $IsBox(bx, u0) } 
+        $IsBox(bx, t0) ==> $IsBox(bx, u0))
+     ==> $Is(f, Tclass._System.___hFunc0(u0)));
+
+axiom (forall f: HandleType, t0: Ty, h: Heap :: 
+  { $IsAlloc(f, Tclass._System.___hFunc0(t0), h) } 
+  $IsGoodHeap(h)
+     ==> ($IsAlloc(f, Tclass._System.___hFunc0(t0), h)
+       <==> Requires0(t0, h, f)
+         ==> (forall r: ref :: 
+          { Set#IsMember(Reads0(t0, h, f), $Box(r)) } 
+          r != null && Set#IsMember(Reads0(t0, h, f), $Box(r))
+             ==> $Unbox(read(h, r, alloc)): bool)));
+
+axiom (forall f: HandleType, t0: Ty, h: Heap :: 
+  { $IsAlloc(f, Tclass._System.___hFunc0(t0), h) } 
+  $IsGoodHeap(h) && $IsAlloc(f, Tclass._System.___hFunc0(t0), h)
+     ==> 
+    Requires0(t0, h, f)
+     ==> $IsAllocBox(Apply0(t0, h, f), t0, h));
+
+function Tclass._System.___hPartialFunc0(Ty) : Ty;
+
+const unique Tagclass._System.___hPartialFunc0: TyTag;
+
+// Tclass._System.___hPartialFunc0 Tag
+axiom (forall #$R: Ty :: 
+  { Tclass._System.___hPartialFunc0(#$R) } 
+  Tag(Tclass._System.___hPartialFunc0(#$R)) == Tagclass._System.___hPartialFunc0
+     && TagFamily(Tclass._System.___hPartialFunc0(#$R)) == tytagFamily$_#PartialFunc0);
+
+function Tclass._System.___hPartialFunc0_0(Ty) : Ty;
+
+// Tclass._System.___hPartialFunc0 injectivity 0
+axiom (forall #$R: Ty :: 
+  { Tclass._System.___hPartialFunc0(#$R) } 
+  Tclass._System.___hPartialFunc0_0(Tclass._System.___hPartialFunc0(#$R)) == #$R);
+
+// Box/unbox axiom for Tclass._System.___hPartialFunc0
+axiom (forall #$R: Ty, bx: Box :: 
+  { $IsBox(bx, Tclass._System.___hPartialFunc0(#$R)) } 
+  $IsBox(bx, Tclass._System.___hPartialFunc0(#$R))
+     ==> $Box($Unbox(bx): HandleType) == bx
+       && $Is($Unbox(bx): HandleType, Tclass._System.___hPartialFunc0(#$R)));
+
+// $Is axiom for subset type _System._#PartialFunc0
+axiom (forall #$R: Ty, f#0: HandleType :: 
+  { $Is(f#0, Tclass._System.___hPartialFunc0(#$R)) } 
+  $Is(f#0, Tclass._System.___hPartialFunc0(#$R))
+     <==> $Is(f#0, Tclass._System.___hFunc0(#$R))
+       && Set#Equal(Reads0(#$R, $OneHeap, f#0), Set#Empty(): Set));
+
+// $IsAlloc axiom for subset type _System._#PartialFunc0
+axiom (forall #$R: Ty, f#0: HandleType, $h: Heap :: 
+  { $IsAlloc(f#0, Tclass._System.___hPartialFunc0(#$R), $h) } 
+  $IsAlloc(f#0, Tclass._System.___hPartialFunc0(#$R), $h)
+     <==> $IsAlloc(f#0, Tclass._System.___hFunc0(#$R), $h));
+
+function Tclass._System.___hTotalFunc0(Ty) : Ty;
+
+const unique Tagclass._System.___hTotalFunc0: TyTag;
+
+// Tclass._System.___hTotalFunc0 Tag
+axiom (forall #$R: Ty :: 
+  { Tclass._System.___hTotalFunc0(#$R) } 
+  Tag(Tclass._System.___hTotalFunc0(#$R)) == Tagclass._System.___hTotalFunc0
+     && TagFamily(Tclass._System.___hTotalFunc0(#$R)) == tytagFamily$_#TotalFunc0);
+
+function Tclass._System.___hTotalFunc0_0(Ty) : Ty;
+
+// Tclass._System.___hTotalFunc0 injectivity 0
+axiom (forall #$R: Ty :: 
+  { Tclass._System.___hTotalFunc0(#$R) } 
+  Tclass._System.___hTotalFunc0_0(Tclass._System.___hTotalFunc0(#$R)) == #$R);
+
+// Box/unbox axiom for Tclass._System.___hTotalFunc0
+axiom (forall #$R: Ty, bx: Box :: 
+  { $IsBox(bx, Tclass._System.___hTotalFunc0(#$R)) } 
+  $IsBox(bx, Tclass._System.___hTotalFunc0(#$R))
+     ==> $Box($Unbox(bx): HandleType) == bx
+       && $Is($Unbox(bx): HandleType, Tclass._System.___hTotalFunc0(#$R)));
+
+// $Is axioms for subset type _System._#TotalFunc0
+axiom (forall #$R: Ty, f#0: HandleType :: 
+  { $Is(f#0, Tclass._System.___hTotalFunc0(#$R)) } 
+  $Is(f#0, Tclass._System.___hTotalFunc0(#$R))
+     ==> $Is(f#0, Tclass._System.___hPartialFunc0(#$R))
+       && 
+      Requires0#canCall(#$R, $OneHeap, f#0)
+       && Requires0(#$R, $OneHeap, f#0));
+
+axiom (forall #$R: Ty, f#0: HandleType :: 
+  { $Is(f#0, Tclass._System.___hTotalFunc0(#$R)) } 
+  $Is(f#0, Tclass._System.___hPartialFunc0(#$R))
+       && (Requires0#canCall(#$R, $OneHeap, f#0) ==> Requires0(#$R, $OneHeap, f#0))
+     ==> $Is(f#0, Tclass._System.___hTotalFunc0(#$R)));
+
+// $IsAlloc axiom for subset type _System._#TotalFunc0
+axiom (forall #$R: Ty, f#0: HandleType, $h: Heap :: 
+  { $IsAlloc(f#0, Tclass._System.___hTotalFunc0(#$R), $h) } 
+  $IsAlloc(f#0, Tclass._System.___hTotalFunc0(#$R), $h)
+     <==> $IsAlloc(f#0, Tclass._System.___hPartialFunc0(#$R), $h));
+
+const unique ##_System._tuple#2._#Make2: DtCtorId
+uses {
 // Constructor identifier
 axiom (forall a#0#0#0: Box, a#0#1#0: Box :: 
   { #_System._tuple#2._#Make2(a#0#0#0, a#0#1#0) } 
   DatatypeCtorId(#_System._tuple#2._#Make2(a#0#0#0, a#0#1#0))
      == ##_System._tuple#2._#Make2);
+}
 
 function _System.Tuple2.___hMake2_q(DatatypeType) : bool;
 
@@ -2792,100 +2702,111 @@ axiom (forall d: DatatypeType ::
      ==> (exists a#1#0#0: Box, a#1#1#0: Box :: 
       d == #_System._tuple#2._#Make2(a#1#0#0, a#1#1#0)));
 
-function Tclass._System.Tuple2(Ty, Ty) : Ty;
-
-// Tclass._System.Tuple2 Tag
-axiom (forall #$T0: Ty, #$T1: Ty :: 
-  { Tclass._System.Tuple2(#$T0, #$T1) } 
-  Tag(Tclass._System.Tuple2(#$T0, #$T1)) == Tagclass._System.Tuple2);
-
 const unique Tagclass._System.Tuple2: TyTag;
 
-// Tclass._System.Tuple2 injectivity 0
-axiom (forall #$T0: Ty, #$T1: Ty :: 
-  { Tclass._System.Tuple2(#$T0, #$T1) } 
-  Tclass._System.Tuple2_0(Tclass._System.Tuple2(#$T0, #$T1)) == #$T0);
+// Tclass._System.Tuple2 Tag
+axiom (forall _System._tuple#2$T0: Ty, _System._tuple#2$T1: Ty :: 
+  { Tclass._System.Tuple2(_System._tuple#2$T0, _System._tuple#2$T1) } 
+  Tag(Tclass._System.Tuple2(_System._tuple#2$T0, _System._tuple#2$T1))
+       == Tagclass._System.Tuple2
+     && TagFamily(Tclass._System.Tuple2(_System._tuple#2$T0, _System._tuple#2$T1))
+       == tytagFamily$_tuple#2);
 
 function Tclass._System.Tuple2_0(Ty) : Ty;
 
-// Tclass._System.Tuple2 injectivity 1
-axiom (forall #$T0: Ty, #$T1: Ty :: 
-  { Tclass._System.Tuple2(#$T0, #$T1) } 
-  Tclass._System.Tuple2_1(Tclass._System.Tuple2(#$T0, #$T1)) == #$T1);
+// Tclass._System.Tuple2 injectivity 0
+axiom (forall _System._tuple#2$T0: Ty, _System._tuple#2$T1: Ty :: 
+  { Tclass._System.Tuple2(_System._tuple#2$T0, _System._tuple#2$T1) } 
+  Tclass._System.Tuple2_0(Tclass._System.Tuple2(_System._tuple#2$T0, _System._tuple#2$T1))
+     == _System._tuple#2$T0);
 
 function Tclass._System.Tuple2_1(Ty) : Ty;
 
+// Tclass._System.Tuple2 injectivity 1
+axiom (forall _System._tuple#2$T0: Ty, _System._tuple#2$T1: Ty :: 
+  { Tclass._System.Tuple2(_System._tuple#2$T0, _System._tuple#2$T1) } 
+  Tclass._System.Tuple2_1(Tclass._System.Tuple2(_System._tuple#2$T0, _System._tuple#2$T1))
+     == _System._tuple#2$T1);
+
 // Box/unbox axiom for Tclass._System.Tuple2
-axiom (forall #$T0: Ty, #$T1: Ty, bx: Box :: 
-  { $IsBox(bx, Tclass._System.Tuple2(#$T0, #$T1)) } 
-  $IsBox(bx, Tclass._System.Tuple2(#$T0, #$T1))
+axiom (forall _System._tuple#2$T0: Ty, _System._tuple#2$T1: Ty, bx: Box :: 
+  { $IsBox(bx, Tclass._System.Tuple2(_System._tuple#2$T0, _System._tuple#2$T1)) } 
+  $IsBox(bx, Tclass._System.Tuple2(_System._tuple#2$T0, _System._tuple#2$T1))
      ==> $Box($Unbox(bx): DatatypeType) == bx
-       && $Is($Unbox(bx): DatatypeType, Tclass._System.Tuple2(#$T0, #$T1)));
+       && $Is($Unbox(bx): DatatypeType, 
+        Tclass._System.Tuple2(_System._tuple#2$T0, _System._tuple#2$T1)));
 
 // Constructor $Is
-axiom (forall #$T0: Ty, #$T1: Ty, a#2#0#0: Box, a#2#1#0: Box :: 
-  { $Is(#_System._tuple#2._#Make2(a#2#0#0, a#2#1#0), Tclass._System.Tuple2(#$T0, #$T1)) } 
-  $Is(#_System._tuple#2._#Make2(a#2#0#0, a#2#1#0), Tclass._System.Tuple2(#$T0, #$T1))
-     <==> $IsBox(a#2#0#0, #$T0) && $IsBox(a#2#1#0, #$T1));
+axiom (forall _System._tuple#2$T0: Ty, _System._tuple#2$T1: Ty, a#2#0#0: Box, a#2#1#0: Box :: 
+  { $Is(#_System._tuple#2._#Make2(a#2#0#0, a#2#1#0), 
+      Tclass._System.Tuple2(_System._tuple#2$T0, _System._tuple#2$T1)) } 
+  $Is(#_System._tuple#2._#Make2(a#2#0#0, a#2#1#0), 
+      Tclass._System.Tuple2(_System._tuple#2$T0, _System._tuple#2$T1))
+     <==> $IsBox(a#2#0#0, _System._tuple#2$T0) && $IsBox(a#2#1#0, _System._tuple#2$T1));
 
 // Constructor $IsAlloc
-axiom (forall #$T0: Ty, #$T1: Ty, a#3#0#0: Box, a#3#1#0: Box, $h: Heap :: 
-  { $IsAlloc(#_System._tuple#2._#Make2(a#3#0#0, a#3#1#0), 
-      Tclass._System.Tuple2(#$T0, #$T1), 
+axiom (forall _System._tuple#2$T0: Ty, 
+    _System._tuple#2$T1: Ty, 
+    a#2#0#0: Box, 
+    a#2#1#0: Box, 
+    $h: Heap :: 
+  { $IsAlloc(#_System._tuple#2._#Make2(a#2#0#0, a#2#1#0), 
+      Tclass._System.Tuple2(_System._tuple#2$T0, _System._tuple#2$T1), 
       $h) } 
   $IsGoodHeap($h)
-     ==> ($IsAlloc(#_System._tuple#2._#Make2(a#3#0#0, a#3#1#0), 
-        Tclass._System.Tuple2(#$T0, #$T1), 
+     ==> ($IsAlloc(#_System._tuple#2._#Make2(a#2#0#0, a#2#1#0), 
+        Tclass._System.Tuple2(_System._tuple#2$T0, _System._tuple#2$T1), 
         $h)
-       <==> $IsAllocBox(a#3#0#0, #$T0, $h) && $IsAllocBox(a#3#1#0, #$T1, $h)));
+       <==> $IsAllocBox(a#2#0#0, _System._tuple#2$T0, $h)
+         && $IsAllocBox(a#2#1#0, _System._tuple#2$T1, $h)));
 
 // Destructor $IsAlloc
-axiom (forall d: DatatypeType, #$T0: Ty, $h: Heap :: 
-  { $IsAllocBox(_System.Tuple2._0(d), #$T0, $h) } 
+axiom (forall d: DatatypeType, _System._tuple#2$T0: Ty, $h: Heap :: 
+  { $IsAllocBox(_System.Tuple2._0(d), _System._tuple#2$T0, $h) } 
   $IsGoodHeap($h)
        && 
       _System.Tuple2.___hMake2_q(d)
-       && (exists #$T1: Ty :: 
-        { $IsAlloc(d, Tclass._System.Tuple2(#$T0, #$T1), $h) } 
-        $IsAlloc(d, Tclass._System.Tuple2(#$T0, #$T1), $h))
-     ==> $IsAllocBox(_System.Tuple2._0(d), #$T0, $h));
+       && (exists _System._tuple#2$T1: Ty :: 
+        { $IsAlloc(d, Tclass._System.Tuple2(_System._tuple#2$T0, _System._tuple#2$T1), $h) } 
+        $IsAlloc(d, Tclass._System.Tuple2(_System._tuple#2$T0, _System._tuple#2$T1), $h))
+     ==> $IsAllocBox(_System.Tuple2._0(d), _System._tuple#2$T0, $h));
 
 // Destructor $IsAlloc
-axiom (forall d: DatatypeType, #$T1: Ty, $h: Heap :: 
-  { $IsAllocBox(_System.Tuple2._1(d), #$T1, $h) } 
+axiom (forall d: DatatypeType, _System._tuple#2$T1: Ty, $h: Heap :: 
+  { $IsAllocBox(_System.Tuple2._1(d), _System._tuple#2$T1, $h) } 
   $IsGoodHeap($h)
        && 
       _System.Tuple2.___hMake2_q(d)
-       && (exists #$T0: Ty :: 
-        { $IsAlloc(d, Tclass._System.Tuple2(#$T0, #$T1), $h) } 
-        $IsAlloc(d, Tclass._System.Tuple2(#$T0, #$T1), $h))
-     ==> $IsAllocBox(_System.Tuple2._1(d), #$T1, $h));
+       && (exists _System._tuple#2$T0: Ty :: 
+        { $IsAlloc(d, Tclass._System.Tuple2(_System._tuple#2$T0, _System._tuple#2$T1), $h) } 
+        $IsAlloc(d, Tclass._System.Tuple2(_System._tuple#2$T0, _System._tuple#2$T1), $h))
+     ==> $IsAllocBox(_System.Tuple2._1(d), _System._tuple#2$T1, $h));
 
 // Constructor literal
-axiom (forall a#4#0#0: Box, a#4#1#0: Box :: 
-  { #_System._tuple#2._#Make2(Lit(a#4#0#0), Lit(a#4#1#0)) } 
-  #_System._tuple#2._#Make2(Lit(a#4#0#0), Lit(a#4#1#0))
-     == Lit(#_System._tuple#2._#Make2(a#4#0#0, a#4#1#0)));
+axiom (forall a#3#0#0: Box, a#3#1#0: Box :: 
+  { #_System._tuple#2._#Make2(Lit(a#3#0#0), Lit(a#3#1#0)) } 
+  #_System._tuple#2._#Make2(Lit(a#3#0#0), Lit(a#3#1#0))
+     == Lit(#_System._tuple#2._#Make2(a#3#0#0, a#3#1#0)));
 
 // Constructor injectivity
-axiom (forall a#5#0#0: Box, a#5#1#0: Box :: 
-  { #_System._tuple#2._#Make2(a#5#0#0, a#5#1#0) } 
-  _System.Tuple2._0(#_System._tuple#2._#Make2(a#5#0#0, a#5#1#0)) == a#5#0#0);
+axiom (forall a#4#0#0: Box, a#4#1#0: Box :: 
+  { #_System._tuple#2._#Make2(a#4#0#0, a#4#1#0) } 
+  _System.Tuple2._0(#_System._tuple#2._#Make2(a#4#0#0, a#4#1#0)) == a#4#0#0);
 
 // Inductive rank
+axiom (forall a#5#0#0: Box, a#5#1#0: Box :: 
+  { DtRank(#_System._tuple#2._#Make2(a#5#0#0, a#5#1#0)) } 
+  BoxRank(a#5#0#0) < DtRank(#_System._tuple#2._#Make2(a#5#0#0, a#5#1#0)));
+
+// Constructor injectivity
 axiom (forall a#6#0#0: Box, a#6#1#0: Box :: 
   { #_System._tuple#2._#Make2(a#6#0#0, a#6#1#0) } 
-  BoxRank(a#6#0#0) < DtRank(#_System._tuple#2._#Make2(a#6#0#0, a#6#1#0)));
-
-// Constructor injectivity
-axiom (forall a#7#0#0: Box, a#7#1#0: Box :: 
-  { #_System._tuple#2._#Make2(a#7#0#0, a#7#1#0) } 
-  _System.Tuple2._1(#_System._tuple#2._#Make2(a#7#0#0, a#7#1#0)) == a#7#1#0);
+  _System.Tuple2._1(#_System._tuple#2._#Make2(a#6#0#0, a#6#1#0)) == a#6#1#0);
 
 // Inductive rank
-axiom (forall a#8#0#0: Box, a#8#1#0: Box :: 
-  { #_System._tuple#2._#Make2(a#8#0#0, a#8#1#0) } 
-  BoxRank(a#8#1#0) < DtRank(#_System._tuple#2._#Make2(a#8#0#0, a#8#1#0)));
+axiom (forall a#7#0#0: Box, a#7#1#0: Box :: 
+  { DtRank(#_System._tuple#2._#Make2(a#7#0#0, a#7#1#0)) } 
+  BoxRank(a#7#1#0) < DtRank(#_System._tuple#2._#Make2(a#7#0#0, a#7#1#0)));
 
 // Depth-one case-split function
 function $IsA#_System.Tuple2(DatatypeType) : bool;
@@ -2896,9 +2817,10 @@ axiom (forall d: DatatypeType ::
   $IsA#_System.Tuple2(d) ==> _System.Tuple2.___hMake2_q(d));
 
 // Questionmark data type disjunctivity
-axiom (forall #$T0: Ty, #$T1: Ty, d: DatatypeType :: 
-  { _System.Tuple2.___hMake2_q(d), $Is(d, Tclass._System.Tuple2(#$T0, #$T1)) } 
-  $Is(d, Tclass._System.Tuple2(#$T0, #$T1)) ==> _System.Tuple2.___hMake2_q(d));
+axiom (forall _System._tuple#2$T0: Ty, _System._tuple#2$T1: Ty, d: DatatypeType :: 
+  { _System.Tuple2.___hMake2_q(d), $Is(d, Tclass._System.Tuple2(_System._tuple#2$T0, _System._tuple#2$T1)) } 
+  $Is(d, Tclass._System.Tuple2(_System._tuple#2$T0, _System._tuple#2$T1))
+     ==> _System.Tuple2.___hMake2_q(d));
 
 // Datatype extensional equality declaration
 function _System.Tuple2#Equal(DatatypeType, DatatypeType) : bool;
@@ -2906,25 +2828,33 @@ function _System.Tuple2#Equal(DatatypeType, DatatypeType) : bool;
 // Datatype extensional equality definition: #_System._tuple#2._#Make2
 axiom (forall a: DatatypeType, b: DatatypeType :: 
   { _System.Tuple2#Equal(a, b) } 
-  true
-     ==> (_System.Tuple2#Equal(a, b)
-       <==> _System.Tuple2._0(a) == _System.Tuple2._0(b)
-         && _System.Tuple2._1(a) == _System.Tuple2._1(b)));
+  _System.Tuple2#Equal(a, b)
+     <==> _System.Tuple2._0(a) == _System.Tuple2._0(b)
+       && _System.Tuple2._1(a) == _System.Tuple2._1(b));
 
 // Datatype extensionality axiom: _System._tuple#2
 axiom (forall a: DatatypeType, b: DatatypeType :: 
   { _System.Tuple2#Equal(a, b) } 
   _System.Tuple2#Equal(a, b) <==> a == b);
 
-const unique class._System.Tuple0: ClassName;
+const unique class._System.Tuple2: ClassName;
 
 // Constructor function declaration
-function #_System._tuple#0._#Make0() : DatatypeType;
-
-const unique ##_System._tuple#0._#Make0: DtCtorId;
-
+function #_System._tuple#0._#Make0() : DatatypeType
+uses {
 // Constructor identifier
 axiom DatatypeCtorId(#_System._tuple#0._#Make0()) == ##_System._tuple#0._#Make0;
+// Constructor $Is
+axiom $Is(#_System._tuple#0._#Make0(), Tclass._System.Tuple0());
+// Constructor literal
+axiom #_System._tuple#0._#Make0() == Lit(#_System._tuple#0._#Make0());
+}
+
+const unique ##_System._tuple#0._#Make0: DtCtorId
+uses {
+// Constructor identifier
+axiom DatatypeCtorId(#_System._tuple#0._#Make0()) == ##_System._tuple#0._#Make0;
+}
 
 function _System.Tuple0.___hMake0_q(DatatypeType) : bool;
 
@@ -2939,10 +2869,12 @@ axiom (forall d: DatatypeType ::
   { _System.Tuple0.___hMake0_q(d) } 
   _System.Tuple0.___hMake0_q(d) ==> d == #_System._tuple#0._#Make0());
 
-function Tclass._System.Tuple0() : Ty;
-
+function Tclass._System.Tuple0() : Ty
+uses {
 // Tclass._System.Tuple0 Tag
-axiom Tag(Tclass._System.Tuple0()) == Tagclass._System.Tuple0;
+axiom Tag(Tclass._System.Tuple0()) == Tagclass._System.Tuple0
+   && TagFamily(Tclass._System.Tuple0()) == tytagFamily$_tuple#0;
+}
 
 const unique Tagclass._System.Tuple0: TyTag;
 
@@ -2953,17 +2885,11 @@ axiom (forall bx: Box ::
      ==> $Box($Unbox(bx): DatatypeType) == bx
        && $Is($Unbox(bx): DatatypeType, Tclass._System.Tuple0()));
 
-// Constructor $Is
-axiom $Is(#_System._tuple#0._#Make0(), Tclass._System.Tuple0());
-
-// Constructor $IsAlloc
-axiom (forall $h: Heap :: 
-  { $IsAlloc(#_System._tuple#0._#Make0(), Tclass._System.Tuple0(), $h) } 
-  $IsGoodHeap($h)
-     ==> $IsAlloc(#_System._tuple#0._#Make0(), Tclass._System.Tuple0(), $h));
-
-// Constructor literal
-axiom #_System._tuple#0._#Make0() == Lit(#_System._tuple#0._#Make0());
+// Datatype $IsAlloc
+axiom (forall d: DatatypeType, $h: Heap :: 
+  { $IsAlloc(d, Tclass._System.Tuple0(), $h) } 
+  $IsGoodHeap($h) && $Is(d, Tclass._System.Tuple0())
+     ==> $IsAlloc(d, Tclass._System.Tuple0(), $h));
 
 // Depth-one case-split function
 function $IsA#_System.Tuple0(DatatypeType) : bool;
@@ -2984,507 +2910,432 @@ function _System.Tuple0#Equal(DatatypeType, DatatypeType) : bool;
 // Datatype extensional equality definition: #_System._tuple#0._#Make0
 axiom (forall a: DatatypeType, b: DatatypeType :: 
   { _System.Tuple0#Equal(a, b) } 
-  true ==> (_System.Tuple0#Equal(a, b) <==> true));
+  _System.Tuple0#Equal(a, b));
 
 // Datatype extensionality axiom: _System._tuple#0
 axiom (forall a: DatatypeType, b: DatatypeType :: 
   { _System.Tuple0#Equal(a, b) } 
   _System.Tuple0#Equal(a, b) <==> a == b);
 
+const unique class._System.Tuple0: ClassName;
+
 const unique class._module.__default: ClassName;
 
-function Tclass._module.__default() : Ty;
+// function declaration for _module._default.maxR
+function _module.__default.maxR($ly: LayerType, l#0: Seq) : int;
 
-// Tclass._module.__default Tag
-axiom Tag(Tclass._module.__default()) == Tagclass._module.__default;
-
-const unique Tagclass._module.__default: TyTag;
-
-// Box/unbox axiom for Tclass._module.__default
-axiom (forall bx: Box :: 
-  { $IsBox(bx, Tclass._module.__default()) } 
-  $IsBox(bx, Tclass._module.__default())
-     ==> $Box($Unbox(bx): ref) == bx && $Is($Unbox(bx): ref, Tclass._module.__default()));
-
-// _default: Class $Is
-axiom (forall $o: ref :: 
-  { $Is($o, Tclass._module.__default()) } 
-  $Is($o, Tclass._module.__default())
-     <==> $o == null || dtype($o) == Tclass._module.__default());
-
-// _default: Class $IsAlloc
-axiom (forall $o: ref, $h: Heap :: 
-  { $IsAlloc($o, Tclass._module.__default(), $h) } 
-  $IsAlloc($o, Tclass._module.__default(), $h)
-     <==> $o == null || read($h, $o, alloc));
-
-// function declaration for _module._default.loop
-function _module.__default.loop($ly: LayerType, p#0: int, l#0: Seq Box) : bool;
-
-function _module.__default.loop#canCall(p#0: int, l#0: Seq Box) : bool;
+function _module.__default.maxR#canCall(l#0: Seq) : bool;
 
 // layer synonym axiom
-axiom (forall $ly: LayerType, p#0: int, l#0: Seq Box :: 
-  { _module.__default.loop($LS($ly), p#0, l#0) } 
-  _module.__default.loop($LS($ly), p#0, l#0)
-     == _module.__default.loop($ly, p#0, l#0));
+axiom (forall $ly: LayerType, l#0: Seq :: 
+  { _module.__default.maxR($LS($ly), l#0) } 
+  _module.__default.maxR($LS($ly), l#0) == _module.__default.maxR($ly, l#0));
 
 // fuel synonym axiom
-axiom (forall $ly: LayerType, p#0: int, l#0: Seq Box :: 
-  { _module.__default.loop(AsFuelBottom($ly), p#0, l#0) } 
-  _module.__default.loop($ly, p#0, l#0) == _module.__default.loop($LZ, p#0, l#0));
+axiom (forall $ly: LayerType, l#0: Seq :: 
+  { _module.__default.maxR(AsFuelBottom($ly), l#0) } 
+  _module.__default.maxR($ly, l#0) == _module.__default.maxR($LZ, l#0));
 
-// consequence axiom for _module.__default.loop
-axiom 0 <= $FunctionContextHeight
-   ==> (forall $ly: LayerType, p#0: int, l#0: Seq Box :: 
-    { _module.__default.loop($ly, p#0, l#0) } 
-    _module.__default.loop#canCall(p#0, l#0)
-         || (0 != $FunctionContextHeight && $Is(l#0, TSeq(TInt)))
-       ==> true);
+function _module.__default.maxR#requires(LayerType, Seq) : bool;
 
-function _module.__default.loop#requires(LayerType, int, Seq Box) : bool;
+// #requires axiom for _module.__default.maxR
+axiom (forall $ly: LayerType, l#0: Seq :: 
+  { _module.__default.maxR#requires($ly, l#0) } 
+  $Is(l#0, TSeq(TInt)) ==> _module.__default.maxR#requires($ly, l#0) == true);
 
-// #requires axiom for _module.__default.loop
-axiom (forall $ly: LayerType, p#0: int, l#0: Seq Box :: 
-  { _module.__default.loop#requires($ly, p#0, l#0) } 
-  $Is(l#0, TSeq(TInt)) ==> _module.__default.loop#requires($ly, p#0, l#0) == true);
+// #requires ==> #canCall for _module.__default.maxR
+axiom (forall $ly: LayerType, l#0: Seq :: 
+  { _module.__default.maxR#requires($ly, l#0) } 
+  _module.__default.maxR#requires($ly, l#0)
+     ==> _module.__default.maxR#canCall(l#0));
 
-// definition axiom for _module.__default.loop(revealed)
-axiom 0 <= $FunctionContextHeight
-   ==> (forall $ly: LayerType, p#0: int, l#0: Seq Box :: 
-    { _module.__default.loop($LS($ly), p#0, l#0) } 
-    _module.__default.loop#canCall(p#0, l#0)
-         || (0 != $FunctionContextHeight && $Is(l#0, TSeq(TInt)))
-       ==> (Seq#Length(l#0) != LitInt(0)
-           ==> 
-          p#0 <= $Unbox(Seq#Index(l#0, LitInt(0))): int
-           ==> _module.__default.loop#canCall($Unbox(Seq#Index(l#0, LitInt(0))): int, Seq#Drop(l#0, LitInt(1))))
-         && _module.__default.loop($LS($ly), p#0, l#0)
-           == (if Seq#Length(l#0) == LitInt(0)
-             then true
-             else p#0 <= $Unbox(Seq#Index(l#0, LitInt(0))): int
-               && _module.__default.loop($ly, $Unbox(Seq#Index(l#0, LitInt(0))): int, Seq#Drop(l#0, LitInt(1)))));
+// definition axiom for _module.__default.maxR (revealed)
+axiom {:id "id0"} (forall $ly: LayerType, l#0: Seq :: 
+  { _module.__default.maxR($LS($ly), l#0) } 
+  _module.__default.maxR#canCall(l#0)
+     ==> (Seq#Length(l#0) != LitInt(0)
+         ==> 
+        Seq#Length(l#0) != LitInt(1)
+         ==> _module.__default.maxR#canCall(Seq#Drop(l#0, LitInt(1))))
+       && _module.__default.maxR($LS($ly), l#0)
+         == (if Seq#Length(l#0) == LitInt(0)
+           then -1
+           else (if Seq#Length(l#0) == LitInt(1)
+             then $Unbox(Seq#Index(l#0, LitInt(0))): int
+             else (var m#0 := _module.__default.maxR($ly, Seq#Drop(l#0, LitInt(1))); 
+              (if $Unbox(Seq#Index(l#0, LitInt(0))): int > m#0
+                 then $Unbox(Seq#Index(l#0, LitInt(0))): int
+                 else m#0)))));
 
-// definition axiom for _module.__default.loop for decreasing-related literals(revealed)
-axiom 0 <= $FunctionContextHeight
-   ==> (forall $ly: LayerType, p#0: int, l#0: Seq Box :: 
-    {:weight 3} { _module.__default.loop($LS($ly), p#0, Lit(l#0)) } 
-    _module.__default.loop#canCall(p#0, Lit(l#0))
-         || (0 != $FunctionContextHeight && $Is(l#0, TSeq(TInt)))
-       ==> (Seq#Length(Lit(l#0)) != LitInt(0)
-           ==> 
-          p#0 <= $Unbox(Seq#Index(Lit(l#0), LitInt(0))): int
-           ==> _module.__default.loop#canCall($Unbox(Seq#Index(Lit(l#0), LitInt(0))): int, Lit(Seq#Drop(Lit(l#0), LitInt(1)))))
-         && _module.__default.loop($LS($ly), p#0, Lit(l#0))
-           == (if Seq#Length(Lit(l#0)) == LitInt(0)
-             then true
-             else p#0 <= $Unbox(Seq#Index(Lit(l#0), LitInt(0))): int
-               && _module.__default.loop($LS($ly), 
-                $Unbox(Seq#Index(Lit(l#0), LitInt(0))): int, 
-                Lit(Seq#Drop(Lit(l#0), LitInt(1))))));
+// definition axiom for _module.__default.maxR for all literals (revealed)
+axiom {:id "id1"} (forall $ly: LayerType, l#0: Seq :: 
+  {:weight 3} { _module.__default.maxR($LS($ly), Lit(l#0)) } 
+  _module.__default.maxR#canCall(Lit(l#0))
+     ==> (Seq#Length(Lit(l#0)) != LitInt(0)
+         ==> 
+        Seq#Length(Lit(l#0)) != LitInt(1)
+         ==> _module.__default.maxR#canCall(Lit(Seq#Drop(Lit(l#0), LitInt(1)))))
+       && _module.__default.maxR($LS($ly), Lit(l#0))
+         == (if Seq#Length(Lit(l#0)) == LitInt(0)
+           then -1
+           else (if Seq#Length(Lit(l#0)) == LitInt(1)
+             then $Unbox(Seq#Index(Lit(l#0), LitInt(0))): int
+             else (var m#1 := LitInt(_module.__default.maxR($LS($ly), Lit(Seq#Drop(Lit(l#0), LitInt(1))))); 
+              (if $Unbox(Seq#Index(Lit(l#0), LitInt(0))): int > m#1
+                 then $Unbox(Seq#Index(Lit(l#0), LitInt(0))): int
+                 else m#1)))));
 
-// definition axiom for _module.__default.loop for all literals(revealed)
-axiom 0 <= $FunctionContextHeight
-   ==> (forall $ly: LayerType, p#0: int, l#0: Seq Box :: 
-    {:weight 3} { _module.__default.loop($LS($ly), LitInt(p#0), Lit(l#0)) } 
-    _module.__default.loop#canCall(LitInt(p#0), Lit(l#0))
-         || (0 != $FunctionContextHeight && $Is(l#0, TSeq(TInt)))
-       ==> (Seq#Length(Lit(l#0)) != LitInt(0)
-           ==> 
-          LitInt(p#0) <= $Unbox(Seq#Index(Lit(l#0), LitInt(0))): int
-           ==> _module.__default.loop#canCall($Unbox(Seq#Index(Lit(l#0), LitInt(0))): int, Lit(Seq#Drop(Lit(l#0), LitInt(1)))))
-         && _module.__default.loop($LS($ly), LitInt(p#0), Lit(l#0))
-           == (if Seq#Length(Lit(l#0)) == LitInt(0)
-             then true
-             else LitInt(p#0) <= $Unbox(Seq#Index(Lit(l#0), LitInt(0))): int
-               && _module.__default.loop($LS($ly), 
-                $Unbox(Seq#Index(Lit(l#0), LitInt(0))): int, 
-                Lit(Seq#Drop(Lit(l#0), LitInt(1))))));
-
-procedure CheckWellformed$$_module.__default.loop(p#0: int, l#0: Seq Box where $Is(l#0, TSeq(TInt)));
-  free requires 0 == $FunctionContextHeight;
-  modifies $Heap, $Tick;
+procedure {:verboseName "maxR (well-formedness)"} CheckWellformed$$_module.__default.maxR(l#0: Seq where $Is(l#0, TSeq(TInt)));
+  modifies $Heap;
 
 
 
-implementation CheckWellformed$$_module.__default.loop(p#0: int, l#0: Seq Box)
+implementation {:smt_option "smt.arith.solver", "2"} {:verboseName "maxR (well-formedness)"} CheckWellformed$$_module.__default.maxR(l#0: Seq)
 {
-  var $_Frame: <beta>[ref,Field beta]bool;
-  var ##p#0: int;
-  var ##l#0: Seq Box;
-  var b$reqreads#0: bool;
+  var $_ReadsFrame: [ref,Field]bool;
+  var m#Z#0: int;
+  var let#0#0#0: int;
+  var ##l#0: Seq;
 
-    b$reqreads#0 := true;
 
-    // AddWellformednessCheck for function loop
-    assume {:captureState "examples/sorting/boogieOutput.dfy(4,9): initial state"} true;
-    $_Frame := (lambda<alpha> $o: ref, $f: Field alpha :: 
-      $o != null && read($Heap, $o, alloc) ==> false);
+    $_ReadsFrame := (lambda $o: ref, $f: Field :: 
+      $o != null && $Unbox(read($Heap, $o, alloc)): bool ==> false);
+    // Check well-formedness of preconditions, and then assume them
+    // Check well-formedness of the reads clause
+    // Check well-formedness of the decreases clause
+    // Check body and ensures clauses
     if (*)
     {
+        // Check well-formedness of postcondition and assume false
         assume false;
     }
     else
     {
-        $_Frame := (lambda<alpha> $o: ref, $f: Field alpha :: 
-          $o != null && read($Heap, $o, alloc) ==> false);
+        // Check well-formedness of body and result subset type constraint
         if (Seq#Length(l#0) == LitInt(0))
         {
-            assume _module.__default.loop($LS($LZ), p#0, l#0) == Lit(true);
             assume true;
+            assume {:id "id2"} _module.__default.maxR($LS($LZ), l#0) == LitInt(-1);
             // CheckWellformedWithResult: any expression
-            assume $Is(_module.__default.loop($LS($LZ), p#0, l#0), TBool);
-        }
-        else
-        {
-            assert 0 <= LitInt(0) && LitInt(0) < Seq#Length(l#0);
-            if (p#0 <= $Unbox(Seq#Index(l#0, LitInt(0))): int)
-            {
-                assert 0 <= LitInt(0) && LitInt(0) < Seq#Length(l#0);
-                assert 0 <= LitInt(1) && LitInt(1) <= Seq#Length(l#0);
-                ##p#0 := $Unbox(Seq#Index(l#0, LitInt(0))): int;
-                // assume allocatedness for argument to function
-                assume $IsAlloc(##p#0, TInt, $Heap);
-                ##l#0 := Seq#Drop(l#0, LitInt(1));
-                // assume allocatedness for argument to function
-                assume $IsAlloc(##l#0, TSeq(TInt), $Heap);
-                b$reqreads#0 := (forall<alpha> $o: ref, $f: Field alpha :: false ==> $_Frame[$o, $f]);
-                assert Seq#Rank(##l#0) < Seq#Rank(l#0);
-                assume _module.__default.loop#canCall($Unbox(Seq#Index(l#0, LitInt(0))): int, Seq#Drop(l#0, LitInt(1)));
-            }
-
-            assume _module.__default.loop($LS($LZ), p#0, l#0)
-               == (p#0 <= $Unbox(Seq#Index(l#0, LitInt(0))): int
-                 && _module.__default.loop($LS($LZ), $Unbox(Seq#Index(l#0, LitInt(0))): int, Seq#Drop(l#0, LitInt(1))));
-            assume p#0 <= $Unbox(Seq#Index(l#0, LitInt(0))): int
-               ==> _module.__default.loop#canCall($Unbox(Seq#Index(l#0, LitInt(0))): int, Seq#Drop(l#0, LitInt(1)));
-            // CheckWellformedWithResult: any expression
-            assume $Is(_module.__default.loop($LS($LZ), p#0, l#0), TBool);
-        }
-
-        assert b$reqreads#0;
-    }
-}
-
-
-
-// function declaration for _module._default.isSortedR
-function _module.__default.isSortedR(l#0: Seq Box) : bool;
-
-function _module.__default.isSortedR#canCall(l#0: Seq Box) : bool;
-
-// consequence axiom for _module.__default.isSortedR
-axiom 1 <= $FunctionContextHeight
-   ==> (forall l#0: Seq Box :: 
-    { _module.__default.isSortedR(l#0) } 
-    _module.__default.isSortedR#canCall(l#0)
-         || (1 != $FunctionContextHeight && $Is(l#0, TSeq(TInt)))
-       ==> true);
-
-function _module.__default.isSortedR#requires(Seq Box) : bool;
-
-// #requires axiom for _module.__default.isSortedR
-axiom (forall l#0: Seq Box :: 
-  { _module.__default.isSortedR#requires(l#0) } 
-  $Is(l#0, TSeq(TInt)) ==> _module.__default.isSortedR#requires(l#0) == true);
-
-// definition axiom for _module.__default.isSortedR(revealed)
-axiom 1 <= $FunctionContextHeight
-   ==> (forall l#0: Seq Box :: 
-    { _module.__default.isSortedR(l#0) } 
-    _module.__default.isSortedR#canCall(l#0)
-         || (1 != $FunctionContextHeight && $Is(l#0, TSeq(TInt)))
-       ==> (Seq#Length(l#0) != LitInt(0)
-           ==> _module.__default.loop#canCall($Unbox(Seq#Index(l#0, LitInt(0))): int, Seq#Drop(l#0, LitInt(1))))
-         && _module.__default.isSortedR(l#0)
-           == (if Seq#Length(l#0) == LitInt(0)
-             then true
-             else _module.__default.loop($LS($LZ), $Unbox(Seq#Index(l#0, LitInt(0))): int, Seq#Drop(l#0, LitInt(1)))));
-
-// definition axiom for _module.__default.isSortedR for all literals(revealed)
-axiom 1 <= $FunctionContextHeight
-   ==> (forall l#0: Seq Box :: 
-    {:weight 3} { _module.__default.isSortedR(Lit(l#0)) } 
-    _module.__default.isSortedR#canCall(Lit(l#0))
-         || (1 != $FunctionContextHeight && $Is(l#0, TSeq(TInt)))
-       ==> (Seq#Length(Lit(l#0)) != LitInt(0)
-           ==> _module.__default.loop#canCall($Unbox(Seq#Index(Lit(l#0), LitInt(0))): int, Lit(Seq#Drop(Lit(l#0), LitInt(1)))))
-         && _module.__default.isSortedR(Lit(l#0))
-           == (if Seq#Length(Lit(l#0)) == LitInt(0)
-             then true
-             else _module.__default.loop($LS($LZ), 
-              $Unbox(Seq#Index(Lit(l#0), LitInt(0))): int, 
-              Lit(Seq#Drop(Lit(l#0), LitInt(1))))));
-
-procedure CheckWellformed$$_module.__default.isSortedR(l#0: Seq Box where $Is(l#0, TSeq(TInt)));
-  free requires 1 == $FunctionContextHeight;
-  modifies $Heap, $Tick;
-
-
-
-implementation CheckWellformed$$_module.__default.isSortedR(l#0: Seq Box)
-{
-  var $_Frame: <beta>[ref,Field beta]bool;
-  var ##p#0: int;
-  var ##l#0: Seq Box;
-  var b$reqreads#0: bool;
-
-    b$reqreads#0 := true;
-
-    // AddWellformednessCheck for function isSortedR
-    assume {:captureState "examples/sorting/boogieOutput.dfy(11,9): initial state"} true;
-    $_Frame := (lambda<alpha> $o: ref, $f: Field alpha :: 
-      $o != null && read($Heap, $o, alloc) ==> false);
-    if (*)
-    {
-        assume false;
-    }
-    else
-    {
-        $_Frame := (lambda<alpha> $o: ref, $f: Field alpha :: 
-          $o != null && read($Heap, $o, alloc) ==> false);
-        if (Seq#Length(l#0) == LitInt(0))
-        {
-            assume _module.__default.isSortedR(l#0) == Lit(true);
-            assume true;
-            // CheckWellformedWithResult: any expression
-            assume $Is(_module.__default.isSortedR(l#0), TBool);
-        }
-        else
-        {
-            assert 0 <= LitInt(0) && LitInt(0) < Seq#Length(l#0);
-            assert 0 <= LitInt(1) && LitInt(1) <= Seq#Length(l#0);
-            ##p#0 := $Unbox(Seq#Index(l#0, LitInt(0))): int;
-            // assume allocatedness for argument to function
-            assume $IsAlloc(##p#0, TInt, $Heap);
-            ##l#0 := Seq#Drop(l#0, LitInt(1));
-            // assume allocatedness for argument to function
-            assume $IsAlloc(##l#0, TSeq(TInt), $Heap);
-            b$reqreads#0 := (forall<alpha> $o: ref, $f: Field alpha :: false ==> $_Frame[$o, $f]);
-            assume _module.__default.loop#canCall($Unbox(Seq#Index(l#0, LitInt(0))): int, Seq#Drop(l#0, LitInt(1)));
-            assume _module.__default.isSortedR(l#0)
-               == _module.__default.loop($LS($LZ), $Unbox(Seq#Index(l#0, LitInt(0))): int, Seq#Drop(l#0, LitInt(1)));
-            assume _module.__default.loop#canCall($Unbox(Seq#Index(l#0, LitInt(0))): int, Seq#Drop(l#0, LitInt(1)));
-            // CheckWellformedWithResult: any expression
-            assume $Is(_module.__default.isSortedR(l#0), TBool);
-        }
-
-        assert b$reqreads#0;
-    }
-}
-
-
-
-// function declaration for _module._default.isSortedB
-function _module.__default.isSortedB($ly: LayerType, l#0: Seq Box) : bool;
-
-function _module.__default.isSortedB#canCall(l#0: Seq Box) : bool;
-
-// layer synonym axiom
-axiom (forall $ly: LayerType, l#0: Seq Box :: 
-  { _module.__default.isSortedB($LS($ly), l#0) } 
-  _module.__default.isSortedB($LS($ly), l#0)
-     == _module.__default.isSortedB($ly, l#0));
-
-// fuel synonym axiom
-axiom (forall $ly: LayerType, l#0: Seq Box :: 
-  { _module.__default.isSortedB(AsFuelBottom($ly), l#0) } 
-  _module.__default.isSortedB($ly, l#0) == _module.__default.isSortedB($LZ, l#0));
-
-// consequence axiom for _module.__default.isSortedB
-axiom 2 <= $FunctionContextHeight
-   ==> (forall $ly: LayerType, l#0: Seq Box :: 
-    { _module.__default.isSortedB($ly, l#0) } 
-    _module.__default.isSortedB#canCall(l#0)
-         || (2 != $FunctionContextHeight && $Is(l#0, TSeq(TInt)))
-       ==> true);
-
-function _module.__default.isSortedB#requires(LayerType, Seq Box) : bool;
-
-// #requires axiom for _module.__default.isSortedB
-axiom (forall $ly: LayerType, l#0: Seq Box :: 
-  { _module.__default.isSortedB#requires($ly, l#0) } 
-  $Is(l#0, TSeq(TInt)) ==> _module.__default.isSortedB#requires($ly, l#0) == true);
-
-// definition axiom for _module.__default.isSortedB(revealed)
-axiom 2 <= $FunctionContextHeight
-   ==> (forall $ly: LayerType, l#0: Seq Box :: 
-    { _module.__default.isSortedB($LS($ly), l#0) } 
-    _module.__default.isSortedB#canCall(l#0)
-         || (2 != $FunctionContextHeight && $Is(l#0, TSeq(TInt)))
-       ==> (Seq#Length(l#0) != LitInt(0)
-           ==> (Seq#Length(l#0) == LitInt(1)
-               ==> _module.__default.isSortedB#canCall(Lit(Seq#Empty(): Seq Box)))
-             && (Seq#Length(l#0) != LitInt(1)
-               ==> 
-              $Unbox(Seq#Index(l#0, LitInt(0))): int <= $Unbox(Seq#Index(l#0, LitInt(1))): int
-               ==> _module.__default.isSortedB#canCall(Seq#Drop(l#0, LitInt(1)))))
-         && _module.__default.isSortedB($LS($ly), l#0)
-           == (if Seq#Length(l#0) == LitInt(0)
-             then true
-             else (if Seq#Length(l#0) == LitInt(1)
-               then _module.__default.isSortedB($ly, Lit(Seq#Empty(): Seq Box))
-               else $Unbox(Seq#Index(l#0, LitInt(0))): int <= $Unbox(Seq#Index(l#0, LitInt(1))): int
-                 && _module.__default.isSortedB($ly, Seq#Drop(l#0, LitInt(1))))));
-
-// definition axiom for _module.__default.isSortedB for all literals(revealed)
-axiom 2 <= $FunctionContextHeight
-   ==> (forall $ly: LayerType, l#0: Seq Box :: 
-    {:weight 3} { _module.__default.isSortedB($LS($ly), Lit(l#0)) } 
-    _module.__default.isSortedB#canCall(Lit(l#0))
-         || (2 != $FunctionContextHeight && $Is(l#0, TSeq(TInt)))
-       ==> (Seq#Length(Lit(l#0)) != LitInt(0)
-           ==> (Seq#Length(Lit(l#0)) == LitInt(1)
-               ==> _module.__default.isSortedB#canCall(Lit(Seq#Empty(): Seq Box)))
-             && (Seq#Length(Lit(l#0)) != LitInt(1)
-               ==> 
-              $Unbox(Seq#Index(Lit(l#0), LitInt(0))): int
-                 <= $Unbox(Seq#Index(Lit(l#0), LitInt(1))): int
-               ==> _module.__default.isSortedB#canCall(Lit(Seq#Drop(Lit(l#0), LitInt(1))))))
-         && _module.__default.isSortedB($LS($ly), Lit(l#0))
-           == (if Seq#Length(Lit(l#0)) == LitInt(0)
-             then true
-             else (if Seq#Length(Lit(l#0)) == LitInt(1)
-               then _module.__default.isSortedB($LS($ly), Lit(Seq#Empty(): Seq Box))
-               else $Unbox(Seq#Index(Lit(l#0), LitInt(0))): int
-                   <= $Unbox(Seq#Index(Lit(l#0), LitInt(1))): int
-                 && _module.__default.isSortedB($LS($ly), Lit(Seq#Drop(Lit(l#0), LitInt(1)))))));
-
-procedure CheckWellformed$$_module.__default.isSortedB(l#0: Seq Box where $Is(l#0, TSeq(TInt)));
-  free requires 2 == $FunctionContextHeight;
-  modifies $Heap, $Tick;
-
-
-
-implementation CheckWellformed$$_module.__default.isSortedB(l#0: Seq Box)
-{
-  var $_Frame: <beta>[ref,Field beta]bool;
-  var ##l#0: Seq Box;
-  var ##l#1: Seq Box;
-  var b$reqreads#0: bool;
-  var b$reqreads#1: bool;
-
-    b$reqreads#0 := true;
-    b$reqreads#1 := true;
-
-    // AddWellformednessCheck for function isSortedB
-    assume {:captureState "examples/sorting/boogieOutput.dfy(18,9): initial state"} true;
-    $_Frame := (lambda<alpha> $o: ref, $f: Field alpha :: 
-      $o != null && read($Heap, $o, alloc) ==> false);
-    if (*)
-    {
-        assume false;
-    }
-    else
-    {
-        $_Frame := (lambda<alpha> $o: ref, $f: Field alpha :: 
-          $o != null && read($Heap, $o, alloc) ==> false);
-        if (Seq#Length(l#0) == LitInt(0))
-        {
-            assume _module.__default.isSortedB($LS($LZ), l#0) == Lit(true);
-            assume true;
-            // CheckWellformedWithResult: any expression
-            assume $Is(_module.__default.isSortedB($LS($LZ), l#0), TBool);
+            assume $Is(_module.__default.maxR($LS($LZ), l#0), TInt);
+            return;
         }
         else
         {
             if (Seq#Length(l#0) == LitInt(1))
             {
-                ##l#0 := Lit(Seq#Empty(): Seq Box);
-                // assume allocatedness for argument to function
-                assume $IsAlloc(##l#0, TSeq(TInt), $Heap);
-                b$reqreads#0 := (forall<alpha> $o: ref, $f: Field alpha :: false ==> $_Frame[$o, $f]);
-                assert 0 <= Seq#Length(l#0) || Seq#Length(##l#0) == Seq#Length(l#0);
-                assert Seq#Length(##l#0) < Seq#Length(l#0);
-                assume _module.__default.isSortedB#canCall(Lit(Seq#Empty(): Seq Box));
-                assume _module.__default.isSortedB($LS($LZ), l#0)
-                   == Lit(_module.__default.isSortedB($LS($LZ), Lit(Seq#Empty(): Seq Box)));
-                assume _module.__default.isSortedB#canCall(Lit(Seq#Empty(): Seq Box));
+                assert {:id "id3"} 0 <= LitInt(0) && LitInt(0) < Seq#Length(l#0);
+                assume true;
+                assume {:id "id4"} _module.__default.maxR($LS($LZ), l#0) == $Unbox(Seq#Index(l#0, LitInt(0))): int;
                 // CheckWellformedWithResult: any expression
-                assume $Is(_module.__default.isSortedB($LS($LZ), l#0), TBool);
+                assume $Is(_module.__default.maxR($LS($LZ), l#0), TInt);
+                return;
             }
             else
             {
-                assert 0 <= LitInt(0) && LitInt(0) < Seq#Length(l#0);
-                assert 0 <= LitInt(1) && LitInt(1) < Seq#Length(l#0);
-                if ($Unbox(Seq#Index(l#0, LitInt(0))): int <= $Unbox(Seq#Index(l#0, LitInt(1))): int)
-                {
-                    assert 0 <= LitInt(1) && LitInt(1) <= Seq#Length(l#0);
-                    ##l#1 := Seq#Drop(l#0, LitInt(1));
-                    // assume allocatedness for argument to function
-                    assume $IsAlloc(##l#1, TSeq(TInt), $Heap);
-                    b$reqreads#1 := (forall<alpha> $o: ref, $f: Field alpha :: false ==> $_Frame[$o, $f]);
-                    assert 0 <= Seq#Length(l#0) || Seq#Length(##l#1) == Seq#Length(l#0);
-                    assert Seq#Length(##l#1) < Seq#Length(l#0);
-                    assume _module.__default.isSortedB#canCall(Seq#Drop(l#0, LitInt(1)));
-                }
-
-                assume _module.__default.isSortedB($LS($LZ), l#0)
-                   == ($Unbox(Seq#Index(l#0, LitInt(0))): int <= $Unbox(Seq#Index(l#0, LitInt(1))): int
-                     && _module.__default.isSortedB($LS($LZ), Seq#Drop(l#0, LitInt(1))));
-                assume $Unbox(Seq#Index(l#0, LitInt(0))): int <= $Unbox(Seq#Index(l#0, LitInt(1))): int
-                   ==> _module.__default.isSortedB#canCall(Seq#Drop(l#0, LitInt(1)));
+                havoc m#Z#0;
+                assert {:id "id5"} 0 <= LitInt(1) && LitInt(1) <= Seq#Length(l#0);
+                ##l#0 := Seq#Drop(l#0, LitInt(1));
+                // assume allocatedness for argument to function
+                assume $IsAlloc(##l#0, TSeq(TInt), $Heap);
+                assume true;
+                assert {:id "id6"} Seq#Rank(##l#0) < Seq#Rank(l#0);
+                assume _module.__default.maxR#canCall(Seq#Drop(l#0, LitInt(1)));
+                assume _module.__default.maxR#canCall(Seq#Drop(l#0, LitInt(1)));
+                assume {:id "id7"} let#0#0#0 == _module.__default.maxR($LS($LZ), Seq#Drop(l#0, LitInt(1)));
                 // CheckWellformedWithResult: any expression
-                assume $Is(_module.__default.isSortedB($LS($LZ), l#0), TBool);
+                assume $Is(let#0#0#0, TInt);
+                assume {:id "id8"} m#Z#0 == let#0#0#0;
+                assert {:id "id9"} 0 <= LitInt(0) && LitInt(0) < Seq#Length(l#0);
+                if ($Unbox(Seq#Index(l#0, LitInt(0))): int > m#Z#0)
+                {
+                    assert {:id "id10"} 0 <= LitInt(0) && LitInt(0) < Seq#Length(l#0);
+                    assume true;
+                    assume {:id "id11"} _module.__default.maxR($LS($LZ), l#0) == $Unbox(Seq#Index(l#0, LitInt(0))): int;
+                    // CheckWellformedWithResult: any expression
+                    assume $Is(_module.__default.maxR($LS($LZ), l#0), TInt);
+                    return;
+                }
+                else
+                {
+                    assume true;
+                    assume {:id "id12"} _module.__default.maxR($LS($LZ), l#0) == m#Z#0;
+                    // CheckWellformedWithResult: any expression
+                    assume $Is(_module.__default.maxR($LS($LZ), l#0), TInt);
+                    return;
+                }
             }
         }
 
-        assert b$reqreads#0;
-        assert b$reqreads#1;
+        assume false;
     }
 }
 
 
 
-procedure {:_induction l#0} CheckWellformed$$_module.__default.isSortedEquivalence(l#0: Seq Box where $Is(l#0, TSeq(TInt)) && $IsAlloc(l#0, TSeq(TInt), $Heap));
-  free requires 3 == $FunctionContextHeight;
-  modifies $Heap, $Tick;
+// function declaration for _module._default.maxC
+function _module.__default.maxC($ly: LayerType, l#0: Seq) : int;
+
+function _module.__default.maxC#canCall(l#0: Seq) : bool;
+
+// layer synonym axiom
+axiom (forall $ly: LayerType, l#0: Seq :: 
+  { _module.__default.maxC($LS($ly), l#0) } 
+  _module.__default.maxC($LS($ly), l#0) == _module.__default.maxC($ly, l#0));
+
+// fuel synonym axiom
+axiom (forall $ly: LayerType, l#0: Seq :: 
+  { _module.__default.maxC(AsFuelBottom($ly), l#0) } 
+  _module.__default.maxC($ly, l#0) == _module.__default.maxC($LZ, l#0));
+
+function _module.__default.maxC#requires(LayerType, Seq) : bool;
+
+// #requires axiom for _module.__default.maxC
+axiom (forall $ly: LayerType, l#0: Seq :: 
+  { _module.__default.maxC#requires($ly, l#0) } 
+  $Is(l#0, TSeq(TInt)) ==> _module.__default.maxC#requires($ly, l#0) == true);
+
+// #requires ==> #canCall for _module.__default.maxC
+axiom (forall $ly: LayerType, l#0: Seq :: 
+  { _module.__default.maxC#requires($ly, l#0) } 
+  _module.__default.maxC#requires($ly, l#0)
+     ==> _module.__default.maxC#canCall(l#0));
+
+// definition axiom for _module.__default.maxC (revealed)
+axiom {:id "id13"} (forall $ly: LayerType, l#0: Seq :: 
+  { _module.__default.maxC($LS($ly), l#0) } 
+  _module.__default.maxC#canCall(l#0)
+     ==> (Seq#Length(l#0) != LitInt(0)
+         ==> 
+        Seq#Length(l#0) != LitInt(1)
+         ==> (var a#0 := $Unbox(Seq#Index(l#0, LitInt(0))): int; 
+          (var b#0 := $Unbox(Seq#Index(l#0, LitInt(1))): int; 
+            (a#0 > b#0
+                 ==> _module.__default.maxC#canCall(Seq#Append(Seq#Build(Seq#Empty(): Seq, Seq#Index(l#0, LitInt(0))), Seq#Drop(l#0, LitInt(2)))))
+               && (b#0 >= a#0 ==> _module.__default.maxC#canCall(Seq#Drop(l#0, LitInt(1)))))))
+       && _module.__default.maxC($LS($ly), l#0)
+         == (if Seq#Length(l#0) == LitInt(0)
+           then -1
+           else (if Seq#Length(l#0) == LitInt(1)
+             then $Unbox(Seq#Index(l#0, LitInt(0))): int
+             else (var a#0 := $Unbox(Seq#Index(l#0, LitInt(0))): int; 
+              (var b#0 := $Unbox(Seq#Index(l#0, LitInt(1))): int; 
+                (if a#0 > b#0
+                   then _module.__default.maxC($ly, 
+                    Seq#Append(Seq#Build(Seq#Empty(): Seq, Seq#Index(l#0, LitInt(0))), Seq#Drop(l#0, LitInt(2))))
+                   else _module.__default.maxC($ly, Seq#Drop(l#0, LitInt(1)))))))));
+
+// definition axiom for _module.__default.maxC for all literals (revealed)
+axiom {:id "id14"} (forall $ly: LayerType, l#0: Seq :: 
+  {:weight 3} { _module.__default.maxC($LS($ly), Lit(l#0)) } 
+  _module.__default.maxC#canCall(Lit(l#0))
+     ==> (Seq#Length(Lit(l#0)) != LitInt(0)
+         ==> 
+        Seq#Length(Lit(l#0)) != LitInt(1)
+         ==> (var a#1 := $Unbox(Seq#Index(Lit(l#0), LitInt(0))): int; 
+          (var b#1 := $Unbox(Seq#Index(Lit(l#0), LitInt(1))): int; 
+            (a#1 > b#1
+                 ==> _module.__default.maxC#canCall(Seq#Append(Seq#Build(Seq#Empty(): Seq, Seq#Index(Lit(l#0), LitInt(0))), 
+                    Seq#Drop(Lit(l#0), LitInt(2)))))
+               && (b#1 >= a#1
+                 ==> _module.__default.maxC#canCall(Lit(Seq#Drop(Lit(l#0), LitInt(1))))))))
+       && _module.__default.maxC($LS($ly), Lit(l#0))
+         == (if Seq#Length(Lit(l#0)) == LitInt(0)
+           then -1
+           else (if Seq#Length(Lit(l#0)) == LitInt(1)
+             then $Unbox(Seq#Index(Lit(l#0), LitInt(0))): int
+             else (var a#1 := $Unbox(Seq#Index(Lit(l#0), LitInt(0))): int; 
+              (var b#1 := $Unbox(Seq#Index(Lit(l#0), LitInt(1))): int; 
+                (if a#1 > b#1
+                   then _module.__default.maxC($LS($ly), 
+                    Seq#Append(Seq#Build(Seq#Empty(): Seq, Seq#Index(Lit(l#0), LitInt(0))), 
+                      Seq#Drop(Lit(l#0), LitInt(2))))
+                   else _module.__default.maxC($LS($ly), Lit(Seq#Drop(Lit(l#0), LitInt(1))))))))));
+
+procedure {:verboseName "maxC (well-formedness)"} CheckWellformed$$_module.__default.maxC(l#0: Seq where $Is(l#0, TSeq(TInt)));
+  modifies $Heap;
 
 
 
-procedure {:_induction l#0} Call$$_module.__default.isSortedEquivalence(l#0: Seq Box where $Is(l#0, TSeq(TInt)) && $IsAlloc(l#0, TSeq(TInt), $Heap));
-  modifies $Heap, $Tick;
-  // user-defined postconditions
-  free ensures _module.__default.isSortedR#canCall(l#0)
-     && _module.__default.isSortedB#canCall(l#0);
-  ensures _module.__default.isSortedR(l#0)
-     == _module.__default.isSortedB($LS($LS($LZ)), l#0);
-  // frame condition
-  free ensures old($Heap) == $Heap;
-
-
-
-procedure {:_induction l#0} Impl$$_module.__default.isSortedEquivalence(l#0: Seq Box where $Is(l#0, TSeq(TInt)) && $IsAlloc(l#0, TSeq(TInt), $Heap))
-   returns ($_reverifyPost: bool);
-  free requires 3 == $FunctionContextHeight;
-  modifies $Heap, $Tick;
-  // user-defined postconditions
-  free ensures _module.__default.isSortedR#canCall(l#0)
-     && _module.__default.isSortedB#canCall(l#0);
-  ensures _module.__default.isSortedR(l#0)
-     == _module.__default.isSortedB($LS($LS($LZ)), l#0);
-  // frame condition
-  free ensures old($Heap) == $Heap;
-
-
-
-implementation {:_induction l#0} Impl$$_module.__default.isSortedEquivalence(l#0: Seq Box) returns ($_reverifyPost: bool)
+implementation {:smt_option "smt.arith.solver", "2"} {:verboseName "maxC (well-formedness)"} CheckWellformed$$_module.__default.maxC(l#0: Seq)
 {
-  var $_Frame: <beta>[ref,Field beta]bool;
+  var $_ReadsFrame: [ref,Field]bool;
+  var a#Z#0: int;
+  var let#0#0#0: int;
+  var b#Z#0: int;
+  var let#1#0#0: int;
+  var ##l#0: Seq;
+  var ##l#1: Seq;
+
+
+    $_ReadsFrame := (lambda $o: ref, $f: Field :: 
+      $o != null && $Unbox(read($Heap, $o, alloc)): bool ==> false);
+    // Check well-formedness of preconditions, and then assume them
+    // Check well-formedness of the reads clause
+    // Check well-formedness of the decreases clause
+    // Check body and ensures clauses
+    if (*)
+    {
+        // Check well-formedness of postcondition and assume false
+        assume false;
+    }
+    else
+    {
+        // Check well-formedness of body and result subset type constraint
+        if (Seq#Length(l#0) == LitInt(0))
+        {
+            assume true;
+            assume {:id "id15"} _module.__default.maxC($LS($LZ), l#0) == LitInt(-1);
+            // CheckWellformedWithResult: any expression
+            assume $Is(_module.__default.maxC($LS($LZ), l#0), TInt);
+            return;
+        }
+        else
+        {
+            if (Seq#Length(l#0) == LitInt(1))
+            {
+                assert {:id "id16"} 0 <= LitInt(0) && LitInt(0) < Seq#Length(l#0);
+                assume true;
+                assume {:id "id17"} _module.__default.maxC($LS($LZ), l#0) == $Unbox(Seq#Index(l#0, LitInt(0))): int;
+                // CheckWellformedWithResult: any expression
+                assume $Is(_module.__default.maxC($LS($LZ), l#0), TInt);
+                return;
+            }
+            else
+            {
+                havoc a#Z#0;
+                assert {:id "id18"} 0 <= LitInt(0) && LitInt(0) < Seq#Length(l#0);
+                assume true;
+                assume {:id "id19"} let#0#0#0 == $Unbox(Seq#Index(l#0, LitInt(0))): int;
+                // CheckWellformedWithResult: any expression
+                assume $Is(let#0#0#0, TInt);
+                assume {:id "id20"} a#Z#0 == let#0#0#0;
+                havoc b#Z#0;
+                assert {:id "id21"} 0 <= LitInt(1) && LitInt(1) < Seq#Length(l#0);
+                assume true;
+                assume {:id "id22"} let#1#0#0 == $Unbox(Seq#Index(l#0, LitInt(1))): int;
+                // CheckWellformedWithResult: any expression
+                assume $Is(let#1#0#0, TInt);
+                assume {:id "id23"} b#Z#0 == let#1#0#0;
+                if (a#Z#0 > b#Z#0)
+                {
+                    assert {:id "id24"} 0 <= LitInt(0) && LitInt(0) < Seq#Length(l#0);
+                    assert {:id "id25"} 0 <= LitInt(2) && LitInt(2) <= Seq#Length(l#0);
+                    ##l#0 := Seq#Append(Seq#Build(Seq#Empty(): Seq, Seq#Index(l#0, LitInt(0))), Seq#Drop(l#0, LitInt(2)));
+                    // assume allocatedness for argument to function
+                    assume $IsAlloc(##l#0, TSeq(TInt), $Heap);
+                    assume true;
+                    assert {:id "id26"} 0 <= Seq#Length(l#0) || Seq#Length(##l#0) == Seq#Length(l#0);
+                    assert {:id "id27"} Seq#Length(##l#0) < Seq#Length(l#0);
+                    assume _module.__default.maxC#canCall(Seq#Append(Seq#Build(Seq#Empty(): Seq, Seq#Index(l#0, LitInt(0))), Seq#Drop(l#0, LitInt(2))));
+                    assume _module.__default.maxC#canCall(Seq#Append(Seq#Build(Seq#Empty(): Seq, Seq#Index(l#0, LitInt(0))), Seq#Drop(l#0, LitInt(2))));
+                    assume {:id "id28"} _module.__default.maxC($LS($LZ), l#0)
+                       == _module.__default.maxC($LS($LZ), 
+                        Seq#Append(Seq#Build(Seq#Empty(): Seq, Seq#Index(l#0, LitInt(0))), Seq#Drop(l#0, LitInt(2))));
+                    // CheckWellformedWithResult: any expression
+                    assume $Is(_module.__default.maxC($LS($LZ), l#0), TInt);
+                    return;
+                }
+                else
+                {
+                    assert {:id "id29"} 0 <= LitInt(1) && LitInt(1) <= Seq#Length(l#0);
+                    ##l#1 := Seq#Drop(l#0, LitInt(1));
+                    // assume allocatedness for argument to function
+                    assume $IsAlloc(##l#1, TSeq(TInt), $Heap);
+                    assume true;
+                    assert {:id "id30"} 0 <= Seq#Length(l#0) || Seq#Length(##l#1) == Seq#Length(l#0);
+                    assert {:id "id31"} Seq#Length(##l#1) < Seq#Length(l#0);
+                    assume _module.__default.maxC#canCall(Seq#Drop(l#0, LitInt(1)));
+                    assume _module.__default.maxC#canCall(Seq#Drop(l#0, LitInt(1)));
+                    assume {:id "id32"} _module.__default.maxC($LS($LZ), l#0)
+                       == _module.__default.maxC($LS($LZ), Seq#Drop(l#0, LitInt(1)));
+                    // CheckWellformedWithResult: any expression
+                    assume $Is(_module.__default.maxC($LS($LZ), l#0), TInt);
+                    return;
+                }
+            }
+        }
+
+        assume false;
+    }
+}
+
+
+
+procedure {:verboseName "maxEquivalence (well-formedness)"} CheckWellFormed$$_module.__default.maxEquivalence(l#0: Seq where $Is(l#0, TSeq(TInt)) && $IsAlloc(l#0, TSeq(TInt), $Heap));
+  modifies $Heap;
+
+
+
+procedure {:verboseName "maxEquivalence (call)"} Call$$_module.__default.maxEquivalence(l#0: Seq where $Is(l#0, TSeq(TInt)) && $IsAlloc(l#0, TSeq(TInt), $Heap));
+  modifies $Heap;
+  // user-defined postconditions
+  free ensures {:always_assume} _module.__default.maxC#canCall(l#0) && _module.__default.maxR#canCall(l#0);
+  ensures {:id "id34"} _module.__default.maxC($LS($LS($LZ)), l#0)
+     == _module.__default.maxR($LS($LS($LZ)), l#0);
+  // frame condition
+  free ensures old($Heap) == $Heap;
+
+
+
+procedure {:verboseName "maxEquivalence (correctness)"} Impl$$_module.__default.maxEquivalence(l#0: Seq where $Is(l#0, TSeq(TInt)) && $IsAlloc(l#0, TSeq(TInt), $Heap))
+   returns ($_reverifyPost: bool);
+  modifies $Heap;
+  // user-defined postconditions
+  free ensures {:always_assume} _module.__default.maxC#canCall(l#0) && _module.__default.maxR#canCall(l#0);
+  ensures {:id "id35"} _module.__default.maxC($LS($LS($LZ)), l#0)
+     == _module.__default.maxR($LS($LS($LZ)), l#0);
+  // frame condition
+  free ensures old($Heap) == $Heap;
+
+
+
+implementation {:smt_option "smt.arith.solver", "2"} {:verboseName "maxEquivalence (correctness)"} Impl$$_module.__default.maxEquivalence(l#0: Seq) returns ($_reverifyPost: bool)
+{
+  var $_ModifiesFrame: [ref,Field]bool;
   var $initHeapForallStmt#0: Heap;
 
-    // AddMethodImpl: isSortedEquivalence, Impl$$_module.__default.isSortedEquivalence
-    $_Frame := (lambda<alpha> $o: ref, $f: Field alpha :: 
-      $o != null && read($Heap, $o, alloc) ==> false);
-    assume {:captureState "examples/sorting/boogieOutput.dfy(29,0): initial state"} true;
+    // AddMethodImpl: maxEquivalence, Impl$$_module.__default.maxEquivalence
+    $_ModifiesFrame := (lambda $o: ref, $f: Field :: 
+      $o != null && $Unbox(read($Heap, $o, alloc)): bool ==> false);
     $initHeapForallStmt#0 := $Heap;
-    havoc $Heap, $Tick;
+    havoc $Heap;
     assume $initHeapForallStmt#0 == $Heap;
-    assume (forall $ih#l0#0: Seq Box :: 
-      $Is($ih#l0#0, TSeq(TInt)) && Lit(true) && Seq#Rank($ih#l0#0) < Seq#Rank(l#0)
-         ==> _module.__default.isSortedR($ih#l0#0)
-           == _module.__default.isSortedB($LS($LZ), $ih#l0#0));
+    assume (forall $ih#l0#0: Seq :: 
+      { _module.__default.maxR($LS($LZ), $ih#l0#0) } 
+        { _module.__default.maxC($LS($LZ), $ih#l0#0) } 
+      $Is($ih#l0#0, TSeq(TInt))
+           && Lit(true)
+           && 
+          0 <= Seq#Length($ih#l0#0)
+           && Seq#Length($ih#l0#0) < Seq#Length(l#0)
+         ==> _module.__default.maxC#canCall($ih#l0#0)
+           && _module.__default.maxR#canCall($ih#l0#0)
+           && _module.__default.maxC($LS($LZ), $ih#l0#0)
+             == _module.__default.maxR($LS($LZ), $ih#l0#0));
     $_reverifyPost := false;
 }
 
 
+
+const unique tytagFamily$nat: TyTagFamily;
+
+const unique tytagFamily$object: TyTagFamily;
+
+const unique tytagFamily$array: TyTagFamily;
+
+const unique tytagFamily$_#Func1: TyTagFamily;
+
+const unique tytagFamily$_#PartialFunc1: TyTagFamily;
+
+const unique tytagFamily$_#TotalFunc1: TyTagFamily;
+
+const unique tytagFamily$_#Func0: TyTagFamily;
+
+const unique tytagFamily$_#PartialFunc0: TyTagFamily;
+
+const unique tytagFamily$_#TotalFunc0: TyTagFamily;
+
+const unique tytagFamily$_tuple#2: TyTagFamily;
+
+const unique tytagFamily$_tuple#0: TyTagFamily;
